Much work done.  Merging potentially incompatible maps is a nightmare.  Need to refactor to avoid the problem.

KeyManagement/RealWorld.v
@@ -1,4 +1,4 @@
-From Coq Require Import String Sumbool.
+From Coq Require Import String Sumbool Morphisms.
 
 Require Import MyPrelude Common Maps.
 
@@ -15,45 +15,40 @@ Lemma key_usage_eq_dec :
   decide equality.
 Defined.
 
-(* A master key type *)
 Inductive key_type :=
 | SymKey
-| AsymKey (has_private_access : bool).
-
-Definition key_type_same (kt1 kt2 : key_type) :=
-  match (kt1,kt2) with
-  | (AsymKey _, AsymKey _) => true
-  | (SymKey   , SymKey   ) => true
-  | _                      => false
-  end.
+| AsymKey.
 
 Lemma key_type_eq_dec :
   forall kt1 kt2 : key_type, { kt1 = kt2 } + { kt1 <> kt2 }.
-  decide equality; auto using Bool.bool_dec.
+  decide equality.
 Defined.
 
-Record key := MkCryptoKey { keyId : key_identifier ;
-                            keyUsage  : key_usage ;
-                            keyType : key_type }.
+Record key :=
+  MkCryptoKey { keyId    : key_identifier
+              ; keyUsage : key_usage
+              ; keyType  : key_type
+              }.
 
 Lemma key_eq_dec :
   forall k1 k2 : key, { k1 = k2 } + { k1 <> k2 }.
   decide equality; auto using Nat.eq_dec, key_usage_eq_dec, key_type_eq_dec.
 Defined.
 
+Record key_permission :=
+  MkKeyPerm { key_ref            : key_identifier
+            ; has_private_access : bool
+            }.
+
+Lemma key_permission_eq_dec :
+  forall kp1 kp2 : key_permission, { kp1 = kp2 } + { kp1 <> kp2 }.
+  decide equality; auto using Nat.eq_dec, Bool.bool_dec.
+Defined.
+
 Notation "x ==kk y" := (key_eq_dec x y) (right associativity, at level 75).
 Notation "x ==ku y" := (key_usage_eq_dec x y) (right associativity, at level 75).
 Notation "x ==kt y" := (key_type_eq_dec x y) (right associativity, at level 75).
-
-Definition keys_compatible (k1 k2 : key) :=
-  if   k1.(keyId) ==n k2.(keyId)
-  then if   k1.(keyUsage) ==ku k2.(keyUsage)
-       then key_type_same k1.(keyType) k2.(keyType)
-       else false
-  else false.
-
-Definition keyEq k1 k2 := k1.(keyId) = k2.(keyId).
-Notation "x ==k y" := (keyEq x y) (right associativity, at level 75).
+Notation "x ==kp y" := (key_permission_eq_dec x y) (right associativity, at level 75).
 
 Definition cipher_id := nat.
 
@@ -68,7 +63,7 @@ Inductive type : Set :=
 Fixpoint typeDenote (t : type) : Set :=
   match t with
   | Nat => nat
-  | Key => key
+  | Key => key_permission
   | CipherId => cipher_id
   | Pair t1 t2 => typeDenote t1 * typeDenote t2
   end.
@@ -76,7 +71,7 @@ Fixpoint typeDenote (t : type) : Set :=
 Inductive message : type -> Type :=
 (* This will eventually be a message Text, using nat for now *)
 | Plaintext (txt : nat) : message Nat
-| KeyMessage  (k : key) : message Key
+| KeyMessage  (k : key_permission) : message Key
 
 | MsgPair {t1 t2 : type} (msg1 : message t1) (msg2 : message t2) : message (Pair t1 t2)
 
@@ -105,9 +100,8 @@ Definition cipher_signing_key (c : cipher) :=
 
 Definition queued_messages := list (sigT message).
 Definition keys            := NatMap.t key.
+Definition key_perms       := NatMap.t key_permission.
 Definition ciphers         := NatMap.t cipher.
-
-(* Definition adversary_knowledge := keys. *)
 
 Inductive msg_accepted_by_pattern (cs : ciphers) (pat : msg_pat) : forall {t : type}, message t -> Prop :=
 | MsgAccept : forall {t} (m : message t),
@@ -131,74 +125,132 @@ Inductive msg_accepted_by_pattern (cs : ciphers) (pat : msg_pat) : forall {t : t
     -> msg_accepted_by_pattern cs pat m
 .
 
+Ltac clean_map_lookups1 :=
+  match goal with
+  | [ H : Some _ = None   |- _ ] => invert H
+  | [ H : None = Some _   |- _ ] => invert H
+  | [ H : Some _ = Some _ |- _ ] => invert H
+  | [ H : $0 $? _ = Some _ |- _ ] => invert H
+  | [ H : _ $+ (?k,_) $? ?k = _ |- _ ] => rewrite add_eq_o in H by trivial
+  | [ H : _ $+ (?k1,_) $? ?k2 = _ |- _ ] => rewrite add_neq_o in H by auto
+  | [ |- context[_ $+ (?k,_) $? ?k] ] => rewrite add_eq_o by trivial
+  | [ |- context[_ $+ (?k1,_) $? ?k2] ] => rewrite add_neq_o by auto
+  | [ H : ~ In _ _ |- _ ] => rewrite not_find_in_iff in H
+  | [ H1 : ?m $? ?k = _ , H2 : ?m $? ?k = _ |- _] => rewrite H1 in H2
+  end.
+
+Ltac contra_map_lookup :=
+  match goal with
+  | [ H1 : ?ks $? ?k = Some _, H2 : ?ks $? ?k = None |- _ ] => rewrite H1 in H2; invert H2
+  | [ H : ?v1 <> ?v2, H1 : ?ks $? ?k = Some ?v1, H2 : ?ks $? ?k = Some ?v2 |- _ ] => rewrite H1 in H2; invert H2; contradiction
+  end.
+
+Ltac clean_map_lookups :=
+  (repeat clean_map_lookups1);
+  try discriminate;
+  try contra_map_lookup.
+
+Ltac split_ands :=
+  repeat match goal with
+         | [ H : _ /\ _ |- _ ] => destruct H
+         end.
+
+Ltac split_ors :=
+  repeat match goal with
+         | [ H : _ \/ _ |- _ ] => destruct H
+         end.
+
+Hint Extern 1 (~ In _ _) => rewrite not_find_in_iff.
+
 Section SafeMessages.
-  Variable honestk advk : keys.
+  Variable all_keys : keys.
+  Variable honestk advk : key_perms.
+
+  Definition has_private_key (k : key_permission) : bool :=
+    match (all_keys $? k.(key_ref)) with
+    | None      => false
+    | Some (MkCryptoKey _ _ SymKey)  => true
+    | Some (MkCryptoKey _ _ AsymKey) => k.(has_private_access)
+    end.
+
+    Definition honest_key (k : key_identifier) : bool :=
+    match all_keys $? k with
+    | None                           => false
+    | Some (MkCryptoKey _ _ SymKey)  =>
+      match honestk $? k with
+      | None   => false
+      | Some _ => true
+      end
+    | Some (MkCryptoKey _ _ AsymKey) =>
+      match honestk $? k with
+      | None                        => false
+      | Some (MkKeyPerm _ has_priv) => has_priv
+      end
+    end.
 
   Definition honest_signing_key (k : key_identifier) : bool :=
-    match honestk $? k with
-    | None   => false
-    | Some (MkCryptoKey _ Signing SymKey)         =>
-      match advk $? k with
-      | None   => true
-      | Some _ => false
-      end
-    | Some (MkCryptoKey _ Signing (AsymKey true)) =>
-      match advk $? k with
-      | None => true
-      | Some (MkCryptoKey _ Signing (AsymKey false)) => true
-      | _    => false
-      end
-    | Some _ => false
-    end.
+    honest_key k
+      && match all_keys $? k with
+         | Some (MkCryptoKey _ Signing _) => true
+         | _                              => false
+         end.
+
+  Definition honest_encryption_key (k : key_identifier) : bool :=
+    honest_key k
+      && match all_keys $? k with
+         | Some (MkCryptoKey _ Encryption _) => true
+         | _                              => false
+         end.
 
   Fixpoint msg_needs_encryption {t} (msg : message t) : bool :=
     match msg with
-    | Plaintext _ => false
-    | KeyMessage k =>
-      match honestk $? k.(keyId) with
-      | Some (MkCryptoKey _ _ SymKey)         => true
-      | Some (MkCryptoKey _ _ (AsymKey true)) => true
-      | _                                     => false
-      end
-    | MsgPair msg1 msg2 => msg_needs_encryption msg1 || msg_needs_encryption msg2
+    | Plaintext _        => false
+    | KeyMessage k       => match all_keys $? k.(key_ref) with
+                           | None   => false
+                           | Some _ => honest_key k.(key_ref)
+                           end
+    | MsgPair msg1 msg2  => msg_needs_encryption msg1 || msg_needs_encryption msg2
     | SignedCiphertext _ => false
-    | Signature msg _ => msg_needs_encryption msg
+    | Signature msg _    => msg_needs_encryption msg
     end.
 
   Definition cipher_adversary_safe (c : cipher) : bool :=
     match c with
     | SigCipher _ k_id msg              => negb (msg_needs_encryption msg)
-    | SigEncCipher _ k__signid k__encid msg =>
-      negb (msg_needs_encryption msg)
-      || match honestk $? k__encid with
-        | Some (MkCryptoKey _ Encryption (AsymKey true)) =>
-          match advk $? k__encid with
-          | None => true
-          | Some (MkCryptoKey _ Encryption (AsymKey false)) => true
-          | _    => false
-          end
-        | Some (MkCryptoKey _ Encryption SymKey)         => 
-          match advk $? k__encid with
-          | None   => true
-          | Some _ => false
-          end
-        | Some _ => false
-        | None   => false
-        end
+    | SigEncCipher _ k__signid k__encid msg => negb (msg_needs_encryption msg)
+                                          || honest_encryption_key k__encid
     end.
+
+  Definition cipher_honestly_signed (c : cipher) : bool :=
+    match c with
+    | SigCipher _ k_id _              => honest_signing_key k_id
+    | SigEncCipher _ k__signid k__encid _ => honest_signing_key k__signid
+    end.
+
+  Definition ciphers_honestly_signed (cs : ciphers) : bool :=
+    for_all (fun _ => cipher_honestly_signed) cs.
 
   Definition message_queue_safe : queued_messages -> bool :=
     forallb (fun m => match m with | existT _ _ msg => msg_needs_encryption msg end).
 
+  Fixpoint msg_pattern_spoofable (pat : msg_pat) : bool :=
+    match pat with
+    | Accept                     => true
+    | Paired p1 p2               => msg_pattern_spoofable p1 || msg_pattern_spoofable p2
+    | Signed k                   => negb (honest_signing_key k)
+    | SignedEncrypted k__sign k__enc => negb (honest_signing_key k__sign)
+    end.
+
 End SafeMessages.
 
-Fixpoint msg_pattern_spoofable (honestk advk : keys) (pat : msg_pat) : bool :=
-  match pat with
-  | Accept                     => true
-  | Paired p1 p2               => msg_pattern_spoofable honestk advk p1 || msg_pattern_spoofable honestk advk p2
-  | Signed k                   => negb (honest_signing_key honestk advk k)
-  | SignedEncrypted k__sign k__enc => negb (honest_signing_key honestk advk k__sign)
-  end.
+Lemma cipher_honestly_signed_proper :
+  forall ks perms,
+    Proper (eq ==> eq ==> eq) (fun _ : NatMap.key => cipher_honestly_signed ks perms).
+Proof.
+  unfold Proper, respectful; intros; subst; eauto.
+Qed.
+
+Hint Resolve cipher_honestly_signed_proper.
 
 Inductive user_cmd : Type -> Type :=
 (* Plumbing *)
@@ -212,14 +264,14 @@ Inductive user_cmd : Type -> Type :=
 | Recv {t} (pat : msg_pat) : user_cmd (message t)
 
 (* Crypto!! *)
-| SignEncrypt {t} (k__sign k__enc : key) (msg : message t) : user_cmd (message CipherId)
+| SignEncrypt {t} (k__sign k__enc : key_permission) (msg : message t) : user_cmd (message CipherId)
 | Decrypt {t} (msg : message CipherId) : user_cmd (message t)
 
-| Sign    {t} (k : key) (msg : message t) : user_cmd (message t)
-| Verify  {t} (k : key) (msg : message t) : user_cmd bool
+| Sign    {t} (k : key_permission) (msg : message t) : user_cmd (message t)
+| Verify  {t} (k : key_permission) (msg : message t) : user_cmd bool
 
-| GenerateSymKey  (usage : key_usage) : user_cmd key
-| GenerateAsymKey (usage : key_usage) : user_cmd key
+| GenerateSymKey  (usage : key_usage) : user_cmd key_permission
+| GenerateAsymKey (usage : key_usage) : user_cmd key_permission
 
 (* Allow administrator to make some global change to the universe -- revoke keys, etc. *)
 (* This may be a universe level step -- Administrator forces all users to stop *)
@@ -235,7 +287,7 @@ Open Scope realworld_scope.
 
 Record user_data (A : Type) :=
   mkUserData {
-      key_heap : keys
+      key_heap : key_perms
     ; protocol : user_cmd A
     ; msg_heap : queued_messages
       (* msg_heap : user_msg_heap ; *)
@@ -265,858 +317,1544 @@ Record universe (A B : Type) :=
       users       : honest_users A
     ; adversary   : user_data B
     ; all_ciphers : ciphers
+    ; all_keys    : keys
     }.
 
-Definition canonical_key (k1 k2 : key) :=
-  match Coq.Init.Nat.compare k1.(keyId) k2.(keyId) with
-  | Gt => k1
-  | Lt => k2
-  | Eq =>
-    match (k1.(keyUsage), k2.(keyUsage)) with
-    | (Signing, Encryption) => k1
-    | (Encryption, Signing) => k2
-    | _                     =>
-      match (k1.(keyType), k2.(keyType)) with
-      | (SymKey, _) => k1
-      | (_, SymKey) => k2
-      | (AsymKey b1, AsymKey b2) => if b1 then k1 else k2
-      end
-    end
-  end.
+(* Definition canonical_key (k1 k2 : key) := *)
+(*   match Coq.Init.Nat.compare k1.(keyId) k2.(keyId) with *)
+(*   | Gt => k1 *)
+(*   | Lt => k2 *)
+(*   | Eq => *)
+(*     match (k1.(keyUsage), k2.(keyUsage)) with *)
+(*     | (Signing, Encryption) => k1 *)
+(*     | (Encryption, Signing) => k2 *)
+(*     | _                     => *)
+(*       match (k1.(keyType), k2.(keyType)) with *)
+(*       | (SymKey, _) => k1 *)
+(*       | (_, SymKey) => k2 *)
+(*       | (AsymKey b1, AsymKey b2) => if b1 then k1 else k2 *)
+(*       end *)
+(*     end *)
+(*   end. *)
 
-Definition add_key (k_id : key_identifier) (k : key) (ks : keys) : keys :=
-  match ks $? k_id with
-  | None     => ks $+ (k_id, k)
-  | Some k'  => if   k ==kk k'
-               then ks
-               else ks $+ (k_id, canonical_key k k')
-               (* else if   keys_compatible k k' *)
-               (*      then if   k'.(keyType) ==kt AsymKey true (* private key do nothing *) *)
-               (*           then ks *)
-               (*           else ks $+ (k_id, k) *)
-               (*      (* Don't ever want to go down this branch *)
-               (*       * Implemented this way to make the fold work nice. *)
-               (*       *) *)
-               (*      else ks $+ (k_id, canonical_key k k') *)
-  end.
+Definition keys_good (ks : keys) : Prop :=
+  forall k_id k,
+    ks $? k_id = Some k
+    -> keyId k = k_id.
 
-Definition merge_keys (ks ks' : keys) : keys :=
-  fold add_key ks ks'.
+Definition key_perms_good (perms : key_perms) : Prop :=
+  forall k_id k,
+      perms $? k_id = Some k
+    -> key_ref k = k_id.
 
-Notation "m1 $k++ m2" := (merge_keys m2 m1) (at level 50, left associativity).
+Section KeyPermissions.
+  Variable perms : key_perms.
+  Variable gperms : key_perms_good perms.
 
-Fixpoint findKeys {t} (msg : message t) : keys :=
+  (* Definition greatest_permission (kp1 kp2 : key_permission) (eq_proof : kp1.(key_ref) = kp2.(key_ref)) : key_permission := *)
+  (*   match (kp1,kp2) with *)
+  (*   | (MkKeyPerm _ has_priv1, MkKeyPerm _ has_priv2) => MkKeyPerm kp1.(key_ref) (has_priv1 || has_priv2) *)
+  (*   end. *)
+
+  Definition greatest_permission (kp1 kp2 : key_permission) : key_permission :=
+    match (kp1,kp2) with
+    | (MkKeyPerm _ has_priv1, MkKeyPerm _ has_priv2) => MkKeyPerm kp1.(key_ref) (has_priv1 || has_priv2)
+    end.
+
+  Definition add_key_perm (kp : key_permission) : key_perms :=
+    match perms $? key_ref kp with
+    | None     => perms $+ (key_ref kp, kp)
+    | Some kp' => perms $+ (key_ref kp, greatest_permission kp kp')
+    end.
+
+  Lemma add_key_keeps_good :
+    forall kp perms',
+      perms' = add_key_perm kp
+      -> key_perms_good perms'.
+  Proof.
+    intros.
+    unfold key_perms_good in *; intros.
+    unfold add_key_perm in *.
+    destruct kp; subst; simpl in *.
+    cases (k_id ==n key_ref0); cases (perms $? key_ref0); subst; clean_map_lookups; auto.
+    unfold greatest_permission; destruct k0; simpl; trivial.
+  Qed.
+
+End KeyPermissions.
+
+Lemma greatest_permission_refl :
+  forall k,
+    greatest_permission k k = k.
+Proof.
+  unfold greatest_permission; intros; destruct k; simpl in *; rewrite orb_diag; trivial.
+Qed.
+
+Lemma greatest_permission_symm :
+  forall k1 k2,
+    key_ref k1 = key_ref k2
+    -> greatest_permission k1 k2 = greatest_permission k2 k1.
+Proof.
+  unfold greatest_permission; intros; destruct k1; destruct k2; simpl in *; subst; rewrite orb_comm; trivial.
+Qed.
+
+Definition add_key_perm_fold_fn (_ : key_identifier) (kp : key_permission) (perms : key_perms) : key_perms :=
+  add_key_perm perms kp.
+
+Definition merge_perms (ks ks' : key_perms) : key_perms :=
+  fold add_key_perm_fold_fn ks ks'.
+
+Notation "m1 $k++ m2" := (merge_perms m2 m1) (at level 50, left associativity).
+
+Lemma add_key_perm_fold_fn_proper :
+  Proper (eq  ==>  eq  ==>  eq  ==>  eq ) add_key_perm_fold_fn.
+Proof.
+  unfold Proper, respectful; intros; subst; trivial.
+Qed.
+
+Lemma add_key_perm_fold_fn_proper_Equal :
+  Proper (eq  ==>  eq  ==>  Equal  ==>  Equal ) add_key_perm_fold_fn.
+Proof.
+  unfold Proper, respectful; intros.
+  apply map_eq_Equal in H1; subst; unfold Equal; intros; trivial.
+Qed.
+
+Lemma add_key_perm_fold_fn_transpose' :
+  forall (k k' : nat) (e e' : key_permission) a,
+    k <> k'
+    -> Equal
+        match match a $? key_ref e' with
+              | Some kp' => a $+ (key_ref e', greatest_permission e' kp')
+              | None => a $+ (key_ref e', e')
+              end $? key_ref e with
+        | Some kp' =>
+          match a $? key_ref e' with
+          | Some kp'0 => a $+ (key_ref e', greatest_permission e' kp'0)
+          | None => a $+ (key_ref e', e')
+          end $+ (key_ref e, greatest_permission e kp')
+        | None => match a $? key_ref e' with
+                 | Some kp' => a $+ (key_ref e', greatest_permission e' kp')
+                 | None => a $+ (key_ref e', e')
+                 end $+ (key_ref e, e)
+        end
+        match match a $? key_ref e with
+              | Some kp' => a $+ (key_ref e, greatest_permission e kp')
+              | None => a $+ (key_ref e, e)
+              end $? key_ref e' with
+        | Some kp' =>
+          match a $? key_ref e with
+          | Some kp'0 => a $+ (key_ref e, greatest_permission e kp'0)
+          | None => a $+ (key_ref e, e)
+          end $+ (key_ref e', greatest_permission e' kp')
+        | None => match a $? key_ref e with
+                 | Some kp' => a $+ (key_ref e, greatest_permission e kp')
+                 | None => a $+ (key_ref e, e)
+                 end $+ (key_ref e', e')
+        end.
+Proof.
+  unfold Equal; intros.
+  destruct e; destruct e'; simpl.
+  cases (key_ref0 ==n key_ref1); subst; auto.
+  - cases (a $? key_ref1); clean_map_lookups; simpl.
+    + cases (y ==n key_ref1); subst; clean_map_lookups; auto.
+      unfold greatest_permission; destruct k0; simpl; auto.
+      rewrite !orb_assoc.
+      rewrite orb_comm with (b1:=has_private_access0).
+      trivial.
+    + unfold greatest_permission; simpl.
+      cases (y ==n key_ref1); subst; clean_map_lookups; auto.
+      rewrite orb_comm; trivial.
+  - cases (a $? key_ref0); cases (a $? key_ref1); clean_map_lookups;
+      rewrite Heq; rewrite Heq0; clean_map_lookups;
+        unfold greatest_permission; try destruct k0; try destruct k1; simpl;
+          cases (y ==n key_ref0); cases (y ==n key_ref1); subst; clean_map_lookups; try contradiction; auto.
+Qed.
+
+Lemma add_key_perm_fold_fn_transpose :
+  transpose_neqkey eq add_key_perm_fold_fn.
+Proof.
+  unfold transpose_neqkey, add_key_perm_fold_fn, add_key_perm; intros.
+  apply map_eq_Equal; eauto using add_key_perm_fold_fn_transpose'.
+Qed.
+
+Lemma add_key_perm_fold_fn_transpose_Equal :
+  transpose_neqkey Equal add_key_perm_fold_fn.
+Proof.
+  unfold transpose_neqkey, add_key_perm_fold_fn, add_key_perm; intros.
+  eauto using add_key_perm_fold_fn_transpose'.
+Qed.
+
+Hint Resolve add_key_perm_fold_fn_proper add_key_perm_fold_fn_transpose
+     add_key_perm_fold_fn_proper_Equal add_key_perm_fold_fn_transpose_Equal.
+
+(* Definition merge_keys (ks ks' : keys) : keys := *)
+(*   fold add_key ks ks'. *)
+
+(* Notation "m1 $k++ m2" := (merge_keys m2 m1) (at level 50, left associativity). *)
+
+Fixpoint findKeys {t} (msg : message t) : key_perms :=
   match msg with
   | Plaintext _        => $0
-  | KeyMessage k       => $0 $+ (keyId k, k)
+  | KeyMessage k       => $0 $+ (key_ref k, k)
   | MsgPair msg1 msg2  => (findKeys msg1) $k++ (findKeys msg2)
   | SignedCiphertext _ => $0
   | Signature m _      => findKeys m
   end.
 
-Definition findUserKeys {A} (us : user_list (user_data A)) : keys :=
+Definition findUserKeys {A} (us : user_list (user_data A)) : key_perms :=
   fold (fun u_id u ks => ks $k++ u.(key_heap)) us $0.
 
-Definition addUserKeys {A} (ks : keys) (u : user_data A) : user_data A :=
+Definition addUserKeys {A} (ks : key_perms) (u : user_data A) : user_data A :=
   {| key_heap := u.(key_heap) $k++ ks ; protocol := u.(protocol) ; msg_heap := u.(msg_heap) |}.
 
-Definition addUsersKeys {A} (us : user_list (user_data A)) (ks : keys) : user_list (user_data A) :=
+Definition addUsersKeys {A} (us : user_list (user_data A)) (ks : key_perms) : user_list (user_data A) :=
   map (addUserKeys ks) us.
 
-Definition adv_no_honest_keys (adv honest : keys) : Prop :=
+Definition adv_no_honest_keys (all_keys : keys) (honestk advk : key_perms) : Prop :=
   forall k_id,
-    match adv $? k_id with
-    | None => True
-    | Some (MkCryptoKey _ _ SymKey)            => honest $? k_id = None
-    | Some (MkCryptoKey kid kt (AsymKey true)) => honest $? k_id = None
-                                               \/ honest $? k_id = Some (MkCryptoKey kid kt (AsymKey false) )
-    | _ => False
+    match all_keys $? k_id with
+    | None                           => True
+    | Some (MkCryptoKey _ _ SymKey)  =>
+      match advk $? k_id with
+      | None   => True
+      | Some _ => False
+      end
+    | Some (MkCryptoKey _ _ AsymKey) => 
+      match advk $? k_id with
+      | None                     => True
+      | Some (MkKeyPerm _ false) => True
+      | Some (MkKeyPerm _ true)  => honest_key all_keys honestk k_id = false
+      end
     end.
-
-Ltac contra_map_lookup :=
-  match goal with
-  | [ H1 : ?ks $? ?k = Some _, H2 : ?ks $? ?k = None |- _ ] => rewrite H1 in H2; invert H2
-  | [ H : ?v1 <> ?v2, H1 : ?ks $? ?k = Some ?v1, H2 : ?ks $? ?k = Some ?v2 |- _ ] => rewrite H1 in H2; invert H2; contradiction
-  end.
-
-Ltac split_ands := 
-  repeat match goal with
-         | [ H : _ /\ _ |- _ ] => destruct H
-         end.
-  
-Ltac split_ors :=
-  repeat match goal with
-         | [ H : _ \/ _ |- _ ] => destruct H
-         end.
 
 Section KeyMergeTheorems.
+  Variable all_keys : keys.
+  Variable honestk advk : key_perms.
 
-  Lemma merge_keys_notation :
-    forall ks1 ks2,
-      fold add_key ks2 ks1 = ks1 $k++ ks2.
-    unfold merge_keys; trivial.
-  Qed.
+  Variable k_good      : keys_good all_keys.
+  Variable honest_good : key_perms_good honestk.
+  Variable adv_good    : key_perms_good advk.
 
-  Lemma safe_messages_have_no_bad_keys :
-    forall {t} (msg : message t) advk honestk msgk,
-      msg_needs_encryption honestk msg = false
-      -> adv_no_honest_keys advk honestk
-      -> msgk = findKeys msg
-      -> forall k_id k,
-            msgk $? k_id = Some k
-          -> honestk $? k_id = None
-          \/ (exists ku, k = MkCryptoKey k_id ku (AsymKey false))
-          \/ (exists ku, k = MkCryptoKey k_id ku (AsymKey true)  /\ honestk $? k_id = Some (MkCryptoKey k_id ku (AsymKey false))).
-  Proof.
-    induction msg; eauto; intros.
-    
-
-
-  Admitted.
-
-
-  Definition keys_good (ks : keys) : Prop :=
-    forall k_id k,
-      ks $? k_id = Some k
-      -> keyId k = k_id.
-
-  Definition key_heaps_compatible (ks1 ks2 : keys) :=
-      keys_good ks1
-    /\ keys_good ks2
-    /\ (forall k_id k k', ks1 $? k_id = Some k -> ks2 $? k_id = Some k' -> keys_compatible k k' = true).
-
-  Lemma canonical_key_one_other :
-    forall k1 k2,
-        canonical_key k1 k2 = k1
-      \/ canonical_key k1 k2 = k2.
-  Proof.
-    intros; unfold canonical_key.
-    destruct k1; destruct k2; simpl.
-    cases (keyId0 ?= keyId1);
-      cases keyUsage0; cases keyUsage1;
-        cases keyType0; cases keyType1; eauto;
-          try rewrite Nat.compare_refl; simpl; eauto;
-            cases has_private_access; cases has_private_access0; eauto.
-  Qed.
-
-  Lemma canonical_key_refl :
-    forall k, canonical_key k k = k.
-  Proof.
-    unfold canonical_key; intros; simpl.
-    rewrite Nat.compare_refl.
-    cases (keyUsage k); cases (keyType k); simpl; eauto; cases has_private_access; eauto.
-  Qed.
-
-  Lemma canonical_key_sym :
-    forall k1 k2,
-      canonical_key k1 k2 = canonical_key k2 k1.
-  Proof.
-    intros; destruct k1; destruct k2; unfold canonical_key; simpl.
-    cases (keyId0 ?= keyId1).
-    - apply Nat.compare_eq in Heq; subst.
-      rewrite Nat.compare_refl.
-      cases keyUsage0; cases keyUsage1; cases keyType0; cases keyType1; eauto.
-      cases has_private_access; cases has_private_access0; eauto.
-      cases has_private_access; cases has_private_access0; eauto.
-
-    - rewrite Nat.compare_antisym; rewrite Heq; simpl; auto.
-    - rewrite Nat.compare_antisym; rewrite Heq; simpl; auto.
-  Qed.
-
-  Lemma canonical_key_assoc :
-    forall k1 k2 k3,
-      canonical_key k1 (canonical_key k2 k3) = canonical_key (canonical_key k1 k2) k3.
-  Proof.
-    intros; destruct k1; destruct k2; destruct k3; unfold canonical_key; simpl.
-
-    cases (keyId0 ?= keyId1); cases (keyId1 ?= keyId2).
-    - apply Nat.compare_eq in Heq; apply Nat.compare_eq in Heq0; subst. simpl.
-      cases keyUsage0; cases keyUsage1; cases keyUsage2;
-        cases keyType0; cases keyType1; cases keyType2;
-          simpl; eauto;
-            try rewrite Nat.compare_refl; eauto;
-              cases has_private_access; cases has_private_access0; try cases has_private_access1; simpl;
-                try rewrite Nat.compare_refl; eauto.
-
-    - apply Nat.compare_eq in Heq; subst; simpl.
-      rewrite Heq0; simpl.
-      cases keyUsage0; cases keyUsage1; cases keyUsage2;
-        cases keyType0; cases keyType1; cases keyType2;
-          simpl; eauto; try rewrite Heq0; simpl; eauto;
-            cases has_private_access; cases has_private_access0; try cases has_private_access1; simpl;
-              rewrite Heq0; simpl; eauto.
-
-    - apply Nat.compare_eq in Heq; subst; simpl.
-      rewrite Nat.compare_refl.
-      cases keyUsage0; cases keyUsage1; cases keyUsage2;
-        cases keyType0; cases keyType1; cases keyType2;
-          simpl; eauto; try rewrite Heq0; simpl; eauto;
-            cases has_private_access; cases has_private_access0; try cases has_private_access1; simpl;
-              rewrite Heq0; simpl; eauto.
-
-    - apply Nat.compare_eq in Heq0; subst; simpl.
-      rewrite Nat.compare_refl; simpl.
-      cases keyUsage0; cases keyUsage1; cases keyUsage2;
-        cases keyType0; cases keyType1; cases keyType2;
-          simpl; eauto; try rewrite Heq; simpl; eauto;
-            cases has_private_access; cases has_private_access0; try cases has_private_access1; simpl;
-              rewrite Heq; simpl; eauto.
-
-    - simpl. rewrite Heq0.
-      pose proof Heq as lt1; pose proof Heq0 as lt2.
-      apply nat_compare_lt in lt1; apply nat_compare_lt in lt2.
-      pose proof (Nat.lt_trans _ _ _ lt1 lt2). apply nat_compare_lt in H.
-      rewrite H; eauto.
-
-    - simpl; rewrite Heq; rewrite Heq0; eauto.
-
-    - apply Nat.compare_eq in Heq0; subst; simpl.
-      rewrite Heq; simpl.
-      cases keyUsage0; cases keyUsage1; cases keyUsage2;
-        cases keyType0; cases keyType1; cases keyType2;
-          simpl; eauto; try rewrite Heq; simpl; eauto;
-            cases has_private_access; cases has_private_access0; try cases has_private_access1; simpl;
-              rewrite Heq; simpl; eauto.
-
-    - simpl. cases (keyId0 ?= keyId2); simpl; eauto.
-    - simpl. rewrite Heq.
-      pose proof Heq as gt1; pose proof Heq0 as gt2.
-      apply nat_compare_gt in gt1; apply nat_compare_gt in gt2.
-
-      pose proof (gt_trans _ _ _ gt1 gt2); apply nat_compare_gt in H.
-      rewrite H; simpl; eauto.
-  Qed.
-
-  Lemma merge_keys_fold_fn_proper :
-      Morphisms.Proper
-        (Morphisms.respectful eq (Morphisms.respectful eq (Morphisms.respectful eq eq)))
-        add_key.
-  Proof.
-    unfold Morphisms.Proper, Morphisms.respectful; intros; simpl; subst; trivial.
-  Qed.
-
-  Lemma merge_keys_fold_fn_proper_flip :
-      Morphisms.Proper
-        (Morphisms.respectful eq (Morphisms.respectful eq (Morphisms.respectful (Basics.flip eq) (Basics.flip eq))))
-        add_key.
-  Proof.
-    unfold Morphisms.Proper, Morphisms.respectful; intros; simpl; unfold Basics.flip in *; subst; trivial.
-  Qed.
-
-  Lemma merge_keys_fold_fn_proper_Equal :
-    Morphisms.Proper
-      (Morphisms.respectful eq (Morphisms.respectful eq (Morphisms.respectful Equal Equal)))
-      add_key.
-  Proof.
-    unfold Morphisms.Proper, Morphisms.respectful; intros; simpl; subst.
-    apply map_eq_Equal in H1; subst.
-    apply Equal_refl.
-  Qed.
-
-  Lemma merge_keys_transpose :
-    transpose_neqkey eq add_key.
-  Proof.
-    unfold transpose_neqkey; intros.
-    unfold add_key; simpl.
-    case_eq (a $? k); case_eq (a $? k'); intros; subst; simpl.
-
-    Ltac work1 :=
-      match goal with
-      | [ H : ?x <> ?x |- _ ] => contradiction
-      | [ H1 : ?x <> ?y, H2 : ?x = ?y |- _ ] => contradiction
-      | [ H : ?a $? ?k  = _ |- context [?a $? ?k]  ] => rewrite H
-      | [ H : ?a $? ?k' = _ |- context [?a $? ?k'] ] => rewrite H
-      | [ |- context[ ?k1 ==kk ?k2 ] ] => case (k1 ==kk k2); intros; subst
-      | [ H : keys_compatible ?k1 ?k2 = _ |- context [ keys_compatible ?k1 ?k2 ]] => rewrite H
-      | [ |- context [ keys_compatible ?k1 ?k2 ]] => case_eq (keys_compatible k1 k2); intros
-      | [ H : keyType ?k = _ |- context [ keyType ?k ==kt ?kt ]] => rewrite H
-      | [ |- context [ keyType ?k ==kt ?kt ]] => case (keyType k ==kt kt); intros
-      | [ |- context [ _ $+ (?k1, _) $? ?k1 ]] => rewrite add_eq_o by (trivial || auto)
-      | [ |- context [ _ $+ (?k1, _) $? ?k2 ]] => rewrite add_neq_o by auto
-      | [ |- context [ _ $- ?k1 $? ?k2 ]] => rewrite remove_neq_o by auto
-      end.
-
-    Ltac maps_equal :=
-      repeat match goal with
-             | [ |- context[find ?k (add ?k _ _) ] ]  => rewrite add_eq_o by auto
-             | [ |- context[find ?k (add ?k' _ _) ] ] => rewrite add_neq_o by auto
-             | [ |- context[find ?k (remove ?k _) ] ]  => rewrite remove_eq_o by auto
-             | [ |- context[find ?k (remove ?k' _) ] ] => rewrite remove_neq_o by auto
-             | [ |- _ $+ (?k1,_) $? ?k = _ ] => case (k1 ==n k); intros; subst
-             | [ |- _ $- ?k1     $? ?k = _ ] => case (k1 ==n k); intros; subst
-             | [ |- add _ _ _ = _ ] => apply map_eq_Equal; unfold Equal; intros ?y
-             end.
-
-    repeat work1; eauto;
-      apply map_eq_Equal; unfold Equal; intros;
-        maps_equal; auto.
-    
-    repeat work1; eauto;
-      apply map_eq_Equal; unfold Equal; intros;
-        maps_equal; auto.
-
-    repeat work1; eauto;
-      apply map_eq_Equal; unfold Equal; intros;
-        maps_equal; auto.
-
-    repeat work1; eauto;
-      apply map_eq_Equal; unfold Equal; intros;
-        maps_equal; auto.
-
-  Qed.
-
-  Lemma merge_keys_transpose_flip :
-    transpose_neqkey (Basics.flip eq) add_key.
-  Proof.
-    unfold transpose_neqkey, Basics.flip; intros.
-    apply merge_keys_transpose; auto.
-  Qed.
-
-  Lemma eq_Equal :
-    forall {V} (m m' : NatMap.t V),
-      m = m'
-      -> Equal m m'.
-    intros; subst; apply Equal_refl.
-  Qed.
-
-  Lemma merge_keys_transpose_Equal :
-    transpose_neqkey Equal add_key.
-  Proof.
-    unfold transpose_neqkey; intros.
-    apply eq_Equal.
-    apply merge_keys_transpose; auto.
-  Qed.
-
-  Hint Resolve merge_keys_fold_fn_proper merge_keys_fold_fn_proper_flip merge_keys_fold_fn_proper_Equal
-               merge_keys_transpose merge_keys_transpose_flip merge_keys_transpose_Equal.
-
-
-  Ltac clean_map_lookups1 :=
-    match goal with
-    | [ H : Some _ = None   |- _ ] => invert H
-    | [ H : None = Some _   |- _ ] => invert H
-    | [ H : Some _ = Some _ |- _ ] => invert H
-    | [ H : $0 $? _ = Some _ |- _ ] => invert H
-    | [ H : _ $+ (?k,_) $? ?k = _ |- _ ] => rewrite add_eq_o in H by trivial
-    | [ H : _ $+ (?k1,_) $? ?k2 = _ |- _ ] => rewrite add_neq_o in H by auto
-    | [ |- context[_ $+ (?k,_) $? ?k] ] => rewrite add_eq_o by trivial
-    | [ |- context[_ $+ (?k1,_) $? ?k2] ] => rewrite add_neq_o by auto
-    | [ H : ~ In _ _ |- _ ] => rewrite not_find_in_iff in H
-    end.
+  Hint Resolve empty_Empty.
 
   Ltac progress_fold_add1 :=
     match goal with
-    | [ H : fold add_key (_ $+ (_,_)) _ $? _ = _ |- _ ] => rewrite fold_add in H
-    | [ |- context[  fold add_key (_ $+ (_,_)) _ ] ] => rewrite fold_add
+    | [ H : fold add_key_perm_fold_fn (_ $+ (_,_)) _ $? _ = _ |- _ ] => rewrite fold_add in H
+    | [ H : _ $k++ (_ $+ (_,_)) $? _ = _ |- _ ] => unfold merge_perms in H; rewrite fold_add in H
+    | [ |- context[ fold add_key_perm_fold_fn (_ $+ (_,_)) _ ] ] => rewrite fold_add
+    | [ |- context[ _ $k++ (_ $+ (_,_))] ] => unfold merge_perms; rewrite fold_add
     end.
 
-  Ltac clean_map_lookups :=
-    (repeat clean_map_lookups1);
-    try discriminate;
-    try contra_map_lookup.
+  Lemma merge_perms_notation :
+    forall ks1 ks2,
+      fold add_key_perm_fold_fn ks2 ks1 = ks1 $k++ ks2.
+    unfold merge_perms; trivial.
+  Qed.
 
-  Hint Resolve empty_Empty.
-  Hint Extern 1 (~ In _ _) => rewrite not_find_in_iff.
-
-  Lemma merge_keys_left_identity :
-    forall ks,
-      $0 $k++ ks = ks.
+  Lemma key_perms_good_add :
+    forall ks k_id kp,
+      key_perms_good (ks $+ (k_id, kp))
+      -> ~ In k_id ks
+      -> key_ref kp = k_id
+      /\ key_perms_good ks.
   Proof.
-    unfold merge_keys.
-    induction ks using P.map_induction_bis; intros.
+    intros.
+    unfold key_perms_good in H.
+    split.
+    - apply H; clean_map_lookups; trivial.
+    - unfold key_perms_good; intros; cases (k_id ==n k_id0); subst; clean_map_lookups;
+        eapply H; clean_map_lookups; auto.
+  Qed.
 
+  Lemma empty_key_perms_good :
+    key_perms_good $0.
+  Proof.
+    unfold key_perms_good; intros; invert H.
+  Qed.
+
+  Hint Resolve empty_key_perms_good.
+
+  Lemma merge_perms_left_identity :
+    forall ks,
+        key_perms_good ks
+      -> $0 $k++ ks = ks.
+  Proof.
+    induction ks using P.map_induction_bis; intros.
     - apply map_eq_Equal in H; subst; auto.
     - apply fold_Empty; eauto.
-    - rewrite fold_add; clean_map_lookups; eauto.
-      rewrite IHks; clear IHks.
-      unfold add_key; rewrite H; eauto.
+    - unfold merge_perms.
+      rewrite fold_add; auto.
+      apply key_perms_good_add in H0; auto; split_ands.
+
+      rewrite merge_perms_notation.
+      unfold add_key_perm_fold_fn, add_key_perm.
+      rewrite IHks; auto.
+
+      case_eq (ks $? key_ref e); intros; subst; clean_map_lookups; trivial.
   Qed.
-    
+
   Lemma merge_keys_right_identity :
     forall ks,
       ks $k++ $0 = ks.
   Proof.
-    unfold merge_keys; intros; rewrite fold_Empty; eauto.
+    unfold merge_perms; intros; rewrite fold_Empty; eauto.
   Qed.
 
-  Hint Resolve merge_keys_left_identity merge_keys_right_identity.
-
-  Lemma merge_keys_adds_no_new_keys :
-    forall ks2 k ks1,
-        ks1 $? k = None
-      -> ks2 $? k = None
-      -> (ks1 $k++ ks2) $? k = None.
+  Lemma key_perms_merge_still_good :
+    forall ks2 ks1,
+      key_perms_good ks1
+      -> key_perms_good ks2
+      -> key_perms_good (ks1 $k++ ks2).
   Proof.
     induction ks2 using P.map_induction_bis; intros.
     - apply map_eq_Equal in H; subst; auto.
     - rewrite merge_keys_right_identity; auto.
-    - unfold merge_keys; rewrite fold_add; auto.
-      case (x ==n k); intros; subst; clean_map_lookups.
-      + rewrite merge_keys_notation; unfold add_key.
-        cases (ks1 $k++ ks2 $? x); clean_map_lookups; eauto.
-        cases (e ==kk k0); subst; eauto.
-        clean_map_lookups. eapply IHks2; auto.
+    - apply key_perms_good_add in H1; split_ands; subst; auto.
+      progress_fold_add1; auto.
+      rewrite merge_perms_notation.
+      unfold add_key_perm_fold_fn, add_key_perm; simpl.
+      cases (ks1 $k++ ks2 $? key_ref e).
+      + unfold key_perms_good; intros.
+        specialize (IHks2 _ H0 H2).
+        assert (ks1 $k++ ks2 $? key_ref e = Some k) as EQ by assumption; apply IHks2 in EQ.
+        cases (key_ref e ==n k_id); subst; clean_map_lookups; auto.
+        unfold greatest_permission; destruct e; destruct k; auto.
+      + unfold key_perms_good; intros.
+        cases (key_ref e ==n k_id); subst; clean_map_lookups; auto.
+        specialize (IHks2 _ H0 H2); auto.
   Qed.
 
-  Lemma merge_keys_no_disappear_keys :
+  Lemma merge_perms_adds_no_new_perms :
     forall ks2 k ks1,
-      (ks1 $k++ ks2) $? k = None
-    -> ks1 $? k = None
-    /\ ks2 $? k = None.
+        ks1 $? k = None
+      -> ks2 $? k = None
+      -> key_perms_good ks2
+      -> (ks1 $k++ ks2) $? k = None.
+  Proof.
+    induction ks2 using P.map_induction_bis; intros; auto.
+    - apply map_eq_Equal in H; subst; auto.
+    - progress_fold_add1; auto.
+      rewrite merge_perms_notation.
+      unfold add_key_perm_fold_fn, add_key_perm.
+      apply key_perms_good_add in H2; split_ands; subst; auto.
+      case (key_ref e ==n k); intros; subst; clean_map_lookups.
+      cases (ks1 $k++ ks2 $? key_ref e); clean_map_lookups; auto.
+  Qed.
+
+  Lemma merge_perms_came_from_somewhere1 :
+    forall ks2 ks1 k v,
+        ks1 $k++ ks2 $? k = Some v
+      -> key_perms_good ks1
+      -> key_perms_good ks2
+      -> ks2 $? k = None
+      -> ks1 $? k = Some v.
   Proof.
     induction ks2 using P.map_induction_bis; intros.
-    - apply map_eq_Equal in H; subst; auto.
-    - rewrite merge_keys_right_identity in H; eauto.
-    - unfold merge_keys in H0. progress_fold_add1; auto.
-      rewrite merge_keys_notation in *; clean_map_lookups.
-      unfold add_key in H0.
-      cases (ks1 $k++ ks2 $? x); clean_map_lookups;
-        [cases (e ==kk k0); subst | ];
-          case (x ==n k); intros; subst; clean_map_lookups; eauto.
+
+    - apply map_eq_Equal in H; subst; eauto.
+    - rewrite merge_keys_right_identity in H; auto.
+    - case (x ==n k); intros; subst; clean_map_lookups.
+      apply key_perms_good_add in H2; split_ands; subst; auto.
+      progress_fold_add1; auto.
+      rewrite merge_perms_notation in H0.
+      unfold add_key_perm_fold_fn, add_key_perm in H0.
+      cases (ks1 $k++ ks2 $? key_ref e); clean_map_lookups; eauto.
   Qed.
 
-  Hint Resolve merge_keys_adds_no_new_keys merge_keys_no_disappear_keys.
+  Lemma merge_perms_came_from_somewhere2 :
+    forall ks2 ks1 k v,
+        ks1 $k++ ks2 $? k = Some v
+      -> key_perms_good ks1
+      -> key_perms_good ks2
+      -> ks1 $? k = None
+      -> ks2 $? k = Some v.
+  Proof.
+    induction ks2 using P.map_induction_bis; intros.
+    - apply map_eq_Equal in H; subst; eauto.
+    - rewrite merge_keys_right_identity in H; clean_map_lookups.
+    - apply key_perms_good_add in H2; split_ands; subst; auto.
+      case (k ==n key_ref e); intros; subst; clean_map_lookups.
+      + progress_fold_add1; auto.
+        rewrite merge_perms_notation in H0.
+        unfold add_key_perm_fold_fn, add_key_perm in H0.
+        assert (ks1 $k++ ks2 $? key_ref e = None) by eauto using merge_perms_adds_no_new_perms.
+        rewrite H2 in H0; clean_map_lookups; trivial.
+      + progress_fold_add1; auto.
+        rewrite merge_perms_notation in H0.
+        unfold add_key_perm_fold_fn, add_key_perm in H0.
+        cases (ks1 $k++ ks2 $? key_ref e); clean_map_lookups; eauto.
+  Qed.
 
-  Lemma merge_keys_adds_ks1 :
+  Lemma merge_perms_adds_ks1 :
     forall ks2 ks1 k v ks,
         ks1 $? k = Some v
       -> ks2 $? k = None
+      -> key_perms_good ks1                 
+      -> key_perms_good ks2
       -> ks = ks1 $k++ ks2
       -> ks $? k = Some v.
   Proof.
-    unfold merge_keys.
+    unfold merge_perms.
     induction ks2 using P.map_induction_bis; intros.
 
     - apply map_eq_Equal in H; subst; eauto.
     - subst; rewrite fold_Empty; eauto.
     - case (x ==n k); intros; subst; clean_map_lookups; eauto.
-      rewrite fold_add; eauto.
-      rewrite merge_keys_notation.
-      unfold add_key.
-      cases ( ks1 $k++ ks2 $? x ); clean_map_lookups; eauto.
-      cases ( e ==kk k0 ); eauto.
-      clean_map_lookups; eauto.
+      progress_fold_add1; auto.
+      rewrite merge_perms_notation.
+      unfold add_key_perm_fold_fn, add_key_perm.
+      apply key_perms_good_add in H3; split_ands; subst; auto.
+      cases ( ks1 $k++ ks2 $? key_ref e ); clean_map_lookups; eauto.
   Qed.
 
-  Lemma merge_keys_adds_ks2 :
+  Lemma merge_perms_adds_ks2 :
     forall ks2 ks1 k v ks,
         ks1 $? k = None
       -> ks2 $? k = Some v
+      -> key_perms_good ks1                 
+      -> key_perms_good ks2
       -> ks = ks1 $k++ ks2
       -> ks $? k = Some v.
   Proof.
-    unfold merge_keys.
+    unfold merge_perms.
     induction ks2 using P.map_induction_bis; intros.
-
     - apply map_eq_Equal in H; subst; eauto.
     - invert H0.
-    - subst.
-      case (x ==n k); intros; subst; clean_map_lookups; eauto.
-      + rewrite fold_add; auto.
-        rewrite merge_keys_notation.
-        unfold add_key.
-        pose proof merge_keys_adds_no_new_keys.
-        cases ( ks1 $k++ ks2 $? k); clean_map_lookups; eauto.
-        cases ( v ==kk k0 ); subst; clean_map_lookups; eauto.
-        specialize (H1 _ _ _ H0 H); contra_map_lookup.
-
-      + rewrite fold_add; auto.
-        rewrite merge_keys_notation.
-        unfold add_key.
-        cases ( ks1 $k++ ks2 $? x); clean_map_lookups; eauto.
-        cases ( e ==kk k0 ); eauto.
-        clean_map_lookups; eauto.
+    - apply key_perms_good_add in H3; auto; split_ands; subst.
+      progress_fold_add1; auto.
+      rewrite merge_perms_notation.
+      unfold add_key_perm_fold_fn, add_key_perm.
+      cases (k ==n key_ref e); subst; clean_map_lookups.
+      + assert (ks1 $k++ ks2 $? key_ref v = None) as RW by eauto using merge_perms_adds_no_new_perms;
+          rewrite RW; clean_map_lookups; trivial.
+      + cases ( ks1 $k++ ks2 $? key_ref e); clean_map_lookups; eauto.
   Qed.
 
-  Hint Resolve merge_keys_adds_ks1 merge_keys_adds_ks2.
-
-  Lemma merge_keys_came_from_somewhere1 :
-    forall ks2 ks1 k v,
-        ks1 $k++ ks2 $? k = Some v
-      -> ks2 $? k = None
-      -> ks1 $? k = Some v.
+  Lemma merge_perms_split :
+    forall ks2 ks1 k,
+      ks1 $k++ ks2 $? key_ref k = Some k
+      -> key_perms_good ks1
+      -> key_perms_good ks2
+      -> ks1 $? key_ref k = Some k
+      \/ ks2 $? key_ref k = Some k.
   Proof.
-    unfold merge_keys.
     induction ks2 using P.map_induction_bis; intros.
-
-    - apply map_eq_Equal in H; subst; eauto.
-    - rewrite fold_Empty in H; auto.
-
-    - case (x ==n k); intros; subst; clean_map_lookups.
-      + progress_fold_add1; auto.
-        rewrite merge_keys_notation in H0; unfold add_key at 1 in H0.
-
-        cases (ks1 $k++ ks2 $? x); clean_map_lookups; eauto.
-        cases ( e ==kk k0 ); subst; clean_map_lookups; eauto.
-  Qed.
-
-  Lemma merge_keys_came_from_somewhere2 :
-    forall ks2 ks1 k v,
-        ks1 $k++ ks2 $? k = Some v
-      -> ks1 $? k = None
-      -> ks2 $? k = Some v.
-  Proof.
-    unfold merge_keys.
-    induction ks2 using P.map_induction_bis; intros.
-
-    - apply map_eq_Equal in H; subst; eauto.
-    - rewrite fold_Empty in H; clean_map_lookups; auto.
-
-    - case (x ==n k); intros; subst; clean_map_lookups; progress_fold_add1; auto.
-      * pose proof (merge_keys_adds_no_new_keys _ _ _ H1 H).
-        rewrite merge_keys_notation in H0; unfold add_key in H0; auto.
-        cases (ks1 $k++ ks2 $? k); clean_map_lookups; eauto.
-
-      * rewrite merge_keys_notation in H0; unfold add_key in H0; auto.
-        cases (ks1 $k++ ks2 $? x); clean_map_lookups; eauto.
-        cases ( e ==kk k0 ); subst; clean_map_lookups; eauto.
-  Qed.
-
-  Hint Resolve merge_keys_came_from_somewhere1 merge_keys_came_from_somewhere2.
-
-  Lemma merge_keys_split :
-    forall ks2 k_id k ks1,
-      ks1 $k++ ks2 $? k_id = Some k
-      -> (ks1 $? k_id = None /\ ks2 $? k_id = Some k)
-      \/ (ks1 $? k_id = Some k /\ ks2 $? k_id = None)
-      \/ exists k1 k2, ks1 $? k_id = Some k1 /\ ks2 $? k_id = Some k2 /\ k = canonical_key k1 k2.
-  Proof.
-    unfold merge_keys.
-    induction ks2 using P.map_induction_bis; intros.
-    - apply map_eq_Equal in H; subst; eauto.
-    - rewrite merge_keys_right_identity in H. intuition idtac.
-    - rewrite fold_add in H0; auto.
-      rewrite merge_keys_notation in H0; unfold add_key in H0; auto.
-      case (x ==n k_id); intros; subst; clean_map_lookups.
-      + cases (ks1 $k++ ks2 $? k_id); intros; simpl.
-        * cases (e ==kk k0); subst.
-          ** rewrite Heq in H0; invert H0. eapply merge_keys_came_from_somewhere1 in Heq; auto.
-             right; right. do 2 eexists; intuition eauto. rewrite canonical_key_refl; trivial.
-          ** clean_map_lookups; eapply merge_keys_came_from_somewhere1 in Heq; auto.
-             right; right; do 2 eexists; intuition eauto. rewrite canonical_key_sym; trivial.
-
-        * clean_map_lookups; eauto. eapply merge_keys_no_disappear_keys in Heq; invert Heq.
+    - apply map_eq_Equal in H; subst; auto.
+    - rewrite merge_keys_right_identity in H; auto.
+    - apply key_perms_good_add in H2; auto; split_ands; subst; clean_map_lookups.
+      cases (key_ref e ==n key_ref k).
+      + progress_fold_add1; auto. rewrite merge_perms_notation in H0.
+        unfold add_key_perm_fold_fn, add_key_perm in H0.
+        case_eq (ks1 $k++ ks2 $? key_ref e); intros; rewrite H2 in H0; clean_map_lookups; eauto.
+        rewrite e0 in H0; clean_map_lookups.
+        rewrite <- e0; clean_map_lookups.
+        unfold greatest_permission in *; destruct e; destruct k0; simpl in *.
+        cases has_private_access0; cases has_private_access1; simpl; auto.
+        pose proof (key_perms_merge_still_good H1 H3) as MERGE_GOOD.
+        assert (ks1 $k++ ks2 $? key_ref0 = Some {| key_ref := key_ref1; has_private_access := true |}) as EQ by assumption.
+        apply MERGE_GOOD in EQ; simpl in EQ; subst.
+        remember ({| key_ref := key_ref0; has_private_access := true |}) as k0.
+        assert (ks1 $k++ ks2 $? key_ref k0 = Some k0) as IND by (subst; simpl; auto).
+        specialize (IHks2 _ _ IND H1 H3); split_ors; subst.
           intuition idtac.
-      + cases (ks1 $k++ ks2 $? x); clean_map_lookups; eauto.
-        cases (e ==kk k0); auto.
-        cases (x ==n k_id); clean_map_lookups; auto.
+          simpl in *; contra_map_lookup.
+          rewrite add_eq_o by auto. rewrite add_eq_o in H0 by auto; intuition idtac.
+      + clean_map_lookups. apply IHks2; eauto.
+        progress_fold_add1; auto. rewrite merge_perms_notation in H0.
+        unfold add_key_perm_fold_fn, add_key_perm in H0; simpl in H0.
+        cases (ks1 $k++ ks2 $? key_ref e); clean_map_lookups; auto.
   Qed.
 
-  Lemma merge_keys_canonicalizes :
-    forall ks2 k_id k k1 k2 ks1,
-        ks1 $k++ ks2 $? k_id = Some k
-      -> ks1 $? k_id = Some k1
-      -> ks2 $? k_id = Some k2
-      -> k = canonical_key k1 k2.
+  Lemma key_perms_good_add_good_perm :
+    forall ks k,
+      key_perms_good ks
+      -> key_perms_good (ks $+ (key_ref k, k)).
   Proof.
-    unfold merge_keys.
-    induction ks2 using P.map_induction_bis; intros.
-    - apply map_eq_Equal in H; subst; eauto.
-    - invert H1.
-
-    - rewrite fold_add in H0; auto.
-      rewrite merge_keys_notation in H0; unfold add_key in H0; auto.
-      case (x ==n k_id); intros; subst; clean_map_lookups.
-      + cases (ks1 $k++ ks2 $? k_id); intros; simpl.
-        * cases (k2 ==kk k0); subst; eauto.
-          ** rewrite Heq in H0; invert H0. eapply merge_keys_came_from_somewhere1 in Heq; auto. rewrite Heq in H1; invert H1. rewrite canonical_key_refl; trivial.
-          ** clean_map_lookups. eapply merge_keys_came_from_somewhere1 in Heq; auto. rewrite Heq in H1; invert H1. rewrite canonical_key_sym; trivial.
-
-        * clean_map_lookups. eapply merge_keys_no_disappear_keys in Heq; destruct Heq; contra_map_lookup.
-
-      + cases (ks1 $k++ ks2 $? x); clean_map_lookups; eauto.
-        cases (e ==kk k0); subst; clean_map_lookups; eauto.
+    unfold key_perms_good; intros.
+    cases (key_ref k ==n k_id); subst; clean_map_lookups; auto.
   Qed.
 
-  Lemma merge_keys_canonicalizes' :
-    forall ks2 k_id k k1 k2 ks1,
-        ks1 $? k_id = Some k1
-      -> ks2 $? k_id = Some k2
-      -> k = canonical_key k1 k2
-      -> ks1 $k++ ks2 $? k_id = Some k.
+  Hint Resolve key_perms_good_add_good_perm.
+
+  Lemma merge_perms_no_disappear_perms :
+    forall ks2 k ks1,
+      (ks1 $k++ ks2) $? k = None
+    -> key_perms_good ks1
+    -> key_perms_good ks2
+    -> ks1 $? k = None
+    /\ ks2 $? k = None.
   Proof.
-    unfold merge_keys.
-    induction ks2 using P.map_induction_bis; intros.
-    - apply map_eq_Equal in H; subst; eauto.
-    - invert H0.
-
-    - rewrite fold_add; auto.
-      rewrite merge_keys_notation; unfold add_key.
-      cases (ks1 $k++ ks2 $? x); case (x ==n k_id); intros; subst; clean_map_lookups.
-      + cases (k2 ==kk k0); subst.
-        * eapply (merge_keys_came_from_somewhere1) in Heq; auto. rewrite Heq in H0; invert H0. rewrite canonical_key_refl. eapply merge_keys_adds_ks1; eauto.
-        * eapply (merge_keys_came_from_somewhere1) in Heq; auto. rewrite Heq in H0; invert H0. rewrite canonical_key_sym. clean_map_lookups; trivial.
-      + cases (e ==kk k0); subst; clean_map_lookups; eauto.
-      + eapply merge_keys_no_disappear_keys in Heq; invert Heq; contra_map_lookup.
-      + eapply IHks2; eauto.
+    induction ks2 using P.map_induction_bis; intros; auto.
+    - apply map_eq_Equal in H; subst; auto.
+    - progress_fold_add1; auto.
+      rewrite merge_perms_notation in *; clean_map_lookups.
+      unfold add_key_perm_fold_fn, add_key_perm in H0.
+      apply key_perms_good_add in H2; split_ands; subst; auto.
+      cases (ks1 $k++ ks2 $? key_ref e); clean_map_lookups;
+        cases (key_ref e ==n k); subst; clean_map_lookups; auto.
   Qed.
 
-  Lemma add_key_results :
-    forall k v ks ks',
-      ks' = add_key k v ks
-      -> ks' = ks
-      \/ ks' = ks $+ (k,v)
-      \/ exists k', ks' = ks $+ (k, canonical_key v k').
+
+  Lemma merge_keys_add_l_pull :
+    forall ks2 ks1 k,
+      ks2 $? key_ref k = None
+      -> key_perms_good ks1
+      -> key_perms_good ks2
+      -> ks1 $k++ ks2 $+ (key_ref k, k) = (ks1 $+ (key_ref k, k)) $k++ ks2.
   Proof.
-    unfold add_key; intros.
-    cases (ks $? k); auto.
-    cases (v ==kk k0); auto.
-    intuition eauto.
+    induction ks2 using P.map_induction_bis; auto; intros.
+    - apply map_eq_Equal in H; subst; auto.
+    - apply key_perms_good_add in H2; split_ands; subst; auto.
+      cases (key_ref e ==n key_ref k); try rewrite e0 in *; clean_map_lookups; auto.
+      unfold merge_perms at 2. rewrite fold_add; auto.
+      unfold add_key_perm_fold_fn at 1.
+      unfold add_key_perm.
+      rewrite merge_perms_notation with (ks1:=ks1 $+ (key_ref k, k)).
+      cases ( (ks1 $+ (key_ref k, k)) $k++ ks2 $? key_ref e); subst; clean_map_lookups; auto.
+      + rewrite <- IHks2; clean_map_lookups; auto.
+        unfold merge_perms at 1; rewrite fold_add; auto.
+        rewrite merge_perms_notation.
+        unfold add_key_perm_fold_fn, add_key_perm.
+        apply merge_perms_came_from_somewhere1 in Heq; auto.
+        clean_map_lookups.
+        assert (ks1 $k++ ks2 $? key_ref e = Some k0) as RW by (eauto using merge_perms_adds_ks1);
+          rewrite RW; clear RW.
+        apply map_eq_Equal; unfold Equal; intros.
+        cases (y ==n key_ref e); cases (y ==n key_ref k); subst; clean_map_lookups; trivial.
+      + rewrite <- IHks2; clean_map_lookups; auto.
+        unfold merge_perms at 1; rewrite fold_add; auto.
+        rewrite merge_perms_notation.
+        unfold add_key_perm_fold_fn, add_key_perm.
+        apply merge_perms_no_disappear_perms in Heq; auto; split_ands; clean_map_lookups.
+        assert (ks1 $k++ ks2 $? key_ref e = None) as RW by (eauto using merge_perms_adds_no_new_perms);
+          rewrite RW; clear RW.
+        apply map_eq_Equal; unfold Equal; intros.
+        cases (y ==n key_ref e); cases (y ==n key_ref k); subst; clean_map_lookups; trivial.
   Qed.
 
-  Lemma keys_compatible_reflexive :
-    forall k,
-      keys_compatible k k = true.
+  Lemma merge_keys_add_l_pull_in :
+    forall ks2 ks1 k k',
+        ks2 $? key_ref k  = Some k'
+      -> ks1 $? key_ref k' = None
+      -> key_perms_good ks1
+      -> key_perms_good ks2
+      -> key_ref k = key_ref k'
+      -> ks1 $k++ ks2 $+ (key_ref k, greatest_permission k k') = (ks1 $+ (key_ref k, k)) $k++ ks2.
   Proof.
-    unfold keys_compatible; intros.
-    cases (keyId k ==n keyId k); eauto.
-    cases (keyUsage k ==ku keyUsage k); eauto.
-    unfold key_type_same; cases (keyType k); eauto.
+    induction ks2 using P.map_induction_bis; auto; intros.
+    - apply map_eq_Equal in H; subst; auto.
+    - clean_map_lookups.
+    - apply key_perms_good_add in H3; split_ands; subst; auto.
+      cases (key_ref e ==n key_ref k'); try rewrite e0 in *; clean_map_lookups; auto.
+      + unfold merge_perms.
+        rewrite !fold_add; auto.
+        rewrite merge_perms_notation.
+        rewrite merge_perms_notation with (ks1:=ks1 $+ (key_ref k, k)).
+        cases (ks2 $? key_ref k).
+        * rewrite H4 in *; clean_map_lookups.
+        * rewrite <- merge_keys_add_l_pull; auto.
+          unfold add_key_perm_fold_fn, add_key_perm.
+          assert (ks1 $k++ ks2 $? key_ref k' = None) as RW by (eauto using merge_perms_adds_no_new_perms);
+            rewrite <- e0 in RW; rewrite RW; simpl; clean_map_lookups. rewrite e0,H4; clean_map_lookups.
+          rewrite H4 in H0; clean_map_lookups.
+          apply map_eq_Equal; unfold Equal; intros.
+          cases (key_ref k' ==n y); subst; clean_map_lookups; auto.
+          rewrite greatest_permission_symm; trivial.
+      + unfold merge_perms.
+        rewrite !fold_add; auto.
+        rewrite merge_perms_notation.
+        rewrite merge_perms_notation with (ks1:=ks1 $+ (key_ref k, k)).
+        rewrite H4 in H0; clean_map_lookups.
+        assert (key_ref e <> key_ref k) by (rewrite H4; assumption).
+        rewrite <- H4 in H0.
+        erewrite <- IHks2; eauto.
+        unfold add_key_perm_fold_fn, add_key_perm.
+        clean_map_lookups.
+        cases (ks1 $k++ ks2 $? key_ref e); subst; clean_map_lookups;
+          apply map_eq_Equal; unfold Equal; intros;
+            cases (y ==n key_ref e); cases (y ==n key_ref k); subst; clean_map_lookups; auto.
   Qed.
 
-  Lemma keys_compatible_symmetric :
-    forall k1 k2,
-      keys_compatible k1 k2 = keys_compatible k2 k1.
+  Lemma merge_perms_sym :
+    forall ks2 ks1,
+      key_perms_good ks1
+      -> key_perms_good ks2
+      -> ks1 $k++ ks2 = ks2 $k++ ks1.
   Proof.
-    unfold keys_compatible; intros.
-    cases (keyId k1 ==n keyId k2).
-    cases (keyUsage k1 ==ku keyUsage k2).
-    cases (key_type_same (keyType k1) (keyType k2)).
-    - rewrite e; rewrite e0; cases (keyId k2 ==n keyId k2); cases (keyUsage k2 ==ku keyUsage k2); try contradiction.
-      unfold key_type_same in *; cases (keyType k1); cases (keyType k2); auto.
-    - rewrite e; rewrite e0; cases (keyId k2 ==n keyId k2); cases (keyUsage k2 ==ku keyUsage k2); try contradiction.
-      unfold key_type_same in *; cases (keyType k1); cases (keyType k2); auto.
-    - rewrite e; cases (keyId k2 ==n keyId k2); auto.
-      cases (keyUsage k2 ==ku keyUsage k1); auto.
-      unfold key_type_same in *; cases (keyType k1); cases (keyType k2); auto.
-    - cases (keyId k2 ==n keyId k1); cases (keyUsage k2 ==ku keyUsage k1); try contradiction; auto.
-      symmetry in e; contradiction.
+    induction ks2 using P.map_induction_bis; auto; intros.
+    - apply map_eq_Equal in H; subst; auto.
+    - rewrite merge_keys_right_identity, merge_perms_left_identity; trivial.
+    - apply key_perms_good_add in H1; split_ands; subst; auto.
+      unfold merge_perms at 1; rewrite fold_add; auto.
+      rewrite merge_perms_notation.
+      unfold add_key_perm_fold_fn, add_key_perm; simpl.
+
+      cases (ks1 $k++ ks2 $? key_ref e); subst; clean_map_lookups.
+      + apply merge_perms_came_from_somewhere1 in Heq; auto.
+        assert (key_ref k = key_ref e) by auto.
+        assert (ks2 $? key_ref k = None) by (rewrite H1; assumption).
+        rewrite IHks2 by auto.
+        erewrite <- merge_keys_add_l_pull_in; eauto.
+      + apply merge_perms_no_disappear_perms in Heq; auto; split_ands.
+        rewrite <- merge_keys_add_l_pull; auto.
+        rewrite IHks2; auto.
   Qed.
 
-  Lemma merge_keys_ok :
-    forall ks2 k_id k1 k2 ks ks1,
-        ks1 $? k_id = Some k1
-      -> ks2 $? k_id = Some k2
-      -> ks = ks1 $k++ ks2
-      -> ( ks $? k_id = Some k1 /\ k1 = k2)
-      \/ ( ks $? k_id = Some (canonical_key k1 k2)).
-  Proof.
-    unfold merge_keys.
-    induction ks2 using P.map_induction_bis; intros.
-
-    - apply map_eq_Equal in H; subst; eauto.
-    - invert H0.
-
-    - subst. progress_fold_add1; clean_map_lookups; eauto.
-      rewrite merge_keys_notation.
-      case (x ==n k_id); intros; subst; clean_map_lookups.
-      + remember (ks1 $k++ ks2) as ks.
-        specialize (merge_keys_adds_ks1 _ _ _ H0 H Heqks). intros; subst.
-        cases (k2 ==kk k1).
-        * unfold add_key; subst. rewrite H1.
-          rewrite canonical_key_refl; simpl.
-          cases (k1 ==kk k1); try contradiction; eauto.
-
-        * unfold add_key; rewrite H1; simpl. cases (k2 ==kk k1); try contradiction.
-          rewrite canonical_key_sym.
-          assert (k1 <> k2) by auto.
-
-          clean_map_lookups; intuition idtac.
-
-      + unfold add_key.
-        cases (ks1 $k++ ks2 $? x); eauto.
-        * cases (e ==kk k); clean_map_lookups; eauto.
-        * clean_map_lookups; eauto.
-  Qed.
-
-  Lemma merge_keys_refl :
+  Lemma merge_perms_refl :
     forall ks,
-      ks $k++ ks = ks.
+      key_perms_good ks
+      -> ks $k++ ks = ks.
   Proof.
-    intros; apply map_eq_Equal; unfold Equal; subst; intros.
-    cases (ks $? y).
-    - remember (ks $k++ ks) as ksks.
-      pose proof (merge_keys_ok _ _ _ Heq Heq Heqksks).
-      rewrite canonical_key_refl in *.
-      intuition idtac.
-    - rewrite merge_keys_adds_no_new_keys; eauto.
+    induction ks using P.map_induction_bis; auto.
+    - apply map_eq_Equal in H; subst; auto.
+    - unfold merge_perms; intros.
+      apply key_perms_good_add in H0; split_ands; subst; auto.
+      progress_fold_add1; auto.
+      rewrite merge_perms_notation.
+      unfold add_key_perm_fold_fn , add_key_perm.
+      rewrite <- merge_keys_add_l_pull; clean_map_lookups; auto.
+      rewrite IHks; auto.
+      apply map_eq_Equal; unfold Equal; intros.
+      cases (y ==n key_ref e); subst; clean_map_lookups; auto.
+      rewrite greatest_permission_refl; trivial.
   Qed.
 
-  Lemma merge_keys_symmetric :
-    forall ks1 ks2,
-      ks1 $k++ ks2 = ks2 $k++ ks1.
+  Hint Extern 1 (key_perms_good (_ $k++ _)) => apply key_perms_merge_still_good.
+
+  Lemma merge_perms_chooses_greatest :
+    forall ks2 ks1 k k',
+      key_perms_good ks1
+      -> key_perms_good ks2
+      -> ks1 $? key_ref k = Some k
+      -> ks2 $? key_ref k' = Some k'
+      -> key_ref k = key_ref k'
+      -> (ks1 $k++ ks2) $? key_ref k = Some (greatest_permission k k').
   Proof.
-    intros.
-
-    apply map_eq_Equal; unfold Equal; subst; intros.
-
-    cases (ks1 $? y); cases (ks2 $? y).
-    - remember (ks1 $k++ ks2) as ks12. remember (ks2 $k++ ks1) as ks21.
-      pose proof (merge_keys_ok _ _ _ Heq Heq0 Heqks12).
-      pose proof (merge_keys_ok _ _ _ Heq0 Heq Heqks21).
-
-      (repeat match goal with
-              | [ H : _ /\ _ |- _ ] => destruct H; subst
-              | [ H : _ \/ _ |- _ ] => destruct H
-              | [ |- context [canonical_key ?k ?k]] => rewrite canonical_key_refl
-              | [ H : _ $k++ _ $? _ = Some _ |- _ ] => rewrite H
-              | [ H : _ $? _ = Some _ |- _ ] => rewrite H
-              end);
-        eauto.
-      rewrite canonical_key_sym; trivial.
-
-    - erewrite (merge_keys_adds_ks1); eauto.
-      erewrite (merge_keys_adds_ks2); eauto.
-    - erewrite (merge_keys_adds_ks2); eauto.
-      erewrite (merge_keys_adds_ks1); eauto.
-    - rewrite merge_keys_adds_no_new_keys; eauto.
-      rewrite merge_keys_adds_no_new_keys; eauto.
+    induction ks2 using P.map_induction_bis; intros; auto.
+    - apply map_eq_Equal in H; subst; auto.
+    - invert H2.
+    - apply key_perms_good_add in H1; split_ands; subst; auto.
+      progress_fold_add1; auto.
+      rewrite merge_perms_notation.
+      unfold add_key_perm_fold_fn, add_key_perm.
+      cases (key_ref e ==n key_ref k'); subst; try rewrite e0 in *; clean_map_lookups.
+      + rewrite H4 in H2.
+        assert (ks1 $k++ ks2 $? key_ref k' = Some k) as RW by eauto using merge_perms_adds_ks1;
+          rewrite RW; rewrite H4; clean_map_lookups.
+        rewrite greatest_permission_symm; auto.
+      + assert (key_ref e <> key_ref k) by (rewrite H4; assumption).
+        cases (ks1 $k++ ks2 $? key_ref e); subst; clean_map_lookups; eauto.
   Qed.
 
-  Hint Extern 1 (keys_compatible _ _ = _) => eassumption || (rewrite keys_compatible_symmetric; eassumption).
-
-  Lemma merge_keys_inequal_addition_no_impact :
-    forall ks1 ks2 k_id k_id' k,
-      k_id <> k_id'
-      -> ks1 $k++ (ks2 $+ (k_id,k)) $? k_id' = ks1 $k++ ks2 $? k_id'.
+  Lemma merge_perms_assoc_helper :
+    forall ks1 ks2 k_id k_id' k k',
+      ks1 $k++ ks2 $? k_id = Some k
+      -> key_ref k = k_id
+      -> key_ref k' = k_id'
+      -> k_id <> k_id'
+      -> ks1 $k++ (ks2 $+ (k_id',k')) $? k_id = Some k.
   Proof.
-    intros.
-    cases (ks1 $k++ ks2 $? k_id').
-    - apply merge_keys_split in Heq.
-      split_ors; split_ands; subst.
-      + eapply merge_keys_adds_ks2 with (ks2:=ks2 $+ (k_id, k)); clean_map_lookups; eauto.
-      + eapply merge_keys_adds_ks1 with (ks2:=ks2 $+ (k_id, k)); clean_map_lookups; eauto.
-      + destruct H0 as [k1 H0]. destruct H0 as [k2 H0]. split_ands.
-        remember (ks1 $k++ ks2) as ks.
-        specialize (merge_keys_ok _ _ _ H0 H1 Heqks); intros; split_ors; split_ands; subst.
-        * rewrite canonical_key_refl.
-          eapply merge_keys_canonicalizes' with (ks2:=ks2 $+ (k_id, k)). eauto. clean_map_lookups; eauto. rewrite canonical_key_refl; trivial.
-        * eapply merge_keys_canonicalizes' with (ks2:=ks2 $+ (k_id, k)). eauto. clean_map_lookups; eauto. trivial.
-    - apply merge_keys_no_disappear_keys in Heq; split_ands.
-      eapply merge_keys_adds_no_new_keys; auto.
-      clean_map_lookups; auto.
+  Admitted.
+
+
+  Lemma merge_perms_assoc :
+    forall ks3 ks1 ks2,
+      key_perms_good ks1
+      -> key_perms_good ks2
+      -> key_perms_good ks3
+      -> ks1 $k++ ks2 $k++ ks3 = ks1 $k++ (ks2 $k++ ks3).
+  Proof.
+    induction ks3 using P.map_induction_bis; intros; auto.
+    - apply map_eq_Equal in H; subst; auto.
+    - apply key_perms_good_add in H2; split_ands; subst; auto.
+      unfold merge_perms at 1.
+      unfold merge_perms at 3.
+      rewrite !fold_add; auto.
+      rewrite merge_perms_notation.
+      unfold add_key_perm_fold_fn at 1.
+      unfold add_key_perm_fold_fn at 1.
+      unfold add_key_perm.
+      rewrite merge_perms_notation with (ks1:=ks2).
+
+      cases (ks1 $k++ ks2 $k++ ks3 $? key_ref e);
+        cases (ks2 $k++ ks3 $? key_ref e); subst; clean_map_lookups;
+          rewrite IHks3 in Heq; auto.
+      + cases (ks1 $? key_ref e).
+        * assert (key_perms_good (ks1 $k++ (ks2 $k++ ks3))) as GD1 by eauto; specialize (GD1 _ _ Heq).
+          assert (key_perms_good (ks1)) as GD2 by eauto; specialize (GD2 _ _ Heq1).
+          assert (key_perms_good (ks2 $k++ ks3)) as GD3 by eauto; specialize (GD3 _ _ Heq0).
+          assert ( ks1 $k++ (ks2 $k++ ks3) $? key_ref k1 = Some (greatest_permission k1 k0) ).
+          eapply merge_perms_chooses_greatest; auto. rewrite GD2; auto. rewrite GD3; auto. rewrite GD2,GD3; trivial.
+          rewrite GD2 in H2. clean_map_lookups.
+          apply map_eq_Equal; unfold Equal; intros.
+          cases (y ==n key_ref e); subst; clean_map_lookups.
+          ** symmetry. rewrite <- GD2 in Heq1.
+             rewrite <- GD2.
+             erewrite merge_perms_chooses_greatest with (k' := greatest_permission e k0); eauto;
+               destruct e; destruct k1; destruct k0; simpl in *; subst; simpl in *;
+                 unfold greatest_permission; simpl; auto.
+             rewrite !orb_assoc, orb_comm with (b1:= has_private_access1); trivial.
+             unfold key_perms_good; intros.
+             cases (key_ref0 ==n k_id); subst; clean_map_lookups; auto.
+             assert (key_perms_good (ks2 $k++ ks3)) by auto. specialize (H4 _ _ H2); eauto.
+             clean_map_lookups; trivial.
+          ** rewrite IHks3; auto.
+             cases (ks1 $k++ (ks2 $k++ ks3) $? y); symmetry.
+             *** assert (key_perms_good (ks1 $k++ (ks2 $k++ ks3))) as GD by auto; specialize (GD _ _ Heq2).
+                 apply merge_perms_assoc_helper; eauto.
+                 unfold greatest_permission; destruct e; destruct k0; simpl in *; eauto.
+             *** apply merge_perms_no_disappear_perms in Heq2; auto; split_ands.
+                 eapply merge_perms_adds_no_new_perms; clean_map_lookups; auto.
+                 unfold key_perms_good; intros.
+                 cases (k_id ==n key_ref e); subst; clean_map_lookups.
+                 unfold greatest_permission; destruct e; destruct k0; simpl in *; trivial.
+                 assert (key_perms_good (ks2 $k++ ks3)) by auto. specialize (H6 _ _ H5); eauto.
+
+        * apply merge_perms_came_from_somewhere2 in Heq; auto; clean_map_lookups.
+          apply map_eq_Equal; unfold Equal; intros.
+          cases (y ==n key_ref e); subst; clean_map_lookups.
+          ** symmetry.
+             eapply merge_perms_adds_ks2 with (ks2 := ks2 $k++ ks3 $+ (key_ref e, greatest_permission e k0));
+               clean_map_lookups; eauto.
+             unfold key_perms_good; intros.
+             cases (k_id ==n key_ref e); subst; clean_map_lookups; eauto.
+             assert (key_perms_good (ks2 $k++ ks3)) as GD by eauto; specialize (GD _ _ Heq).
+             unfold greatest_permission; destruct e; destruct k0; simpl in *; trivial.
+             assert (key_perms_good (ks2 $k++ ks3)) as GD by eauto; specialize (GD _ _ H2); auto.
+          ** rewrite IHks3; auto.
+             cases (ks1 $k++ (ks2 $k++ ks3) $? y); symmetry.
+             *** assert (key_perms_good (ks1 $k++ (ks2 $k++ ks3))) as GD by auto; specialize (GD _ _ Heq0).
+                 apply merge_perms_assoc_helper; eauto.
+                 unfold greatest_permission; destruct e; destruct k0; simpl in *; eauto.
+             *** apply merge_perms_no_disappear_perms in Heq0; auto; split_ands.
+                 eapply merge_perms_adds_no_new_perms; clean_map_lookups; auto.
+                 unfold key_perms_good; intros.
+                 cases (k_id ==n key_ref e); subst; clean_map_lookups.
+                 unfold greatest_permission; destruct e; destruct k0; simpl in *; trivial.
+                 assert (key_perms_good (ks2 $k++ ks3)) by auto. specialize (H6 _ _ H5); eauto.
+
+      + unfold merge_perms at 3.
+        rewrite fold_add; auto.
+        rewrite merge_perms_notation with (ks2:=ks2 $k++ ks3).
+        unfold add_key_perm_fold_fn, add_key_perm.
+        rewrite Heq.
+        rewrite IHks3; auto.
+      + apply merge_perms_no_disappear_perms in Heq; auto; split_ands; contra_map_lookup.
+
+      + unfold merge_perms at 3.
+        rewrite fold_add; auto.
+        rewrite merge_perms_notation with (ks2:=ks2 $k++ ks3).
+        unfold add_key_perm_fold_fn, add_key_perm.
+        rewrite Heq.
+        rewrite IHks3; auto.
   Qed.
 
-  Lemma merge_keys_assoc :
-    forall ks3 ks1 ks2 : keys,
-      ks1 $k++ ks2 $k++ ks3 = ks1 $k++ (ks2 $k++ ks3).
-  Proof.
-    induction ks3 using P.map_induction_bis; intros.
-
-    - apply map_eq_Equal in H; subst; eauto.
-    - rewrite !merge_keys_right_identity; trivial.
-    - apply map_eq_Equal; unfold Equal; subst; intros.
-      unfold merge_keys.
-      progress_fold_add1; auto. progress_fold_add1; auto.
-      rewrite merge_keys_notation with (ks1 := ks1).
-      rewrite merge_keys_notation with (ks2 := ks3).
-      unfold add_key at 1; unfold add_key at 2.
-
-      (* clean up notation of induction hypothesis *) 
-      specialize (IHks3 ks1 ks2); unfold merge_keys in IHks3.
-      rewrite merge_keys_notation  with (ks1 := ks1) in IHks3.
-      rewrite merge_keys_notation  with (ks1 := ks2) in IHks3.
-      rewrite merge_keys_notation  with (ks2 := ks3) in IHks3.
-      rewrite merge_keys_notation  with (ks2 := ks2 $k++ ks3) in IHks3.
-
-      rewrite merge_keys_notation with (ks1 := ks2).
-
-      Ltac rewrite123 :=
-        match goal with | [ H : _ $k++ _ $k++ _ $? _ = _ |- _ ] => rewrite H end.
-
-      cases (ks1 $k++ ks2 $k++ ks3 $? x);
-        intros; subst; clean_map_lookups.
-
-      + cases (ks2 $k++ ks3 $? x).
-        * assert (ks1 $k++ ks2 $k++ ks3 $? x = Some k) as S by auto.
-          rewrite IHks3 in S; eapply merge_keys_split in S; auto.
-          cases (e ==kk k); cases (e ==kk k0); subst.
-          ** rewrite merge_keys_notation with (ks2:=ks2$k++ks3); rewrite IHks3; trivial.
-          ** rewrite merge_keys_notation with (ks2:=ks2 $k++ ks3 $+ (x, canonical_key k k0)).
-             split_ors; split_ands; subst.
-             *** rewrite Heq0 in H1; invert H1. contradiction.
-             *** contra_map_lookup.
-             *** destruct H0 as [k1 H0]. destruct H0 as [k2]. split_ands. rewrite Heq0 in H1; invert H1. symmetry.
-                 rewrite <- canonical_key_assoc. rewrite canonical_key_refl.
-                 cases (x ==n y); subst.
-                   rewrite Heq. eapply merge_keys_canonicalizes'. eassumption. clean_map_lookups. reflexivity. rewrite canonical_key_assoc, canonical_key_refl; trivial.
-                   rewrite IHks3. eapply merge_keys_inequal_addition_no_impact; assumption.
-          ** rewrite merge_keys_notation with (ks2:=ks2$k++ks3). rewrite <- IHks3.
-             split_ors; split_ands; subst.
-             *** rewrite Heq0 in H1; invert H1. contradiction.
-             *** contra_map_lookup.
-             *** destruct H0 as [k1 H0]. destruct H0 as [k2]. split_ands. rewrite Heq0 in H1; invert H1.
-                 cases (x ==n y); subst.
-                   rewrite canonical_key_sym, <- canonical_key_assoc, canonical_key_refl. clean_map_lookups; rewrite Heq; trivial.
-                   clean_map_lookups; trivial.
-          ** rewrite merge_keys_notation with (ks2:=ks2 $k++ ks3 $+ (x, canonical_key e k0)).
-             split_ors; split_ands; subst.
-             *** rewrite Heq0 in H1; invert H1. symmetry.
-                 cases (x ==n y); subst; clean_map_lookups.
-                   eapply merge_keys_adds_ks2. eauto. 2:reflexivity. clean_map_lookups; trivial.
-                   rewrite IHks3. eapply merge_keys_inequal_addition_no_impact; assumption.
-             *** contra_map_lookup.
-             *** destruct H0 as [k1 H0]. destruct H0 as [k2]. split_ands. rewrite Heq0 in H1; invert H1.
-                 symmetry.
-                 cases (x ==n y); subst; clean_map_lookups.
-                 **** eapply merge_keys_canonicalizes'; clean_map_lookups; eauto.
-                      rewrite canonical_key_assoc, canonical_key_sym with (k1:=e), <- canonical_key_assoc; trivial.
-                 **** rewrite IHks3. eapply merge_keys_inequal_addition_no_impact; assumption.
-
-        * cases (e ==kk k); subst.
-          ** rewrite fold_add; auto. unfold add_key at 1. rewrite merge_keys_notation with (ks2:=ks2 $k++ ks3), <- IHks3. rewrite Heq.
-             cases (k ==kk k); simpl; eauto. contradiction.
-          ** rewrite fold_add; auto. unfold add_key at 1. rewrite merge_keys_notation with (ks2:=ks2 $k++ ks3), <- IHks3. rewrite Heq.
-             cases (e ==kk k); simpl; eauto. contradiction.
-
-
-      + assert (ks1 $k++ ks2 $k++ ks3 $? x = None) as HH by assumption; rewrite IHks3 in HH; eapply merge_keys_no_disappear_keys in HH; split_ands.
-        rewrite H1.
-        progress_fold_add1; auto.
-        unfold add_key at 1.
-        rewrite merge_keys_notation with (ks2:=ks2 $k++ ks3). rewrite <- IHks3. rewrite Heq; clean_map_lookups; trivial.
-  Qed.
-
-  Lemma findUserKeys_fold_fn_proper :
+  Lemma merge_perm_heaps_proper :
     forall {A},
-    Morphisms.Proper
-      (Morphisms.respectful eq (Morphisms.respectful eq (Morphisms.respectful eq eq)))
-      (fun (_ : NatMap.key) (u : user_data A) (ks : keys) => ks $k++ key_heap u).
-    unfold Morphisms.Proper, Morphisms.respectful; intros; simpl; subst; trivial.
+      Proper (eq ==> eq ==> eq ==> eq) (fun (_ : NatMap.key) (u : user_data A) (ks : key_perms) => ks $k++ key_heap u).
+  Proof.
+    unfold Proper, respectful; intros; subst; trivial.
   Qed.
 
-  Lemma findUserKeys_fold_fn_proper_Equal :
+  Lemma merge_perm_heaps_transpose :
     forall {A},
-    Morphisms.Proper
-      (Morphisms.respectful eq (Morphisms.respectful eq (Morphisms.respectful Equal Equal)))
-      (fun (_ : NatMap.key) (u : user_data A) (ks : keys) => ks $k++ key_heap u).
-    unfold Morphisms.Proper, Morphisms.respectful; intros.
-    apply map_eq_Equal in H1; subst.
-    unfold Equal; intros; trivial.
-  Qed.
-
-  Lemma findUserKeys_transpose :
-    forall {A},
-      transpose_neqkey eq (fun (_ : NatMap.key) (u : user_data A) (ks : keys) => ks $k++ key_heap u).
+      transpose_neqkey eq (fun (_ : NatMap.key) (u : user_data A) (ks : key_perms) => ks $k++ key_heap u).
   Proof.
     unfold transpose_neqkey; intros.
-    rewrite merge_keys_symmetric with (ks1 := a).
-    rewrite merge_keys_symmetric with (ks1 := a $k++ key_heap e).
-    rewrite merge_keys_assoc; trivial.
-  Qed.
+    rewrite !merge_perms_assoc, merge_perms_sym with (ks1:= key_heap e'); trivial.
 
-  Lemma findUserKeys_transpose_Equal :
-    forall {A},
-      transpose_neqkey Equal (fun (_ : NatMap.key) (u : user_data A) (ks : keys) => ks $k++ key_heap u).
+  Admitted.
+
+
+
+
+
+  Lemma findKeys_good :
+    forall {t} (msg : message t),
+      key_perms_good (findKeys msg).
   Proof.
-    unfold transpose_neqkey; intros.
-    unfold Equal; intros.
-    rewrite merge_keys_symmetric with (ks1 := a).
-    rewrite merge_keys_symmetric with (ks1 := a $k++ key_heap e).
-    rewrite merge_keys_assoc; trivial.
+    induction msg; intros; simpl in *; subst; eauto using key_perms_merge_still_good.
   Qed.
 
-  Hint Resolve findUserKeys_fold_fn_proper findUserKeys_fold_fn_proper_Equal findUserKeys_transpose findUserKeys_transpose_Equal.
+  Definition all_user_key_perms_good {A} (usrs : honest_users A) :=
+    forall u_id u_d, usrs $? u_id = Some u_d -> key_perms_good u_d.(key_heap).
+
+  Lemma findUserKeys_result_perms_good :
+    forall {A} (usrs : honest_users A),
+        all_user_key_perms_good usrs
+      -> key_perms_good (findUserKeys usrs).
+  Proof.
+    unfold all_user_key_perms_good, findUserKeys; intros.
+    apply P.fold_rec_bis; auto; intros.
+    apply find_mapsto_iff in H0.
+    apply key_perms_merge_still_good; eauto.
+  Qed.
+
+  (* Lemma findUserKeys_as_map_fold : *)
+  (*   forall {A} (usrs : honest_users A), *)
+  (*     all_user_key_perms_good usrs *)
+  (*     -> findUserKeys usrs = fold (fun _ => merge_perms) (map (@key_heap A) usrs) $0. *)
+  (* Proof. *)
+  (*   unfold findUserKeys; intros. *)
+  (*   apply P.fold_rec_bis; intros; subst; eauto. *)
+  (*   - apply map_eq_Equal in H0; subst; auto. *)
+  (*   - admit. *)
+  (* Admitted. *)
+
+  Lemma findUserKeys_readd_user_same_keys_idempotent :
+    forall {A} (usrs : honest_users A) u_id u_d proto msgs,
+      usrs $? u_id = Some u_d
+      -> all_user_key_perms_good usrs
+      -> key_perms_good (findUserKeys usrs)
+      -> findUserKeys usrs = findUserKeys (usrs $+ (u_id, {| key_heap := key_heap u_d; protocol := proto; msg_heap := msgs |})).
+  Proof.
+    intros.
+    unfold findUserKeys; generalize H H0 H1.
+    apply P.fold_rec_bis; intros; subst.
+    - apply map_eq_Equal in H2; subst; auto.
+    - invert H2.
+    - unfold all_user_key_perms_good in H6.
+      assert (key_perms_good (key_heap e)) by (eapply H6 with (u_id := k); clean_map_lookups; auto).
+      cases (k ==n u_id); subst; clean_map_lookups.
+
+  Admitted.
+
+
+  Lemma safe_messages_have_no_bad_keys :
+    forall {t} (msg : message t) msgk,
+      msg_needs_encryption all_keys honestk msg = false
+      -> adv_no_honest_keys all_keys honestk advk
+      -> msgk = findKeys msg
+      -> forall k_id k,
+            msgk $? k_id = Some k
+          -> honest_key all_keys honestk k_id = false.
+  Proof.
+    induction msg; auto; intros; simpl in *; subst; clean_map_lookups.
+
+    - destruct k; simpl in *.
+      unfold honest_key.
+      cases (key_ref0 ==n k_id); subst; clean_map_lookups.
+      cases (all_keys $? k_id); eauto.
+      destruct k.
+      specialize (k_good _ Heq); simpl in k_good; subst.
+      unfold honest_key in *. rewrite Heq in H.
+      cases keyType0; eauto.
+    - apply orb_false_elim in H; split_ands.
+      assert (key_perms_good (findKeys msg1 $k++ findKeys msg2)) as FIND by eauto using findKeys_good, key_perms_merge_still_good.
+      assert (findKeys msg1 $k++ findKeys msg2 $? k_id = Some k) as KID by assumption.
+      apply FIND in KID; rewrite <- KID in H2.
+      apply merge_perms_split in H2; eauto using findKeys_good.
+      split_ors; eauto.
+  Qed.
+
+  (* Definition key_heaps_compatible (ks1 ks2 : keys) := *)
+  (*     keys_good ks1 *)
+  (*   /\ keys_good ks2 *)
+  (*   /\ (forall k_id k k', ks1 $? k_id = Some k -> ks2 $? k_id = Some k' -> keys_compatible k k' = true). *)
+
+  (* Lemma canonical_key_one_other : *)
+  (*   forall k1 k2, *)
+  (*       canonical_key k1 k2 = k1 *)
+  (*     \/ canonical_key k1 k2 = k2. *)
+  (* Proof. *)
+  (*   intros; unfold canonical_key. *)
+  (*   destruct k1; destruct k2; simpl. *)
+  (*   cases (keyId0 ?= keyId1); *)
+  (*     cases keyUsage0; cases keyUsage1; *)
+  (*       cases keyType0; cases keyType1; eauto; *)
+  (*         try rewrite Nat.compare_refl; simpl; eauto; *)
+  (*           cases has_private_access; cases has_private_access0; eauto. *)
+  (* Qed. *)
+
+  (* Lemma canonical_key_refl : *)
+  (*   forall k, canonical_key k k = k. *)
+  (* Proof. *)
+  (*   unfold canonical_key; intros; simpl. *)
+  (*   rewrite Nat.compare_refl. *)
+  (*   cases (keyUsage k); cases (keyType k); simpl; eauto; cases has_private_access; eauto. *)
+  (* Qed. *)
+
+  (* Lemma canonical_key_sym : *)
+  (*   forall k1 k2, *)
+  (*     canonical_key k1 k2 = canonical_key k2 k1. *)
+  (* Proof. *)
+  (*   intros; destruct k1; destruct k2; unfold canonical_key; simpl. *)
+  (*   cases (keyId0 ?= keyId1). *)
+  (*   - apply Nat.compare_eq in Heq; subst. *)
+  (*     rewrite Nat.compare_refl. *)
+  (*     cases keyUsage0; cases keyUsage1; cases keyType0; cases keyType1; eauto. *)
+  (*     cases has_private_access; cases has_private_access0; eauto. *)
+  (*     cases has_private_access; cases has_private_access0; eauto. *)
+
+  (*   - rewrite Nat.compare_antisym; rewrite Heq; simpl; auto. *)
+  (*   - rewrite Nat.compare_antisym; rewrite Heq; simpl; auto. *)
+  (* Qed. *)
+
+  (* Lemma canonical_key_assoc : *)
+  (*   forall k1 k2 k3, *)
+  (*     canonical_key k1 (canonical_key k2 k3) = canonical_key (canonical_key k1 k2) k3. *)
+  (* Proof. *)
+  (*   intros; destruct k1; destruct k2; destruct k3; unfold canonical_key; simpl. *)
+
+  (*   cases (keyId0 ?= keyId1); cases (keyId1 ?= keyId2). *)
+  (*   - apply Nat.compare_eq in Heq; apply Nat.compare_eq in Heq0; subst. simpl. *)
+  (*     cases keyUsage0; cases keyUsage1; cases keyUsage2; *)
+  (*       cases keyType0; cases keyType1; cases keyType2; *)
+  (*         simpl; eauto; *)
+  (*           try rewrite Nat.compare_refl; eauto; *)
+  (*             cases has_private_access; cases has_private_access0; try cases has_private_access1; simpl; *)
+  (*               try rewrite Nat.compare_refl; eauto. *)
+
+  (*   - apply Nat.compare_eq in Heq; subst; simpl. *)
+  (*     rewrite Heq0; simpl. *)
+  (*     cases keyUsage0; cases keyUsage1; cases keyUsage2; *)
+  (*       cases keyType0; cases keyType1; cases keyType2; *)
+  (*         simpl; eauto; try rewrite Heq0; simpl; eauto; *)
+  (*           cases has_private_access; cases has_private_access0; try cases has_private_access1; simpl; *)
+  (*             rewrite Heq0; simpl; eauto. *)
+
+  (*   - apply Nat.compare_eq in Heq; subst; simpl. *)
+  (*     rewrite Nat.compare_refl. *)
+  (*     cases keyUsage0; cases keyUsage1; cases keyUsage2; *)
+  (*       cases keyType0; cases keyType1; cases keyType2; *)
+  (*         simpl; eauto; try rewrite Heq0; simpl; eauto; *)
+  (*           cases has_private_access; cases has_private_access0; try cases has_private_access1; simpl; *)
+  (*             rewrite Heq0; simpl; eauto. *)
+
+  (*   - apply Nat.compare_eq in Heq0; subst; simpl. *)
+  (*     rewrite Nat.compare_refl; simpl. *)
+  (*     cases keyUsage0; cases keyUsage1; cases keyUsage2; *)
+  (*       cases keyType0; cases keyType1; cases keyType2; *)
+  (*         simpl; eauto; try rewrite Heq; simpl; eauto; *)
+  (*           cases has_private_access; cases has_private_access0; try cases has_private_access1; simpl; *)
+  (*             rewrite Heq; simpl; eauto. *)
+
+  (*   - simpl. rewrite Heq0. *)
+  (*     pose proof Heq as lt1; pose proof Heq0 as lt2. *)
+  (*     apply nat_compare_lt in lt1; apply nat_compare_lt in lt2. *)
+  (*     pose proof (Nat.lt_trans _ _ _ lt1 lt2). apply nat_compare_lt in H. *)
+  (*     rewrite H; eauto. *)
+
+  (*   - simpl; rewrite Heq; rewrite Heq0; eauto. *)
+
+  (*   - apply Nat.compare_eq in Heq0; subst; simpl. *)
+  (*     rewrite Heq; simpl. *)
+  (*     cases keyUsage0; cases keyUsage1; cases keyUsage2; *)
+  (*       cases keyType0; cases keyType1; cases keyType2; *)
+  (*         simpl; eauto; try rewrite Heq; simpl; eauto; *)
+  (*           cases has_private_access; cases has_private_access0; try cases has_private_access1; simpl; *)
+  (*             rewrite Heq; simpl; eauto. *)
+
+  (*   - simpl. cases (keyId0 ?= keyId2); simpl; eauto. *)
+  (*   - simpl. rewrite Heq. *)
+  (*     pose proof Heq as gt1; pose proof Heq0 as gt2. *)
+  (*     apply nat_compare_gt in gt1; apply nat_compare_gt in gt2. *)
+
+  (*     pose proof (gt_trans _ _ _ gt1 gt2); apply nat_compare_gt in H. *)
+  (*     rewrite H; simpl; eauto. *)
+  (* Qed. *)
+
+  (* Lemma merge_keys_fold_fn_proper : *)
+  (*     Morphisms.Proper *)
+  (*       (Morphisms.respectful eq (Morphisms.respectful eq (Morphisms.respectful eq eq))) *)
+  (*       add_key. *)
+  (* Proof. *)
+  (*   unfold Morphisms.Proper, Morphisms.respectful; intros; simpl; subst; trivial. *)
+  (* Qed. *)
+
+  (* Lemma merge_keys_fold_fn_proper_flip : *)
+  (*     Morphisms.Proper *)
+  (*       (Morphisms.respectful eq (Morphisms.respectful eq (Morphisms.respectful (Basics.flip eq) (Basics.flip eq)))) *)
+  (*       add_key. *)
+  (* Proof. *)
+  (*   unfold Morphisms.Proper, Morphisms.respectful; intros; simpl; unfold Basics.flip in *; subst; trivial. *)
+  (* Qed. *)
+
+  (* Lemma merge_keys_fold_fn_proper_Equal : *)
+  (*   Morphisms.Proper *)
+  (*     (Morphisms.respectful eq (Morphisms.respectful eq (Morphisms.respectful Equal Equal))) *)
+  (*     add_key. *)
+  (* Proof. *)
+  (*   unfold Morphisms.Proper, Morphisms.respectful; intros; simpl; subst. *)
+  (*   apply map_eq_Equal in H1; subst. *)
+  (*   apply Equal_refl. *)
+  (* Qed. *)
+
+  (* Lemma merge_keys_transpose : *)
+  (*   transpose_neqkey eq add_key. *)
+  (* Proof. *)
+  (*   unfold transpose_neqkey; intros. *)
+  (*   unfold add_key; simpl. *)
+  (*   case_eq (a $? k); case_eq (a $? k'); intros; subst; simpl. *)
+
+  (*   Ltac work1 := *)
+  (*     match goal with *)
+  (*     | [ H : ?x <> ?x |- _ ] => contradiction *)
+  (*     | [ H1 : ?x <> ?y, H2 : ?x = ?y |- _ ] => contradiction *)
+  (*     | [ H : ?a $? ?k  = _ |- context [?a $? ?k]  ] => rewrite H *)
+  (*     | [ H : ?a $? ?k' = _ |- context [?a $? ?k'] ] => rewrite H *)
+  (*     | [ |- context[ ?k1 ==kk ?k2 ] ] => case (k1 ==kk k2); intros; subst *)
+  (*     | [ H : keys_compatible ?k1 ?k2 = _ |- context [ keys_compatible ?k1 ?k2 ]] => rewrite H *)
+  (*     | [ |- context [ keys_compatible ?k1 ?k2 ]] => case_eq (keys_compatible k1 k2); intros *)
+  (*     | [ H : keyType ?k = _ |- context [ keyType ?k ==kt ?kt ]] => rewrite H *)
+  (*     | [ |- context [ keyType ?k ==kt ?kt ]] => case (keyType k ==kt kt); intros *)
+  (*     | [ |- context [ _ $+ (?k1, _) $? ?k1 ]] => rewrite add_eq_o by (trivial || auto) *)
+  (*     | [ |- context [ _ $+ (?k1, _) $? ?k2 ]] => rewrite add_neq_o by auto *)
+  (*     | [ |- context [ _ $- ?k1 $? ?k2 ]] => rewrite remove_neq_o by auto *)
+  (*     end. *)
+
+  (*   Ltac maps_equal := *)
+  (*     repeat match goal with *)
+  (*            | [ |- context[find ?k (add ?k _ _) ] ]  => rewrite add_eq_o by auto *)
+  (*            | [ |- context[find ?k (add ?k' _ _) ] ] => rewrite add_neq_o by auto *)
+  (*            | [ |- context[find ?k (remove ?k _) ] ]  => rewrite remove_eq_o by auto *)
+  (*            | [ |- context[find ?k (remove ?k' _) ] ] => rewrite remove_neq_o by auto *)
+  (*            | [ |- _ $+ (?k1,_) $? ?k = _ ] => case (k1 ==n k); intros; subst *)
+  (*            | [ |- _ $- ?k1     $? ?k = _ ] => case (k1 ==n k); intros; subst *)
+  (*            | [ |- add _ _ _ = _ ] => apply map_eq_Equal; unfold Equal; intros ?y *)
+  (*            end. *)
+
+  (*   repeat work1; eauto; *)
+  (*     apply map_eq_Equal; unfold Equal; intros; *)
+  (*       maps_equal; auto. *)
+    
+  (*   repeat work1; eauto; *)
+  (*     apply map_eq_Equal; unfold Equal; intros; *)
+  (*       maps_equal; auto. *)
+
+  (*   repeat work1; eauto; *)
+  (*     apply map_eq_Equal; unfold Equal; intros; *)
+  (*       maps_equal; auto. *)
+
+  (*   repeat work1; eauto; *)
+  (*     apply map_eq_Equal; unfold Equal; intros; *)
+  (*       maps_equal; auto. *)
+
+  (* Qed. *)
+
+  (* Lemma merge_keys_transpose_flip : *)
+  (*   transpose_neqkey (Basics.flip eq) add_key. *)
+  (* Proof. *)
+  (*   unfold transpose_neqkey, Basics.flip; intros. *)
+  (*   apply merge_keys_transpose; auto. *)
+  (* Qed. *)
+
+  (* Lemma eq_Equal : *)
+  (*   forall {V} (m m' : NatMap.t V), *)
+  (*     m = m' *)
+  (*     -> Equal m m'. *)
+  (*   intros; subst; apply Equal_refl. *)
+  (* Qed. *)
+
+  (* Lemma merge_keys_transpose_Equal : *)
+  (*   transpose_neqkey Equal add_key. *)
+  (* Proof. *)
+  (*   unfold transpose_neqkey; intros. *)
+  (*   apply eq_Equal. *)
+  (*   apply merge_keys_transpose; auto. *)
+  (* Qed. *)
+
+  (* Hint Resolve merge_keys_fold_fn_proper merge_keys_fold_fn_proper_flip merge_keys_fold_fn_proper_Equal *)
+  (*              merge_keys_transpose merge_keys_transpose_flip merge_keys_transpose_Equal. *)
+
+  (* Lemma merge_keys_left_identity : *)
+  (*   forall ks, *)
+  (*     $0 $k++ ks = ks. *)
+  (* Proof. *)
+  (*   unfold merge_keys. *)
+  (*   induction ks using P.map_induction_bis; intros. *)
+
+  (*   - apply map_eq_Equal in H; subst; auto. *)
+  (*   - apply fold_Empty; eauto. *)
+  (*   - rewrite fold_add; clean_map_lookups; eauto. *)
+  (*     rewrite IHks; clear IHks. *)
+  (*     unfold add_key; rewrite H; eauto. *)
+  (* Qed. *)
+
+  (* Lemma merge_keys_right_identity : *)
+  (*   forall ks, *)
+  (*     ks $k++ $0 = ks. *)
+  (* Proof. *)
+  (*   unfold merge_keys; intros; rewrite fold_Empty; eauto. *)
+  (* Qed. *)
+
+  (* Hint Resolve merge_keys_left_identity merge_keys_right_identity. *)
+
+  (* Lemma merge_keys_adds_no_new_keys : *)
+  (*   forall ks2 k ks1, *)
+  (*       ks1 $? k = None *)
+  (*     -> ks2 $? k = None *)
+  (*     -> (ks1 $k++ ks2) $? k = None. *)
+  (* Proof. *)
+  (*   induction ks2 using P.map_induction_bis; intros. *)
+  (*   - apply map_eq_Equal in H; subst; auto. *)
+  (*   - rewrite merge_keys_right_identity; auto. *)
+  (*   - unfold merge_keys; rewrite fold_add; auto. *)
+  (*     case (x ==n k); intros; subst; clean_map_lookups. *)
+  (*     + rewrite merge_keys_notation; unfold add_key. *)
+  (*       cases (ks1 $k++ ks2 $? x); clean_map_lookups; eauto. *)
+  (*       cases (e ==kk k0); subst; eauto. *)
+  (*       clean_map_lookups. eapply IHks2; auto. *)
+  (* Qed. *)
+
+  (* Lemma merge_keys_no_disappear_keys : *)
+  (*   forall ks2 k ks1, *)
+  (*     (ks1 $k++ ks2) $? k = None *)
+  (*   -> ks1 $? k = None *)
+  (*   /\ ks2 $? k = None. *)
+  (* Proof. *)
+  (*   induction ks2 using P.map_induction_bis; intros. *)
+  (*   - apply map_eq_Equal in H; subst; auto. *)
+  (*   - rewrite merge_keys_right_identity in H; eauto. *)
+  (*   - unfold merge_keys in H0. progress_fold_add1; auto. *)
+  (*     rewrite merge_keys_notation in *; clean_map_lookups. *)
+  (*     unfold add_key in H0. *)
+  (*     cases (ks1 $k++ ks2 $? x); clean_map_lookups; *)
+  (*       [cases (e ==kk k0); subst | ]; *)
+  (*         case (x ==n k); intros; subst; clean_map_lookups; eauto. *)
+  (* Qed. *)
+
+  (* Hint Resolve merge_keys_adds_no_new_keys merge_keys_no_disappear_keys. *)
+
+  (* Lemma merge_keys_adds_ks1 : *)
+  (*   forall ks2 ks1 k v ks, *)
+  (*       ks1 $? k = Some v *)
+  (*     -> ks2 $? k = None *)
+  (*     -> ks = ks1 $k++ ks2 *)
+  (*     -> ks $? k = Some v. *)
+  (* Proof. *)
+  (*   unfold merge_keys. *)
+  (*   induction ks2 using P.map_induction_bis; intros. *)
+
+  (*   - apply map_eq_Equal in H; subst; eauto. *)
+  (*   - subst; rewrite fold_Empty; eauto. *)
+  (*   - case (x ==n k); intros; subst; clean_map_lookups; eauto. *)
+  (*     rewrite fold_add; eauto. *)
+  (*     rewrite merge_keys_notation. *)
+  (*     unfold add_key. *)
+  (*     cases ( ks1 $k++ ks2 $? x ); clean_map_lookups; eauto. *)
+  (*     cases ( e ==kk k0 ); eauto. *)
+  (*     clean_map_lookups; eauto. *)
+  (* Qed. *)
+
+  (* Lemma merge_keys_adds_ks2 : *)
+  (*   forall ks2 ks1 k v ks, *)
+  (*       ks1 $? k = None *)
+  (*     -> ks2 $? k = Some v *)
+  (*     -> ks = ks1 $k++ ks2 *)
+  (*     -> ks $? k = Some v. *)
+  (* Proof. *)
+  (*   unfold merge_keys. *)
+  (*   induction ks2 using P.map_induction_bis; intros. *)
+
+  (*   - apply map_eq_Equal in H; subst; eauto. *)
+  (*   - invert H0. *)
+  (*   - subst. *)
+  (*     case (x ==n k); intros; subst; clean_map_lookups; eauto. *)
+  (*     + rewrite fold_add; auto. *)
+  (*       rewrite merge_keys_notation. *)
+  (*       unfold add_key. *)
+  (*       pose proof merge_keys_adds_no_new_keys. *)
+  (*       cases ( ks1 $k++ ks2 $? k); clean_map_lookups; eauto. *)
+  (*       cases ( v ==kk k0 ); subst; clean_map_lookups; eauto. *)
+  (*       specialize (H1 _ _ _ H0 H); contra_map_lookup. *)
+
+  (*     + rewrite fold_add; auto. *)
+  (*       rewrite merge_keys_notation. *)
+  (*       unfold add_key. *)
+  (*       cases ( ks1 $k++ ks2 $? x); clean_map_lookups; eauto. *)
+  (*       cases ( e ==kk k0 ); eauto. *)
+  (*       clean_map_lookups; eauto. *)
+  (* Qed. *)
+
+  (* Hint Resolve merge_keys_adds_ks1 merge_keys_adds_ks2. *)
+
+  (* Lemma merge_keys_came_from_somewhere1 : *)
+  (*   forall ks2 ks1 k v, *)
+  (*       ks1 $k++ ks2 $? k = Some v *)
+  (*     -> ks2 $? k = None *)
+  (*     -> ks1 $? k = Some v. *)
+  (* Proof. *)
+  (*   unfold merge_keys. *)
+  (*   induction ks2 using P.map_induction_bis; intros. *)
+
+  (*   - apply map_eq_Equal in H; subst; eauto. *)
+  (*   - rewrite fold_Empty in H; auto. *)
+
+  (*   - case (x ==n k); intros; subst; clean_map_lookups. *)
+  (*     + progress_fold_add1; auto. *)
+  (*       rewrite merge_keys_notation in H0; unfold add_key at 1 in H0. *)
+
+  (*       cases (ks1 $k++ ks2 $? x); clean_map_lookups; eauto. *)
+  (*       cases ( e ==kk k0 ); subst; clean_map_lookups; eauto. *)
+  (* Qed. *)
+
+  (* Lemma merge_keys_came_from_somewhere2 : *)
+  (*   forall ks2 ks1 k v, *)
+  (*       ks1 $k++ ks2 $? k = Some v *)
+  (*     -> ks1 $? k = None *)
+  (*     -> ks2 $? k = Some v. *)
+  (* Proof. *)
+  (*   unfold merge_keys. *)
+  (*   induction ks2 using P.map_induction_bis; intros. *)
+
+  (*   - apply map_eq_Equal in H; subst; eauto. *)
+  (*   - rewrite fold_Empty in H; clean_map_lookups; auto. *)
+
+  (*   - case (x ==n k); intros; subst; clean_map_lookups; progress_fold_add1; auto. *)
+  (*     * pose proof (merge_keys_adds_no_new_keys _ _ _ H1 H). *)
+  (*       rewrite merge_keys_notation in H0; unfold add_key in H0; auto. *)
+  (*       cases (ks1 $k++ ks2 $? k); clean_map_lookups; eauto. *)
+
+  (*     * rewrite merge_keys_notation in H0; unfold add_key in H0; auto. *)
+  (*       cases (ks1 $k++ ks2 $? x); clean_map_lookups; eauto. *)
+  (*       cases ( e ==kk k0 ); subst; clean_map_lookups; eauto. *)
+  (* Qed. *)
+
+  (* Hint Resolve merge_keys_came_from_somewhere1 merge_keys_came_from_somewhere2. *)
+
+  (* Lemma merge_keys_split : *)
+  (*   forall ks2 k_id k ks1, *)
+  (*     ks1 $k++ ks2 $? k_id = Some k *)
+  (*     -> (ks1 $? k_id = None /\ ks2 $? k_id = Some k) *)
+  (*     \/ (ks1 $? k_id = Some k /\ ks2 $? k_id = None) *)
+  (*     \/ exists k1 k2, ks1 $? k_id = Some k1 /\ ks2 $? k_id = Some k2 /\ k = canonical_key k1 k2. *)
+  (* Proof. *)
+  (*   unfold merge_keys. *)
+  (*   induction ks2 using P.map_induction_bis; intros. *)
+  (*   - apply map_eq_Equal in H; subst; eauto. *)
+  (*   - rewrite merge_keys_right_identity in H. intuition idtac. *)
+  (*   - rewrite fold_add in H0; auto. *)
+  (*     rewrite merge_keys_notation in H0; unfold add_key in H0; auto. *)
+  (*     case (x ==n k_id); intros; subst; clean_map_lookups. *)
+  (*     + cases (ks1 $k++ ks2 $? k_id); intros; simpl. *)
+  (*       * cases (e ==kk k0); subst. *)
+  (*         ** rewrite Heq in H0; invert H0. eapply merge_keys_came_from_somewhere1 in Heq; auto. *)
+  (*            right; right. do 2 eexists; intuition eauto. rewrite canonical_key_refl; trivial. *)
+  (*         ** clean_map_lookups; eapply merge_keys_came_from_somewhere1 in Heq; auto. *)
+  (*            right; right; do 2 eexists; intuition eauto. rewrite canonical_key_sym; trivial. *)
+
+  (*       * clean_map_lookups; eauto. eapply merge_keys_no_disappear_keys in Heq; invert Heq. *)
+  (*         intuition idtac. *)
+  (*     + cases (ks1 $k++ ks2 $? x); clean_map_lookups; eauto. *)
+  (*       cases (e ==kk k0); auto. *)
+  (*       cases (x ==n k_id); clean_map_lookups; auto. *)
+  (* Qed. *)
+
+  (* Lemma merge_keys_canonicalizes : *)
+  (*   forall ks2 k_id k k1 k2 ks1, *)
+  (*       ks1 $k++ ks2 $? k_id = Some k *)
+  (*     -> ks1 $? k_id = Some k1 *)
+  (*     -> ks2 $? k_id = Some k2 *)
+  (*     -> k = canonical_key k1 k2. *)
+  (* Proof. *)
+  (*   unfold merge_keys. *)
+  (*   induction ks2 using P.map_induction_bis; intros. *)
+  (*   - apply map_eq_Equal in H; subst; eauto. *)
+  (*   - invert H1. *)
+
+  (*   - rewrite fold_add in H0; auto. *)
+  (*     rewrite merge_keys_notation in H0; unfold add_key in H0; auto. *)
+  (*     case (x ==n k_id); intros; subst; clean_map_lookups. *)
+  (*     + cases (ks1 $k++ ks2 $? k_id); intros; simpl. *)
+  (*       * cases (k2 ==kk k0); subst; eauto. *)
+  (*         ** rewrite Heq in H0; invert H0. eapply merge_keys_came_from_somewhere1 in Heq; auto. rewrite Heq in H1; invert H1. rewrite canonical_key_refl; trivial. *)
+  (*         ** clean_map_lookups. eapply merge_keys_came_from_somewhere1 in Heq; auto. rewrite Heq in H1; invert H1. rewrite canonical_key_sym; trivial. *)
+
+  (*       * clean_map_lookups. eapply merge_keys_no_disappear_keys in Heq; destruct Heq; contra_map_lookup. *)
+
+  (*     + cases (ks1 $k++ ks2 $? x); clean_map_lookups; eauto. *)
+  (*       cases (e ==kk k0); subst; clean_map_lookups; eauto. *)
+  (* Qed. *)
+
+  (* Lemma merge_keys_canonicalizes' : *)
+  (*   forall ks2 k_id k k1 k2 ks1, *)
+  (*       ks1 $? k_id = Some k1 *)
+  (*     -> ks2 $? k_id = Some k2 *)
+  (*     -> k = canonical_key k1 k2 *)
+  (*     -> ks1 $k++ ks2 $? k_id = Some k. *)
+  (* Proof. *)
+  (*   unfold merge_keys. *)
+  (*   induction ks2 using P.map_induction_bis; intros. *)
+  (*   - apply map_eq_Equal in H; subst; eauto. *)
+  (*   - invert H0. *)
+
+  (*   - rewrite fold_add; auto. *)
+  (*     rewrite merge_keys_notation; unfold add_key. *)
+  (*     cases (ks1 $k++ ks2 $? x); case (x ==n k_id); intros; subst; clean_map_lookups. *)
+  (*     + cases (k2 ==kk k0); subst. *)
+  (*       * eapply (merge_keys_came_from_somewhere1) in Heq; auto. rewrite Heq in H0; invert H0. rewrite canonical_key_refl. eapply merge_keys_adds_ks1; eauto. *)
+  (*       * eapply (merge_keys_came_from_somewhere1) in Heq; auto. rewrite Heq in H0; invert H0. rewrite canonical_key_sym. clean_map_lookups; trivial. *)
+  (*     + cases (e ==kk k0); subst; clean_map_lookups; eauto. *)
+  (*     + eapply merge_keys_no_disappear_keys in Heq; invert Heq; contra_map_lookup. *)
+  (*     + eapply IHks2; eauto. *)
+  (* Qed. *)
+
+  (* Lemma add_key_results : *)
+  (*   forall k v ks ks', *)
+  (*     ks' = add_key k v ks *)
+  (*     -> ks' = ks *)
+  (*     \/ ks' = ks $+ (k,v) *)
+  (*     \/ exists k', ks' = ks $+ (k, canonical_key v k'). *)
+  (* Proof. *)
+  (*   unfold add_key; intros. *)
+  (*   cases (ks $? k); auto. *)
+  (*   cases (v ==kk k0); auto. *)
+  (*   intuition eauto. *)
+  (* Qed. *)
+
+  (* Lemma keys_compatible_reflexive : *)
+  (*   forall k, *)
+  (*     keys_compatible k k = true. *)
+  (* Proof. *)
+  (*   unfold keys_compatible; intros. *)
+  (*   cases (keyId k ==n keyId k); eauto. *)
+  (*   cases (keyUsage k ==ku keyUsage k); eauto. *)
+  (*   unfold key_type_same; cases (keyType k); eauto. *)
+  (* Qed. *)
+
+  (* Lemma keys_compatible_symmetric : *)
+  (*   forall k1 k2, *)
+  (*     keys_compatible k1 k2 = keys_compatible k2 k1. *)
+  (* Proof. *)
+  (*   unfold keys_compatible; intros. *)
+  (*   cases (keyId k1 ==n keyId k2). *)
+  (*   cases (keyUsage k1 ==ku keyUsage k2). *)
+  (*   cases (key_type_same (keyType k1) (keyType k2)). *)
+  (*   - rewrite e; rewrite e0; cases (keyId k2 ==n keyId k2); cases (keyUsage k2 ==ku keyUsage k2); try contradiction. *)
+  (*     unfold key_type_same in *; cases (keyType k1); cases (keyType k2); auto. *)
+  (*   - rewrite e; rewrite e0; cases (keyId k2 ==n keyId k2); cases (keyUsage k2 ==ku keyUsage k2); try contradiction. *)
+  (*     unfold key_type_same in *; cases (keyType k1); cases (keyType k2); auto. *)
+  (*   - rewrite e; cases (keyId k2 ==n keyId k2); auto. *)
+  (*     cases (keyUsage k2 ==ku keyUsage k1); auto. *)
+  (*     unfold key_type_same in *; cases (keyType k1); cases (keyType k2); auto. *)
+  (*   - cases (keyId k2 ==n keyId k1); cases (keyUsage k2 ==ku keyUsage k1); try contradiction; auto. *)
+  (*     symmetry in e; contradiction. *)
+  (* Qed. *)
+
+  (* Lemma merge_keys_ok : *)
+  (*   forall ks2 k_id k1 k2 ks ks1, *)
+  (*       ks1 $? k_id = Some k1 *)
+  (*     -> ks2 $? k_id = Some k2 *)
+  (*     -> ks = ks1 $k++ ks2 *)
+  (*     -> ( ks $? k_id = Some k1 /\ k1 = k2) *)
+  (*     \/ ( ks $? k_id = Some (canonical_key k1 k2)). *)
+  (* Proof. *)
+  (*   unfold merge_keys. *)
+  (*   induction ks2 using P.map_induction_bis; intros. *)
+
+  (*   - apply map_eq_Equal in H; subst; eauto. *)
+  (*   - invert H0. *)
+
+  (*   - subst. progress_fold_add1; clean_map_lookups; eauto. *)
+  (*     rewrite merge_keys_notation. *)
+  (*     case (x ==n k_id); intros; subst; clean_map_lookups. *)
+  (*     + remember (ks1 $k++ ks2) as ks. *)
+  (*       specialize (merge_keys_adds_ks1 _ _ _ H0 H Heqks). intros; subst. *)
+  (*       cases (k2 ==kk k1). *)
+  (*       * unfold add_key; subst. rewrite H1. *)
+  (*         rewrite canonical_key_refl; simpl. *)
+  (*         cases (k1 ==kk k1); try contradiction; eauto. *)
+
+  (*       * unfold add_key; rewrite H1; simpl. cases (k2 ==kk k1); try contradiction. *)
+  (*         rewrite canonical_key_sym. *)
+  (*         assert (k1 <> k2) by auto. *)
+
+  (*         clean_map_lookups; intuition idtac. *)
+
+  (*     + unfold add_key. *)
+  (*       cases (ks1 $k++ ks2 $? x); eauto. *)
+  (*       * cases (e ==kk k); clean_map_lookups; eauto. *)
+  (*       * clean_map_lookups; eauto. *)
+  (* Qed. *)
+
+  (* Lemma merge_keys_refl : *)
+  (*   forall ks, *)
+  (*     ks $k++ ks = ks. *)
+  (* Proof. *)
+  (*   intros; apply map_eq_Equal; unfold Equal; subst; intros. *)
+  (*   cases (ks $? y). *)
+  (*   - remember (ks $k++ ks) as ksks. *)
+  (*     pose proof (merge_keys_ok _ _ _ Heq Heq Heqksks). *)
+  (*     rewrite canonical_key_refl in *. *)
+  (*     intuition idtac. *)
+  (*   - rewrite merge_keys_adds_no_new_keys; eauto. *)
+  (* Qed. *)
+
+  (* Lemma merge_keys_symmetric : *)
+  (*   forall ks1 ks2, *)
+  (*     ks1 $k++ ks2 = ks2 $k++ ks1. *)
+  (* Proof. *)
+  (*   intros. *)
+
+  (*   apply map_eq_Equal; unfold Equal; subst; intros. *)
+
+  (*   cases (ks1 $? y); cases (ks2 $? y). *)
+  (*   - remember (ks1 $k++ ks2) as ks12. remember (ks2 $k++ ks1) as ks21. *)
+  (*     pose proof (merge_keys_ok _ _ _ Heq Heq0 Heqks12). *)
+  (*     pose proof (merge_keys_ok _ _ _ Heq0 Heq Heqks21). *)
+
+  (*     (repeat match goal with *)
+  (*             | [ H : _ /\ _ |- _ ] => destruct H; subst *)
+  (*             | [ H : _ \/ _ |- _ ] => destruct H *)
+  (*             | [ |- context [canonical_key ?k ?k]] => rewrite canonical_key_refl *)
+  (*             | [ H : _ $k++ _ $? _ = Some _ |- _ ] => rewrite H *)
+  (*             | [ H : _ $? _ = Some _ |- _ ] => rewrite H *)
+  (*             end); *)
+  (*       eauto. *)
+  (*     rewrite canonical_key_sym; trivial. *)
+
+  (*   - erewrite (merge_keys_adds_ks1); eauto. *)
+  (*     erewrite (merge_keys_adds_ks2); eauto. *)
+  (*   - erewrite (merge_keys_adds_ks2); eauto. *)
+  (*     erewrite (merge_keys_adds_ks1); eauto. *)
+  (*   - rewrite merge_keys_adds_no_new_keys; eauto. *)
+  (*     rewrite merge_keys_adds_no_new_keys; eauto. *)
+  (* Qed. *)
+
+  (* Hint Extern 1 (keys_compatible _ _ = _) => eassumption || (rewrite keys_compatible_symmetric; eassumption). *)
+
+  (* Lemma merge_keys_inequal_addition_no_impact : *)
+  (*   forall ks1 ks2 k_id k_id' k, *)
+  (*     k_id <> k_id' *)
+  (*     -> ks1 $k++ (ks2 $+ (k_id,k)) $? k_id' = ks1 $k++ ks2 $? k_id'. *)
+  (* Proof. *)
+  (*   intros. *)
+  (*   cases (ks1 $k++ ks2 $? k_id'). *)
+  (*   - apply merge_keys_split in Heq. *)
+  (*     split_ors; split_ands; subst. *)
+  (*     + eapply merge_keys_adds_ks2 with (ks2:=ks2 $+ (k_id, k)); clean_map_lookups; eauto. *)
+  (*     + eapply merge_keys_adds_ks1 with (ks2:=ks2 $+ (k_id, k)); clean_map_lookups; eauto. *)
+  (*     + destruct H0 as [k1 H0]. destruct H0 as [k2 H0]. split_ands. *)
+  (*       remember (ks1 $k++ ks2) as ks. *)
+  (*       specialize (merge_keys_ok _ _ _ H0 H1 Heqks); intros; split_ors; split_ands; subst. *)
+  (*       * rewrite canonical_key_refl. *)
+  (*         eapply merge_keys_canonicalizes' with (ks2:=ks2 $+ (k_id, k)). eauto. clean_map_lookups; eauto. rewrite canonical_key_refl; trivial. *)
+  (*       * eapply merge_keys_canonicalizes' with (ks2:=ks2 $+ (k_id, k)). eauto. clean_map_lookups; eauto. trivial. *)
+  (*   - apply merge_keys_no_disappear_keys in Heq; split_ands. *)
+  (*     eapply merge_keys_adds_no_new_keys; auto. *)
+  (*     clean_map_lookups; auto. *)
+  (* Qed. *)
+
+  (* Lemma merge_keys_assoc : *)
+  (*   forall ks3 ks1 ks2 : keys, *)
+  (*     ks1 $k++ ks2 $k++ ks3 = ks1 $k++ (ks2 $k++ ks3). *)
+  (* Proof. *)
+  (*   induction ks3 using P.map_induction_bis; intros. *)
+
+  (*   - apply map_eq_Equal in H; subst; eauto. *)
+  (*   - rewrite !merge_keys_right_identity; trivial. *)
+  (*   - apply map_eq_Equal; unfold Equal; subst; intros. *)
+  (*     unfold merge_keys. *)
+  (*     progress_fold_add1; auto. progress_fold_add1; auto. *)
+  (*     rewrite merge_keys_notation with (ks1 := ks1). *)
+  (*     rewrite merge_keys_notation with (ks2 := ks3). *)
+  (*     unfold add_key at 1; unfold add_key at 2. *)
+
+  (*     (* clean up notation of induction hypothesis *)  *)
+  (*     specialize (IHks3 ks1 ks2); unfold merge_keys in IHks3. *)
+  (*     rewrite merge_keys_notation  with (ks1 := ks1) in IHks3. *)
+  (*     rewrite merge_keys_notation  with (ks1 := ks2) in IHks3. *)
+  (*     rewrite merge_keys_notation  with (ks2 := ks3) in IHks3. *)
+  (*     rewrite merge_keys_notation  with (ks2 := ks2 $k++ ks3) in IHks3. *)
+
+  (*     rewrite merge_keys_notation with (ks1 := ks2). *)
+
+  (*     Ltac rewrite123 := *)
+  (*       match goal with | [ H : _ $k++ _ $k++ _ $? _ = _ |- _ ] => rewrite H end. *)
+
+  (*     cases (ks1 $k++ ks2 $k++ ks3 $? x); *)
+  (*       intros; subst; clean_map_lookups. *)
+
+  (*     + cases (ks2 $k++ ks3 $? x). *)
+  (*       * assert (ks1 $k++ ks2 $k++ ks3 $? x = Some k) as S by auto. *)
+  (*         rewrite IHks3 in S; eapply merge_keys_split in S; auto. *)
+  (*         cases (e ==kk k); cases (e ==kk k0); subst. *)
+  (*         ** rewrite merge_keys_notation with (ks2:=ks2$k++ks3); rewrite IHks3; trivial. *)
+  (*         ** rewrite merge_keys_notation with (ks2:=ks2 $k++ ks3 $+ (x, canonical_key k k0)). *)
+  (*            split_ors; split_ands; subst. *)
+  (*            *** rewrite Heq0 in H1; invert H1. contradiction. *)
+  (*            *** contra_map_lookup. *)
+  (*            *** destruct H0 as [k1 H0]. destruct H0 as [k2]. split_ands. rewrite Heq0 in H1; invert H1. symmetry. *)
+  (*                rewrite <- canonical_key_assoc. rewrite canonical_key_refl. *)
+  (*                cases (x ==n y); subst. *)
+  (*                  rewrite Heq. eapply merge_keys_canonicalizes'. eassumption. clean_map_lookups. reflexivity. rewrite canonical_key_assoc, canonical_key_refl; trivial. *)
+  (*                  rewrite IHks3. eapply merge_keys_inequal_addition_no_impact; assumption. *)
+  (*         ** rewrite merge_keys_notation with (ks2:=ks2$k++ks3). rewrite <- IHks3. *)
+  (*            split_ors; split_ands; subst. *)
+  (*            *** rewrite Heq0 in H1; invert H1. contradiction. *)
+  (*            *** contra_map_lookup. *)
+  (*            *** destruct H0 as [k1 H0]. destruct H0 as [k2]. split_ands. rewrite Heq0 in H1; invert H1. *)
+  (*                cases (x ==n y); subst. *)
+  (*                  rewrite canonical_key_sym, <- canonical_key_assoc, canonical_key_refl. clean_map_lookups; rewrite Heq; trivial. *)
+  (*                  clean_map_lookups; trivial. *)
+  (*         ** rewrite merge_keys_notation with (ks2:=ks2 $k++ ks3 $+ (x, canonical_key e k0)). *)
+  (*            split_ors; split_ands; subst. *)
+  (*            *** rewrite Heq0 in H1; invert H1. symmetry. *)
+  (*                cases (x ==n y); subst; clean_map_lookups. *)
+  (*                  eapply merge_keys_adds_ks2. eauto. 2:reflexivity. clean_map_lookups; trivial. *)
+  (*                  rewrite IHks3. eapply merge_keys_inequal_addition_no_impact; assumption. *)
+  (*            *** contra_map_lookup. *)
+  (*            *** destruct H0 as [k1 H0]. destruct H0 as [k2]. split_ands. rewrite Heq0 in H1; invert H1. *)
+  (*                symmetry. *)
+  (*                cases (x ==n y); subst; clean_map_lookups. *)
+  (*                **** eapply merge_keys_canonicalizes'; clean_map_lookups; eauto. *)
+  (*                     rewrite canonical_key_assoc, canonical_key_sym with (k1:=e), <- canonical_key_assoc; trivial. *)
+  (*                **** rewrite IHks3. eapply merge_keys_inequal_addition_no_impact; assumption. *)
+
+  (*       * cases (e ==kk k); subst. *)
+  (*         ** rewrite fold_add; auto. unfold add_key at 1. rewrite merge_keys_notation with (ks2:=ks2 $k++ ks3), <- IHks3. rewrite Heq. *)
+  (*            cases (k ==kk k); simpl; eauto. contradiction. *)
+  (*         ** rewrite fold_add; auto. unfold add_key at 1. rewrite merge_keys_notation with (ks2:=ks2 $k++ ks3), <- IHks3. rewrite Heq. *)
+  (*            cases (e ==kk k); simpl; eauto. contradiction. *)
+
+
+  (*     + assert (ks1 $k++ ks2 $k++ ks3 $? x = None) as HH by assumption; rewrite IHks3 in HH; eapply merge_keys_no_disappear_keys in HH; split_ands. *)
+  (*       rewrite H1. *)
+  (*       progress_fold_add1; auto. *)
+  (*       unfold add_key at 1. *)
+  (*       rewrite merge_keys_notation with (ks2:=ks2 $k++ ks3). rewrite <- IHks3. rewrite Heq; clean_map_lookups; trivial. *)
+  (* Qed. *)
+
+  (* Lemma findUserKeys_fold_fn_proper : *)
+  (*   forall {A}, *)
+  (*   Morphisms.Proper *)
+  (*     (Morphisms.respectful eq (Morphisms.respectful eq (Morphisms.respectful eq eq))) *)
+  (*     (fun (_ : NatMap.key) (u : user_data A) (ks : keys) => ks $k++ key_heap u). *)
+  (*   unfold Morphisms.Proper, Morphisms.respectful; intros; simpl; subst; trivial. *)
+  (* Qed. *)
+
+  (* Lemma findUserKeys_fold_fn_proper_Equal : *)
+  (*   forall {A}, *)
+  (*   Morphisms.Proper *)
+  (*     (Morphisms.respectful eq (Morphisms.respectful eq (Morphisms.respectful Equal Equal))) *)
+  (*     (fun (_ : NatMap.key) (u : user_data A) (ks : keys) => ks $k++ key_heap u). *)
+  (*   unfold Morphisms.Proper, Morphisms.respectful; intros. *)
+  (*   apply map_eq_Equal in H1; subst. *)
+  (*   unfold Equal; intros; trivial. *)
+  (* Qed. *)
+
+  (* Lemma findUserKeys_transpose : *)
+  (*   forall {A}, *)
+  (*     transpose_neqkey eq (fun (_ : NatMap.key) (u : user_data A) (ks : keys) => ks $k++ key_heap u). *)
+  (* Proof. *)
+  (*   unfold transpose_neqkey; intros. *)
+  (*   rewrite merge_keys_symmetric with (ks1 := a). *)
+  (*   rewrite merge_keys_symmetric with (ks1 := a $k++ key_heap e). *)
+  (*   rewrite merge_keys_assoc; trivial. *)
+  (* Qed. *)
+
+  (* Lemma findUserKeys_transpose_Equal : *)
+  (*   forall {A}, *)
+  (*     transpose_neqkey Equal (fun (_ : NatMap.key) (u : user_data A) (ks : keys) => ks $k++ key_heap u). *)
+  (* Proof. *)
+  (*   unfold transpose_neqkey; intros. *)
+  (*   unfold Equal; intros. *)
+  (*   rewrite merge_keys_symmetric with (ks1 := a). *)
+  (*   rewrite merge_keys_symmetric with (ks1 := a $k++ key_heap e). *)
+  (*   rewrite merge_keys_assoc; trivial. *)
+  (* Qed. *)
+
+  (* Hint Resolve findUserKeys_fold_fn_proper findUserKeys_fold_fn_proper_Equal findUserKeys_transpose findUserKeys_transpose_Equal. *)
 
   (* TODO move to Maps.v *)
   Lemma add_remove_eq :
@@ -1154,61 +1892,63 @@ Section KeyMergeTheorems.
     rewrite remove_neq_o; auto.
   Qed.
 
-  Lemma find_user_keys_includes_user_keys:
-    forall {A} (us : honest_users A) u_id u_d,
-      us $? u_id = Some u_d
-      -> findUserKeys us = u_d.(key_heap) $k++ findUserKeys (us $- u_id).
-  Proof.
-    unfold findUserKeys.
-    induction us using P.map_induction_bis; intros.
-    
-    - apply map_eq_Equal in H; subst; eauto.
-    - invert H.
-    - apply map_eq_Equal; unfold Equal; subst; intros.
-      simpl.
-      cases (x ==n u_id); intros; subst; clean_map_lookups.
-      + rewrite add_remove_eq.
-        rewrite fold_add; auto. rewrite remove_not_in_idempotent by assumption.
-        rewrite merge_keys_symmetric.
-        trivial.
-      + rewrite add_remove_neq by assumption.
-        rewrite !fold_add; auto.
-        rewrite <- merge_keys_assoc.
-        erewrite IHus; eauto.
-        rewrite not_find_in_iff; rewrite remove_neq_o; auto.
-  Qed.
+  (* Lemma find_user_keys_includes_user_keys: *)
+  (*   forall {A} (us : honest_users A) u_id u_d, *)
+  (*     us $? u_id = Some u_d *)
+  (*     -> findUserKeys us = u_d.(key_heap) $k++ findUserKeys (us $- u_id). *)
+  (* Proof. *)
+  (*   unfold findUserKeys. *)
+  (*   induction us using P.map_induction_bis; intros. *)
 
-  Lemma find_user_keys_universe_user :
-    forall {A B} (U : universe A B) u_id u_d,
-        adv_no_honest_keys U.(adversary).(key_heap) (findUserKeys U.(users))
-      -> U.(users) $? u_id = Some u_d
-      -> key_heaps_compatible U.(adversary).(key_heap) (findUserKeys U.(users))
-      -> adv_no_honest_keys U.(adversary).(key_heap) u_d.(key_heap).
-  Proof.
-  Admitted.
+  (*   - apply map_eq_Equal in H; subst; eauto. *)
+  (*   - invert H. *)
+  (*   - apply map_eq_Equal; unfold Equal; subst; intros. *)
+  (*     simpl. *)
+  (*     cases (x ==n u_id); intros; subst; clean_map_lookups. *)
+  (*     + rewrite add_remove_eq. *)
+  (*       rewrite fold_add; auto. rewrite remove_not_in_idempotent by assumption. *)
+  (*       rewrite merge_keys_symmetric. *)
+  (*       trivial. *)
+  (*     + rewrite add_remove_neq by assumption. *)
+  (*       rewrite !fold_add; auto. *)
+  (*       rewrite <- merge_keys_assoc. *)
+  (*       erewrite IHus; eauto. *)
+  (*       rewrite not_find_in_iff; rewrite remove_neq_o; auto. *)
+  (* Qed. *)
+
+  (* Lemma find_user_keys_universe_user : *)
+  (*   forall {A B} (U : universe A B) u_id u_d, *)
+  (*       adv_no_honest_keys U.(adversary).(key_heap) (findUserKeys U.(users)) *)
+  (*     -> U.(users) $? u_id = Some u_d *)
+  (*     -> key_heaps_compatible U.(adversary).(key_heap) (findUserKeys U.(users)) *)
+  (*     -> adv_no_honest_keys U.(adversary).(key_heap) u_d.(key_heap). *)
+  (* Proof. *)
+  (* Admitted. *)
 
 End KeyMergeTheorems.
 
-Definition encryptMessage {t} (k__sign k__enc : key) (m : message t) (c_id : cipher_id) : option cipher :=
-  match (k__sign.(keyUsage), k__enc.(keyUsage)) with
-  | (Signing, Encryption) =>
-    let c := SigEncCipher c_id k__sign.(keyId) k__enc.(keyId) m
-    in  match k__sign with
-        | MkCryptoKey _ _ SymKey         => Some c
-        | MkCryptoKey _ _ (AsymKey true) => Some c
-        | _       => None
-        end
-  | _          => None
+Definition sign_if_ok (c : cipher) (kt : key_type) (k : key_permission) : option cipher :=
+  match (kt,k) with
+  | (SymKey,  MkKeyPerm _ _)      => Some c
+  | (AsymKey, MkKeyPerm _ true)   => Some c
+  | (AsymKey, MkKeyPerm _ false)  => None
   end.
 
-Definition signMessage {t} (k : key) (m : message t) (c_id : cipher_id) : option cipher :=
-  match k with
-  | MkCryptoKey _ Signing SymKey         => Some (SigCipher c_id k.(keyId) m)
-  | MkCryptoKey _ Signing (AsymKey true) => Some (SigCipher c_id k.(keyId) m)
-  | _       => None
+Definition encryptMessage {t} (ks : keys) (k__sign k__enc : key_permission) (m : message t) (c_id : cipher_id) : option cipher :=
+  match (ks $? k__sign.(key_ref), ks $? k__enc.(key_ref)) with
+  | (Some (MkCryptoKey _ Signing kt__sign), Some (MkCryptoKey _ Encryption kt__enc)) =>
+    sign_if_ok (SigEncCipher c_id k__sign.(key_ref) k__enc.(key_ref) m) kt__sign k__sign
+  | _ => None
   end.
 
-Definition canVerifySignature {A} (cs : ciphers)(usrDat : user_data A)(c_id : cipher_id) : Prop :=
+Definition signMessage {t} (ks : keys) (k : key_permission) (m : message t) (c_id : cipher_id) : option cipher :=
+  match (ks $? k.(key_ref)) with
+  | Some (MkCryptoKey _ Signing kt)     =>
+    sign_if_ok (SigCipher c_id k.(key_ref) m) kt k
+  | _ => None
+  end.
+
+Definition canVerifySignature {A} (cs : ciphers) (usrDat : user_data A) (c_id : cipher_id) : Prop :=
   forall t (m : message t) k_id k ,
     cs $? c_id = Some (SigCipher c_id k_id m)
     (*  Make sure that the user has access to the key.  If we are doing asymmetric signatures,
@@ -1216,19 +1956,21 @@ Definition canVerifySignature {A} (cs : ciphers)(usrDat : user_data A)(c_id : ci
     /\ usrDat.(key_heap) $? k_id = Some k.
 
 Definition buildUniverse {A B}
-           (usrs : honest_users A) (adv : user_data B) (cs : ciphers)
+           (usrs : honest_users A) (adv : user_data B) (cs : ciphers) (ks : keys)
            (u_id : user_id) (userData : user_data A) : universe A B :=
   {| users        := usrs $+ (u_id, userData)
    ; adversary    := adv
    ; all_ciphers  := cs
+   ; all_keys     := ks
    |}.
 
 Definition buildUniverseAdv {A B}
-           (usrs : honest_users A) (cs : ciphers)
+           (usrs : honest_users A) (cs : ciphers) (ks : keys)
            (userData : user_data B) : universe A B :=
   {| users        := usrs
    ; adversary    := userData
    ; all_ciphers  := cs
+   ; all_keys     := ks
    |}.
 
 Definition extractPlainText {t} (msg : message t) : option nat :=
@@ -1257,64 +1999,63 @@ Definition unSig {t} (msg : message t) : option (message t) :=
 
 
 Inductive action : Type :=
-| Input  t (msg : message t) (pat : msg_pat) (uks : keys)
+| Input  t (msg : message t) (pat : msg_pat) (uks : key_perms)
 | Output t (msg : message t)
 .
 
 Definition rlabel := @label action.
 
-Definition action_adversary_safe (honestk advk : keys) (a : action) : bool :=
+Definition action_adversary_safe (all_keys : keys) (honestk advk : key_perms) (a : action) : bool :=
   match a with
-  | Input _ pat _ => negb (msg_pattern_spoofable honestk advk pat)
+  | Input _ pat _ => negb (msg_pattern_spoofable all_keys honestk pat)
   | Output _      => true
   end.
 
 Definition data_step0 (A B C : Type) : Type :=
-  honest_users A * user_data B * ciphers * keys * queued_messages * user_cmd C.
+  honest_users A * user_data B * ciphers * keys * key_perms * queued_messages * user_cmd C.
 
 Definition build_data_step {A B C} (U : universe A B) (u_data : user_data C) : data_step0 A B C :=
-  (U.(users), U.(adversary), U.(all_ciphers), u_data.(key_heap), u_data.(msg_heap), u_data.(protocol)).
+  (U.(users), U.(adversary), U.(all_ciphers), U.(all_keys), u_data.(key_heap), u_data.(msg_heap), u_data.(protocol)).
 
 (* Labeled transition system *)
-Print sigT.
 
 Inductive step_user : forall A B C, rlabel -> data_step0 A B C -> data_step0 A B C -> Prop :=
 
 (* Plumbing *)
 | StepBindRecur : forall {B r r'} (usrs usrs' : honest_users r') (adv adv' : user_data B)
-                     lbl cs cs' qmsgs qmsgs' ks ks' (cmd1 cmd1' : user_cmd r) (cmd2 : r -> user_cmd r'),
-      step_user lbl (usrs, adv, cs, ks, qmsgs, cmd1) (usrs', adv', cs', ks', qmsgs', cmd1')
-    -> step_user lbl (usrs, adv, cs, ks, qmsgs, Bind cmd1 cmd2) (usrs', adv', cs', ks', qmsgs', Bind cmd1' cmd2)
-| StepBindProceed : forall {B r r'} (usrs : honest_users r) (adv : user_data B) cs ks qmsgs (v : r') (cmd : r' -> user_cmd r),
-    step_user Silent (usrs, adv, cs, ks, qmsgs, Bind (Return v) cmd) (usrs, adv, cs, ks, qmsgs, cmd v)
+                     lbl cs cs' qmsgs qmsgs' gks gks' ks ks' (cmd1 cmd1' : user_cmd r) (cmd2 : r -> user_cmd r'),
+      step_user lbl (usrs, adv, cs, gks, ks, qmsgs, cmd1) (usrs', adv', cs', gks', ks', qmsgs', cmd1')
+    -> step_user lbl (usrs, adv, cs, gks, ks, qmsgs, Bind cmd1 cmd2) (usrs', adv', cs', gks', ks', qmsgs', Bind cmd1' cmd2)
+| StepBindProceed : forall {B r r'} (usrs : honest_users r) (adv : user_data B) cs gks ks qmsgs (v : r') (cmd : r' -> user_cmd r),
+    step_user Silent (usrs, adv, cs, gks, ks, qmsgs, Bind (Return v) cmd) (usrs, adv, cs, gks, ks, qmsgs, cmd v)
 
-| StepGen : forall {A B} (usrs : honest_users A) (adv : user_data B) cs ks qmsgs n,
-    step_user Silent (usrs, adv, cs, ks, qmsgs, Gen) (usrs, adv, cs, ks, qmsgs, Return n)
+| StepGen : forall {A B} (usrs : honest_users A) (adv : user_data B) cs gks ks qmsgs n,
+    step_user Silent (usrs, adv, cs, gks, ks, qmsgs, Gen) (usrs, adv, cs, gks, ks, qmsgs, Return n)
 
 (* Comms  *)
-| StepRecv : forall {A B} {t} (usrs : honest_users A) (adv : user_data B) cs ks ks' qmsgs qmsgs' (msg : message t) msgs pat newkeys,
+| StepRecv : forall {A B} {t} (usrs : honest_users A) (adv : user_data B) cs gks ks ks' qmsgs qmsgs' (msg : message t) msgs pat newkeys,
       qmsgs = (existT _ _ msg) :: msgs (* we have a message waiting for us! *)
     -> qmsgs' = msgs
     -> findKeys msg = newkeys
     -> ks' = ks $k++ newkeys
     -> msg_accepted_by_pattern cs pat msg
     -> step_user (Action (Input msg pat ks))
-                (usrs, adv, cs, ks , qmsgs , Recv pat)
-                (usrs, adv, cs, ks', qmsgs', Return msg)
+                (usrs, adv, cs, gks, ks , qmsgs , Recv pat)
+                (usrs, adv, cs, gks, ks', qmsgs', Return msg)
 
-| StepRecvDrop : forall {A B} {t} (usrs : honest_users A) (adv : user_data B) cs ks qmsgs qmsgs' (msg : message t) pat msgs,
+| StepRecvDrop : forall {A B} {t} (usrs : honest_users A) (adv : user_data B) cs gks ks qmsgs qmsgs' (msg : message t) pat msgs,
       qmsgs = (existT _ _ msg) :: msgs (* we have a message waiting for us! *)
     -> qmsgs' = msgs
     -> ~ msg_accepted_by_pattern cs pat msg
     -> step_user Silent (* Error label ... *)
-                (usrs, adv, cs, ks, qmsgs , Recv pat)
-                (usrs, adv, cs, ks, qmsgs', Return msg)
+                (usrs, adv, cs, gks, ks, qmsgs , Recv pat)
+                (usrs, adv, cs, gks, ks, qmsgs', Return msg)
 
 (* Augment attacker's keys with those available through messages sent,
  * including traversing through ciphers already known by attacker, etc.
  *)
 | StepSend : forall {A B} {t} (usrs usrs' : honest_users A) (adv adv' : user_data B)
-               cs ks qmsgs rec_u_id rec_u newkeys (msg : message t),
+               cs gks ks qmsgs rec_u_id rec_u newkeys (msg : message t),
     findKeys msg = newkeys
     -> adv' = addUserKeys newkeys adv
     -> usrs $? rec_u_id = Some rec_u
@@ -1322,55 +2063,58 @@ Inductive step_user : forall A B C, rlabel -> data_step0 A B C -> data_step0 A B
                                   ; protocol := rec_u.(protocol) 
                                   ; msg_heap := rec_u.(msg_heap) ++ [existT _ _ msg]  |})
     -> step_user (Action (Output msg))
-                (usrs , adv , cs, ks, qmsgs, Send rec_u_id msg)
-                (usrs', adv', cs, ks, qmsgs, Return tt)
+                (usrs , adv , cs, gks, ks, qmsgs, Send rec_u_id msg)
+                (usrs', adv', cs, gks, ks, qmsgs, Return tt)
 
 (* Encryption / Decryption *)
-| StepEncrypt : forall {A B} {t} (usrs : honest_users A) (adv : user_data B) cs cs' ks qmsgs (msg : message t) k__sign k__enc k__signid k__encid c_id cipherMsg,
-      keyId k__sign = k__signid
-    -> keyId k__enc = k__encid
+| StepEncrypt : forall {A B} {t} (usrs : honest_users A) (adv : user_data B) cs cs' gks ks qmsgs (msg : message t) k__sign k__enc k__signid k__encid c_id cipherMsg,
+      key_ref k__sign = k__signid
+    -> key_ref k__enc = k__encid
     -> ks $? k__signid = Some k__sign
+    -> has_private_key gks k__sign = true
     -> ks $? k__encid = Some k__enc
     -> ~ In c_id cs
-    -> encryptMessage k__sign k__enc msg c_id = Some cipherMsg
+    -> encryptMessage gks k__sign k__enc msg c_id = Some cipherMsg
     -> cs' = cs $+ (c_id, cipherMsg)
     -> step_user Silent
-                (usrs, adv, cs , ks, qmsgs, SignEncrypt k__sign k__enc msg)
-                (usrs, adv, cs', ks, qmsgs, Return (SignedCiphertext c_id))
+                (usrs, adv, cs , gks, ks, qmsgs, SignEncrypt k__sign k__enc msg)
+                (usrs, adv, cs', gks, ks, qmsgs, Return (SignedCiphertext c_id))
 
-| StepDecrypt : forall {A B} {t} (usrs : honest_users A) (adv : user_data B) cs ks ks' qmsgs (msg : message t) k__signid k__sign k__encid c_id newkeys,
+| StepDecrypt : forall {A B} {t} (usrs : honest_users A) (adv : user_data B) cs gks ks ks' qmsgs (msg : message t) k__signid k__sign k__encid c_id newkeys kt b,
       cs $? c_id = Some (SigEncCipher c_id k__signid k__encid msg)
-    -> ( ks $? k__encid = Some (MkCryptoKey k__encid Encryption (AsymKey true)) (* check we have access to private key *)
-      \/ ks $? k__encid = Some (MkCryptoKey k__encid Encryption SymKey) )
+    -> ( (gks $? k__encid = Some (MkCryptoKey k__encid Encryption SymKey)  /\ ks $? k__encid = Some (MkKeyPerm k__encid b))
+      \/ (gks $? k__encid = Some (MkCryptoKey k__encid Encryption AsymKey) /\ ks $? k__encid = Some (MkKeyPerm k__encid true))
+      )
+    -> gks $? k__signid = Some (MkCryptoKey k__signid Signing kt)
     -> ks $? k__signid = Some k__sign
-    (* -> k.(keyId) = k_id *)
     -> findKeys msg = newkeys
     -> ks' = ks $k++ newkeys
     -> step_user Silent
-                (usrs, adv, cs, ks , qmsgs, Decrypt (SignedCiphertext c_id))
-                (usrs, adv, cs, ks', qmsgs, Return msg)
+                (usrs, adv, cs, gks, ks , qmsgs, Decrypt (SignedCiphertext c_id))
+                (usrs, adv, cs, gks, ks', qmsgs, Return msg)
 
 (* Signing / Verification *)
-| StepSign : forall {A B} {t} (usrs : honest_users A) (adv : user_data B) cs cs' ks qmsgs (msg : message t) k k_id c_id cipherMsg,
-      keyId k = k_id
+| StepSign : forall {A B} {t} (usrs : honest_users A) (adv : user_data B) cs cs' gks ks qmsgs (msg : message t) k k_id c_id cipherMsg,
+      key_ref k = k_id
     -> ks $? k_id = Some k
+    -> has_private_key gks k = true
     -> ~(In c_id cs)
-    -> signMessage k msg c_id = Some cipherMsg
+    -> signMessage gks k msg c_id = Some cipherMsg
     -> cs' = cs $+ (c_id, cipherMsg)
     -> step_user Silent
-                (usrs, adv, cs , ks, qmsgs, Sign k msg)
-                (usrs, adv, cs', ks, qmsgs, Return (Signature msg c_id))
+                (usrs, adv, cs , gks, ks, qmsgs, Sign k msg)
+                (usrs, adv, cs', gks, ks, qmsgs, Return (Signature msg c_id))
 
-| StepVerify : forall {A B} {t} (usrs : honest_users A) (adv : user_data B) cs ks qmsgs (msg : message t) k_id k c_id,
-    keyId k = k_id
+| StepVerify : forall {A B} {t} (usrs : honest_users A) (adv : user_data B) cs gks ks qmsgs (msg : message t) k_id k c_id,
+    key_ref k = k_id
     (* k is in your key heap *)
-    -> ks $? (keyId k) = Some k
+    -> ks $? (key_ref k) = Some k
     (* return true or false whether k was used to sign the message *)
     -> cs $? c_id = Some (SigCipher c_id k_id msg)
     (* -> findKeys msg = newkeys *)
     -> step_user Silent
-                (usrs, adv, cs, ks, qmsgs, (Verify k (Signature msg c_id)))
-                (usrs, adv, cs, ks, qmsgs, Return true)
+                (usrs, adv, cs, gks, ks, qmsgs, (Verify k (Signature msg c_id)))
+                (usrs, adv, cs, gks, ks, qmsgs, Return true)
                 (* (usrs, adv, cs, ks, qmsgs, Return (if (k_id ==n (keyId k)) then true else false)) *)
 .
 
@@ -1402,17 +2146,17 @@ Inductive step_user : forall A B C, rlabel -> data_step0 A B C -> data_step0 A B
 (* Qed. *)
 
 Inductive step_universe {A B} : universe A B -> rlabel -> universe A B -> Prop :=
-| StepUser : forall U U' u_id userData usrs adv cs ks qmsgs lbl (cmd : user_cmd A),
+| StepUser : forall U U' u_id userData usrs adv cs gks ks qmsgs lbl (cmd : user_cmd A),
     U.(users) $? u_id = Some userData
     -> step_user lbl
                 (build_data_step U userData)
-                (usrs, adv, cs, ks, qmsgs, cmd)
-    -> U' = buildUniverse usrs adv cs u_id {| key_heap := ks ; msg_heap := qmsgs ; protocol := cmd |}
+                (usrs, adv, cs, gks, ks, qmsgs, cmd)
+    -> U' = buildUniverse usrs adv cs gks u_id {| key_heap := ks ; msg_heap := qmsgs ; protocol := cmd |}
     -> step_universe U lbl U'
-| StepAdversary : forall U U' usrs adv cs ks qmsgs lbl (cmd : user_cmd B),
+| StepAdversary : forall U U' usrs adv cs gks ks qmsgs lbl (cmd : user_cmd B),
       step_user lbl
                 (build_data_step U U.(adversary))
-                (usrs, adv, cs, ks, qmsgs, cmd)
-    -> U' = buildUniverseAdv usrs cs {| key_heap := adv.(key_heap) $k++ ks ; msg_heap := qmsgs ; protocol := cmd |}
+                (usrs, adv, cs, gks, ks, qmsgs, cmd)
+    -> U' = buildUniverseAdv usrs cs gks {| key_heap := adv.(key_heap) $k++ ks ; msg_heap := qmsgs ; protocol := cmd |}
     -> step_universe U Silent U'
 .
