KeyManagement/Simulation.v
@@ -5,8 +5,7 @@ From Coq Require Import
      Program.Equality (* for dependent induction *)
 .
 
-
-Require Import MyPrelude Maps Common MapLtac. 
+Require Import MyPrelude Maps Common MapLtac.
 
 Require IdealWorld
         RealWorld.
@@ -75,8 +74,9 @@ Definition simulates {A B : Type}
 
   (forall U__r U__i,
       R U__r U__i
-      -> RealWorld.key_heaps_compatible (RealWorld.findUserKeys U__r.(RealWorld.users)) U__r.(RealWorld.adversary).(RealWorld.key_heap)
-      -> RealWorld.adv_no_honest_keys U__r.(RealWorld.adversary).(RealWorld.key_heap) (RealWorld.findUserKeys U__r.(RealWorld.users))
+      -> RealWorld.keys_good U__r.(RealWorld.all_keys)
+      -> RealWorld.all_user_key_perms_good U__r.(RealWorld.users)
+      -> RealWorld.adv_no_honest_keys U__r.(RealWorld.all_keys) U__r.(RealWorld.adversary).(RealWorld.key_heap) (RealWorld.findUserKeys U__r.(RealWorld.users))
       -> forall U__r',
           rstepSilent U__r U__r'
           -> exists U__i',
@@ -85,8 +85,9 @@ Definition simulates {A B : Type}
 
 /\ (forall U__r U__i,
       R U__r U__i
-      -> RealWorld.key_heaps_compatible (RealWorld.findUserKeys U__r.(RealWorld.users)) U__r.(RealWorld.adversary).(RealWorld.key_heap)
-      -> RealWorld.adv_no_honest_keys U__r.(RealWorld.adversary).(RealWorld.key_heap) (RealWorld.findUserKeys U__r.(RealWorld.users))
+      -> RealWorld.keys_good U__r.(RealWorld.all_keys)
+      -> RealWorld.all_user_key_perms_good U__r.(RealWorld.users)
+      -> RealWorld.adv_no_honest_keys U__r.(RealWorld.all_keys) U__r.(RealWorld.adversary).(RealWorld.key_heap) (RealWorld.findUserKeys U__r.(RealWorld.users))
       -> forall a1 U__r',
           RealWorld.step_universe U__r (Action a1) U__r' (* excludes adversary steps *)
           -> exists a2 U__i' U__i'',
@@ -94,14 +95,15 @@ Definition simulates {A B : Type}
             /\ IdealWorld.lstep_universe U__i' (Action a2) U__i''
             /\ action_matches a1 a2
             /\ R U__r' U__i''
-            /\ RealWorld.action_adversary_safe (RealWorld.findUserKeys U__r.(RealWorld.users)) U__r.(RealWorld.adversary).(RealWorld.key_heap) a1 = true
-            /\ RealWorld.adv_no_honest_keys U__r'.(RealWorld.adversary).(RealWorld.key_heap) (RealWorld.findUserKeys U__r'.(RealWorld.users))
+            /\ RealWorld.action_adversary_safe U__r.(RealWorld.all_keys) (RealWorld.findUserKeys U__r.(RealWorld.users)) U__r.(RealWorld.adversary).(RealWorld.key_heap) a1 = true
+            /\ RealWorld.adv_no_honest_keys U__r'.(RealWorld.all_keys) U__r'.(RealWorld.adversary).(RealWorld.key_heap) (RealWorld.findUserKeys U__r'.(RealWorld.users))
   (* and adversary couldn't have constructed message seen in a1 *)
   )
 
 /\ R U__r U__i
-/\ RealWorld.key_heaps_compatible (RealWorld.findUserKeys U__r.(RealWorld.users)) U__r.(RealWorld.adversary).(RealWorld.key_heap)
-/\ RealWorld.adv_no_honest_keys U__r.(RealWorld.adversary).(RealWorld.key_heap) (RealWorld.findUserKeys U__r.(RealWorld.users))
+/\ RealWorld.keys_good U__r.(RealWorld.all_keys)
+/\ RealWorld.all_user_key_perms_good U__r.(RealWorld.users)
+/\ RealWorld.adv_no_honest_keys U__r.(RealWorld.all_keys) U__r.(RealWorld.adversary).(RealWorld.key_heap) (RealWorld.findUserKeys U__r.(RealWorld.users))
 .
 
 
@@ -138,64 +140,73 @@ Section SingleAdversarySimulates.
   Section AdversaryHelpers.
     Import RealWorld.
 
+    Variable global_keys : keys.
+    Variable honestk advk : key_perms.
+
     Definition add_adversary {A B} (U__r : universe A B) (advcode : user_cmd B) :=
       {| users       := U__r.(users)
        ; adversary   := {| key_heap := $0
                          ; msg_heap := []
                          ; protocol := advcode |}
        ; all_ciphers := U__r.(all_ciphers)
+       ; all_keys    := U__r.(all_keys)
       |}.
 
-    Fixpoint msg_safe {t} (honestk advk : keys) (msg : message t) : bool :=
+    Fixpoint msg_safe {t} (cs : ciphers) (msg : message t) : bool :=
       match msg with
       | Plaintext _ => false
       | KeyMessage _ => false
-      | MsgPair m1 m2 => msg_safe honestk advk m1 && msg_safe honestk advk m2
-      | SignedCiphertext _ => true
-      | Signature _ _ => true
+      | MsgPair m1 m2 => msg_safe cs m1 && msg_safe cs m2
+      | SignedCiphertext c_id =>
+        match cs $? c_id with
+        | None   => false
+        | Some c => honest_signing_key global_keys honestk (cipher_signing_key c)
+        end
+      | Signature _ c_id =>
+        match cs $? c_id with
+        | None   => false
+        | Some c => honest_signing_key global_keys honestk (cipher_signing_key c)
+        end
       end.
     
-    Fixpoint msg_filter (honestk advk : keys) (sigM : { t & message t } ) : bool :=
+    Fixpoint msg_filter (cs : ciphers) (sigM : { t & message t } ) : bool :=
       match sigM with
-      | existT _ _ msg => msg_safe honestk advk msg
+      | existT _ _ msg => msg_safe cs msg
       end.
 
-    Definition clean_messages (honestk advk : keys) (msgs : queued_messages) :=
-      List.filter (msg_filter honestk advk) msgs.
+    Definition clean_messages (cs : ciphers) (msgs : queued_messages) :=
+      List.filter (msg_filter cs) msgs.
 
-    Definition clean_users {A} (honestk advk : keys) (usrs : honest_users A) :=
+    Definition clean_users {A} (cs : ciphers) (usrs : honest_users A) :=
       (* usrs. *)
       map (fun u_d => {| key_heap := u_d.(key_heap)
                     ; protocol := u_d.(protocol)
-                    ; msg_heap := clean_messages honestk advk u_d.(msg_heap) |}) usrs.
+                    ; msg_heap := clean_messages cs u_d.(msg_heap) |}) usrs.
 
-    Definition honest_cipher_filter_fn (honestk advk : keys) (c_id : cipher_id) (c : cipher) :=
+    Definition honest_cipher_filter_fn (c_id : cipher_id) (c : cipher) :=
       match c with
-      | SigCipher _ k_id _          => honest_signing_key honestk advk k_id
-      | SigEncCipher _ k__sign k__enc _ => honest_signing_key honestk advk k__sign
+      | SigCipher _ k_id _          => honest_signing_key global_keys honestk k_id
+      | SigEncCipher _ k__sign k__enc _ => honest_signing_key global_keys honestk k__sign
       end.
 
     Lemma honest_cipher_filter_fn_proper :
-      forall honestk advk,
-        Proper (eq  ==>  eq  ==>  eq) (honest_cipher_filter_fn honestk advk).
+      Proper (eq  ==>  eq  ==>  eq) honest_cipher_filter_fn.
     Proof.
       unfold Proper, Morphisms.respectful; intros; subst; reflexivity.
     Qed.
 
     Lemma honest_cipher_filter_fn_filter_proper :
-      forall honestk advk,
-        Proper
-          ( eq  ==>  eq  ==>  Equal  ==>  Equal)
-          (fun (k : NatMap.key) (e : cipher) (m : t cipher) => if honest_cipher_filter_fn honestk advk k e then m $+ (k, e) else m).
+      Proper
+        ( eq  ==>  eq  ==>  Equal  ==>  Equal)
+        (fun (k : NatMap.key) (e : cipher) (m : t cipher) => if honest_cipher_filter_fn k e then m $+ (k, e) else m).
     Proof.
       unfold Proper, respectful;
-      unfold Equal; intros; apply map_eq_Equal in H1; subst; auto.
+        unfold Equal; intros; apply map_eq_Equal in H1; subst; auto.
     Qed.
 
     Lemma honest_cipher_filter_fn_filter_transpose :
-      forall honestk advk,
-        transpose_neqkey Equal
-          (fun (k : NatMap.key) (e : cipher) (m : t cipher) => if honest_cipher_filter_fn honestk advk k e then m $+ (k, e) else m).
+      transpose_neqkey Equal
+        (fun (k : NatMap.key) (e : cipher) (m : t cipher) => if honest_cipher_filter_fn k e then m $+ (k, e) else m).
     Proof.
       unfold transpose_neqkey, Equal, honest_cipher_filter_fn; intros.
       cases e; cases e'; simpl.
@@ -213,40 +224,33 @@ Section SingleAdversarySimulates.
         | [ H : ~ In _ _ |- _ ] => rewrite not_find_in_iff in H
         end.
 
-      cases (honest_signing_key honestk advk k_id); cases (honest_signing_key honestk advk k_id0); eauto.
+      cases (honest_signing_key global_keys honestk k_id); cases (honest_signing_key global_keys honestk k_id0); eauto.
         cases (y ==n k); cases (y ==n k'); subst; repeat clean_map_lookups1; try contradiction; eauto.
-      cases (honest_signing_key honestk advk k_id); cases (honest_signing_key honestk advk k__sign); eauto.
+      cases (honest_signing_key global_keys honestk k_id); cases (honest_signing_key global_keys honestk k__sign); eauto.
         cases (y ==n k); cases (y ==n k'); subst; repeat clean_map_lookups1; try contradiction; eauto.
-      cases (honest_signing_key honestk advk k_id); cases (honest_signing_key honestk advk k__sign); eauto.
+      cases (honest_signing_key global_keys honestk k_id); cases (honest_signing_key global_keys honestk k__sign); eauto.
         cases (y ==n k); cases (y ==n k'); subst; repeat clean_map_lookups1; try contradiction; eauto.
-      cases (honest_signing_key honestk advk k__sign); cases (honest_signing_key honestk advk k__sign0); eauto.
+      cases (honest_signing_key global_keys honestk k__sign); cases (honest_signing_key global_keys honestk k__sign0); eauto.
         cases (y ==n k); cases (y ==n k'); subst; repeat clean_map_lookups1; try contradiction; eauto.
     Qed.
 
-    (* Lemma merge_maps_proper : *)
-    (*   forall {B}, *)
-    (*     Proper (eq  ==>  eq  ==>  eq  ==>  eq) *)
-    (*       (fun (k: NatMap.key) (u : user_data B) (ks : t key) => ks $++ key_heap u). *)
-    (* Proof. *)
-    (*   unfold Proper, respectful; intros; subst; trivial. *)
-    (* Qed. *)
-
-    Definition clean_ciphers (honestk advk : keys) (cs : ciphers) :=
-      filter (honest_cipher_filter_fn honestk advk) cs.
-
-    Definition strip_adversary {A B} (U__r : universe A B) (b : B) : universe A B :=
-      let honestk := findUserKeys U__r.(users)
-      in {| users       := clean_users honestk U__r.(adversary).(key_heap) U__r.(users)
-          ; adversary   := {| key_heap := $0
-                            ; msg_heap := []
-                            ; protocol := Return b |}
-          ; all_ciphers := clean_ciphers honestk U__r.(adversary).(key_heap) U__r.(all_ciphers)
-         |}.
+    Definition clean_ciphers (cs : ciphers) :=
+      filter honest_cipher_filter_fn cs.
 
   End AdversaryHelpers.
 
   Section RealWorldLemmas.
     Import RealWorld.
+
+    Definition strip_adversary {A B} (U__r : universe A B) (b : B) : universe A B :=
+      let honestk := findUserKeys U__r.(users)
+      in {| users       := clean_users U__r.(all_keys) (findUserKeys U__r.(users)) U__r.(all_ciphers) U__r.(users)
+          ; adversary   := {| key_heap := $0
+                            ; msg_heap := []
+                            ; protocol := Return b |}
+          ; all_ciphers := clean_ciphers U__r.(all_keys) honestk U__r.(all_ciphers)
+          ; all_keys    := U__r.(all_keys)
+         |}.
 
     Hint Resolve
          honest_cipher_filter_fn_proper
@@ -258,6 +262,7 @@ Section SingleAdversarySimulates.
         {| users       := users U__r
          ; adversary   := adversary U__r
          ; all_ciphers := all_ciphers U__r
+         ; all_keys    := all_keys U__r
         |} = U__r.
       intros. destruct U__r; simpl; trivial.
     Qed.
@@ -277,18 +282,18 @@ Section SingleAdversarySimulates.
       eexists; intuition. eassumption.
     Qed.
 
-    Lemma clean_ciphers_mapsto_iff : forall honestk advk cs c_id c,
-        MapsTo c_id c (clean_ciphers honestk advk cs) <-> MapsTo c_id c cs /\ honest_cipher_filter_fn honestk advk c_id c = true.
+    Lemma clean_ciphers_mapsto_iff : forall allks honestk cs c_id c,
+        MapsTo c_id c (clean_ciphers allks honestk cs) <-> MapsTo c_id c cs /\ honest_cipher_filter_fn allks honestk c_id c = true.
     Proof.
       intros.
       apply filter_iff; eauto.
-      Qed.
+    Qed.
     
     Lemma clean_ciphers_keeps_honest_cipher :
-      forall c_id c honestk advk cs,
+      forall c_id c allks honestk cs,
         cs $? c_id = Some c
-        -> honest_cipher_filter_fn honestk advk c_id c = true
-        -> clean_ciphers honestk advk cs $? c_id = Some c.
+        -> honest_cipher_filter_fn allks honestk c_id c = true
+        -> clean_ciphers allks honestk cs $? c_id = Some c.
     Proof.
       intros.
       rewrite <- find_mapsto_iff.
@@ -297,8 +302,8 @@ Section SingleAdversarySimulates.
     Qed.
 
     Lemma clean_ciphers_accepts :
-      forall {t} honestk advk cs p (m : message t),
-          msg_accepted_by_pattern (clean_ciphers honestk advk cs) p m
+      forall {t} allks honestk cs p (m : message t),
+          msg_accepted_by_pattern (clean_ciphers allks honestk cs) p m
         -> msg_accepted_by_pattern cs p m.
     Proof.
       induction 1; intros; subst; eauto.
@@ -313,11 +318,11 @@ Section SingleAdversarySimulates.
     Qed.
 
     Lemma honest_signing_key_not_cleaned :
-      forall cs c_id c honestk advks k,
+      forall cs c_id c allks honestk k,
         cs $? c_id = Some c
-        -> honest_signing_key honestk advks k = true
+        -> honest_signing_key allks honestk k = true
         -> k = cipher_signing_key c
-        -> clean_ciphers honestk advks cs $? c_id = Some c.
+        -> clean_ciphers allks honestk cs $? c_id = Some c.
     Proof.
       intros.
       eapply clean_ciphers_keeps_honest_cipher; auto.
@@ -327,12 +332,12 @@ Section SingleAdversarySimulates.
     Qed.
 
     Lemma clean_ciphers_accepts_non_spoofable :
-      forall {t} honestk advks cs p (m : message t),
+      forall {t} allks honestk cs p (m : message t),
         msg_accepted_by_pattern cs p m
         -> forall p',
           p' = p
-        -> msg_pattern_spoofable honestk advks p' = false
-        -> msg_accepted_by_pattern (clean_ciphers honestk advks cs) p' m.
+        -> msg_pattern_spoofable allks honestk p' = false
+        -> msg_accepted_by_pattern (clean_ciphers allks honestk cs) p' m.
     Proof.
       induction 1; intros; subst; eauto.
       - econstructor; auto.
@@ -349,9 +354,9 @@ Section SingleAdversarySimulates.
     Hint Constructors msg_accepted_by_pattern.
 
     Lemma clean_ciphers_doesn't_make_unaccepted_msg_accepted :
-      forall {t} cs pat honestk advk (msg : message t),
+      forall {t} cs pat allks honestk (msg : message t),
           ~ msg_accepted_by_pattern cs pat msg
-        -> ~ msg_accepted_by_pattern (clean_ciphers honestk advk cs) pat msg.
+        -> ~ msg_accepted_by_pattern (clean_ciphers allks honestk cs) pat msg.
     Proof.
       unfold "~"; induction 2; subst;
         eauto;
@@ -367,15 +372,15 @@ Section SingleAdversarySimulates.
     Hint Extern 1 (_ $+ (?k, _) $? ?v = _) => rewrite add_neq_o.
 
     Lemma clean_ciphers_eliminates_dishonest_cipher :
-      forall c_id c honestk advk cs k,
+      forall c_id c allks honestk cs k,
         cs $? c_id = Some c
-        -> honest_signing_key honestk advk k = false
+        -> honest_signing_key allks honestk k = false
         -> k = cipher_signing_key c
-        -> clean_ciphers honestk advk cs $? c_id = None.
+        -> clean_ciphers allks honestk cs $? c_id = None.
     Proof.
       intros; unfold clean_ciphers, filter.
       apply P.fold_rec_bis; intros; eauto.
-      cases (honest_cipher_filter_fn honestk advk k0 e); eauto.
+      cases (honest_cipher_filter_fn allks honestk k0 e); eauto.
       cases (c_id ==n k0); subst; eauto.
       exfalso.
       rewrite find_mapsto_iff in H2; rewrite H2 in H; invert H.
@@ -387,15 +392,15 @@ Section SingleAdversarySimulates.
     Hint Resolve clean_ciphers_eliminates_dishonest_cipher clean_ciphers_keeps_honest_cipher.
 
     Lemma clean_ciphers_reduces_or_keeps_same_ciphers :
-      forall c_id c honestk advk cs,
+      forall c_id c allks honestk cs,
         cs $? c_id = Some c
-        -> ( clean_ciphers honestk advk cs $? c_id = Some c
-          /\ honest_signing_key honestk advk (cipher_signing_key c) = true)
-        \/ ( clean_ciphers honestk advk cs $? c_id = None
-          /\ honest_signing_key honestk advk (cipher_signing_key c) = false).
+        -> ( clean_ciphers allks honestk  cs $? c_id = Some c
+          /\ honest_signing_key allks honestk (cipher_signing_key c) = true)
+        \/ ( clean_ciphers allks honestk cs $? c_id = None
+          /\ honest_signing_key allks honestk (cipher_signing_key c) = false).
     Proof.
       intros.
-      case_eq (honest_signing_key honestk advk (cipher_signing_key c)); intros; eauto.
+      case_eq (honest_signing_key allks honestk (cipher_signing_key c)); intros; eauto.
       left; intuition idtac.
       eapply clean_ciphers_keeps_honest_cipher; eauto.
       unfold honest_cipher_filter_fn, cipher_signing_key in *.
@@ -403,14 +408,14 @@ Section SingleAdversarySimulates.
     Qed.
 
     Lemma clean_ciphers_no_new_ciphers :
-      forall c_id cs honestk advk,
+      forall c_id cs allks honestk,
         cs $? c_id = None
-        -> clean_ciphers honestk advk cs $? c_id = None.
+        -> clean_ciphers allks honestk cs $? c_id = None.
     Proof.
       intros.
       unfold clean_ciphers, filter.
       apply P.fold_rec_bis; intros; eauto.
-      cases (honest_cipher_filter_fn honestk advk k e); eauto.
+      cases (honest_cipher_filter_fn allks honestk k e); eauto.
       - case (c_id ==n k); intro; subst; unfold honest_cipher_filter_fn.
         + rewrite find_mapsto_iff in H0; rewrite H0 in H; invert H.
         + rewrite add_neq_o; eauto.
@@ -419,11 +424,11 @@ Section SingleAdversarySimulates.
     Hint Resolve clean_ciphers_no_new_ciphers.
 
     Lemma clean_ciphers_eliminates_added_dishonest_cipher :
-      forall c_id c honestk advk cs k,
+      forall c_id c allks honestk cs k,
         cs $? c_id = None
-        -> honest_signing_key honestk advk k = false
+        -> honest_signing_key allks honestk k = false
         -> k = cipher_signing_key c
-        -> clean_ciphers honestk advk cs = clean_ciphers honestk advk (cs $+ (c_id,c)).
+        -> clean_ciphers allks honestk cs = clean_ciphers allks honestk (cs $+ (c_id,c)).
     Proof.
       intros.
       apply map_eq_Equal; unfold Equal; intros.
@@ -435,13 +440,12 @@ Section SingleAdversarySimulates.
         rewrite fold_add; auto. simpl.
         unfold honest_cipher_filter_fn at 1.
         cases c; simpl in *; rewrite H0; trivial.
-        rewrite not_find_in_iff; assumption.
     Qed.
 
     Lemma not_in_ciphers_not_in_cleaned_ciphers :
-      forall c_id cs honestk advk,
+      forall c_id cs allks honestk,
           ~ In c_id cs
-        -> ~ In c_id (clean_ciphers honestk advk cs).
+        -> ~ In c_id (clean_ciphers allks honestk cs).
     Proof.
       intros.
       rewrite not_find_in_iff in H.
@@ -458,90 +462,75 @@ Section SingleAdversarySimulates.
         end; try discriminate.
 
     Lemma enc_message_has_honest_signing_key :
-      forall {t} k__sign k__enc honestk advk c_id (msg : message t) cipherMsg,
-          encryptMessage k__sign k__enc msg c_id = Some cipherMsg
-        -> honestk $? (keyId k__sign) = Some k__sign
-        -> adv_no_honest_keys advk honestk
-        -> key_heaps_compatible honestk advk
-        -> honest_signing_key honestk advk (keyId k__sign) = true
-        /\ cipherMsg = SigEncCipher c_id (keyId k__sign) (keyId k__enc) msg
-        /\ (k__sign.(keyType) = SymKey \/ k__sign.(keyType) = AsymKey true).
-
+      forall {t} k__sign k__enc allks honestk advk c_id (msg : message t) cipherMsg,
+          encryptMessage allks k__sign k__enc msg c_id = Some cipherMsg
+        -> honestk $? (key_ref k__sign) = Some k__sign
+        -> has_private_key allks k__sign = true
+        -> adv_no_honest_keys allks honestk advk
+        (* -> key_perms_good advk *)
+        (* -> key_heaps_compatible honestk advk *)
+        -> honest_signing_key allks honestk (key_ref k__sign) = true
+        /\ cipherMsg = SigEncCipher c_id (key_ref k__sign) (key_ref k__enc) msg.
+        (* /\ (k__sign.(keyType) = SymKey \/ k__sign.(keyType) = AsymKey true). *)
     Proof.
       intros.
       unfold encryptMessage in *.
       destruct k__sign; destruct k__enc; simpl in *.
       unfold honest_signing_key.
-      rewrite H0.
-      cases keyUsage; eauto.
-      invert H.
-      unfold key_heaps_compatible, adv_no_honest_keys in *; split_ands.
-      specialize (H1 keyId); simpl in *.
-      cases keyType; eauto; cases (advk $? keyId); auto.
-      - exfalso. specialize (H4 _ _ _ H0 Heq).
-        destruct k; unfold keys_compatible in *; simpl in *.
-        cases (keyId ==n keyId1); cases (keyType); subst; contra_map_lookup.
-        cases (has_private_access); eauto; split_ors; contra_map_lookup.
-      - cases keyUsage0; invert H; intuition idtac.
-      - destruct k; cases has_private_access; subst.
-        cases keyType; contra_map_lookup.
-        cases has_private_access; split_ors; contra_map_lookup.
-        contradiction.
-        exfalso.
-        cases keyType; contra_map_lookup.
-        cases has_private_access; split_ors; contra_map_lookup.
-        cases keyUsage0; discriminate.
-        cases keyUsage0; discriminate.
+      cases (allks $? key_ref); subst; try discriminate.
+      destruct k; simpl in *.
+      cases keyUsage; subst; try discriminate.
+      cases (allks $? key_ref0); try discriminate.
+      destruct k; simpl in *.
+      cases keyUsage; subst; try discriminate.
+      unfold sign_if_ok in *.
+      cases keyType; subst; try discriminate.
+      - invert H; intuition eauto.
+        unfold honest_key. rewrite Heq, H0.
+        specialize (H2 key_ref).
+        cases (advk $? key_ref); auto.
 
-      - cases keyUsage0.
-        cases has_private_access; invert H; eauto.
-        invert H.
+      - cases has_private_access; try discriminate; invert H; intuition idtac.
+        rewrite andb_true_r.
+        unfold honest_key. rewrite Heq. rewrite H0. trivial.
     Qed.
 
     Lemma sign_message_has_honest_signing_key :
-      forall {t} k honestk advk c_id (msg : message t) cipherMsg,
-          signMessage k msg c_id = Some cipherMsg
-        -> honestk $? (keyId k) = Some k
-        -> adv_no_honest_keys advk honestk
-        -> key_heaps_compatible honestk advk
-        -> honest_signing_key honestk advk (keyId k) = true
-        /\ cipherMsg = SigCipher c_id (keyId k) msg
-        /\ (k.(keyType) = SymKey \/ k.(keyType) = AsymKey  true).
-
+      forall {t} k allks honestk advk c_id (msg : message t) cipherMsg,
+          signMessage allks k msg c_id = Some cipherMsg
+        -> honestk $? (key_ref k) = Some k
+        -> has_private_key allks k = true
+        -> adv_no_honest_keys allks honestk advk
+        (* -> key_heaps_compatible honestk advk *)
+        -> honest_signing_key allks honestk (key_ref k) = true
+        /\ cipherMsg = SigCipher c_id (key_ref k) msg.
+        (* /\ (k.(keyType) = SymKey \/ k.(keyType) = AsymKey  true). *)
     Proof.
       intros.
       unfold signMessage in *.
       destruct k; simpl in *.
       unfold honest_signing_key.
-      rewrite H0.
-      cases keyUsage; contra_map_lookup; invert H.
-      unfold key_heaps_compatible, adv_no_honest_keys in *; split_ands.
-      specialize (H1 keyId); simpl in *.
-      cases keyType; eauto; cases (advk $? keyId); auto.
-      - exfalso. specialize (H3 _ _ _ H0 Heq).
-        destruct k; unfold keys_compatible in *; simpl in *.
-        cases (keyId ==n keyId0); cases (keyType); subst; contra_map_lookup.
-        cases (has_private_access); eauto; split_ors; contra_map_lookup.
-      - invert H4; intuition idtac.
-      - destruct k; cases has_private_access; subst; invert H4.
-        cases keyType; contra_map_lookup.
-        cases has_private_access; split_ors; contra_map_lookup.
-        contradiction.
-      - cases has_private_access; invert H4; eauto.
+      cases (allks $? key_ref); subst; try discriminate.
+      destruct k; simpl in *.
+      cases keyUsage; subst; try discriminate.
+      unfold  sign_if_ok in H.
+      cases keyType; subst; invert H.
+      - unfold honest_key; rewrite Heq,H0; auto.
+      - unfold honest_key; rewrite Heq,H0; cases has_private_access; invert H4; auto.
     Qed.
 
     Lemma dishonest_cipher_cleaned :
-      forall cs honestk advk c_id cipherMsg,
-          honest_signing_key honestk advk (cipher_signing_key cipherMsg) = false
+      forall cs allks honestk c_id cipherMsg,
+          honest_signing_key allks honestk (cipher_signing_key cipherMsg) = false
         -> ~ In c_id cs
-        -> clean_ciphers honestk advk cs = clean_ciphers honestk advk (cs $+ (c_id, cipherMsg)).
+        -> clean_ciphers allks honestk cs = clean_ciphers allks honestk (cs $+ (c_id, cipherMsg)).
     Proof.
       intros.
       apply map_eq_Equal; unfold Equal; intros.
 
       case_eq (cs $? y); intros.
 
-      - apply clean_ciphers_reduces_or_keeps_same_ciphers with (honestk:=honestk) (advk:=advk) in H1.
+      - eapply clean_ciphers_reduces_or_keeps_same_ciphers in H1.
         destruct H1; destruct H1;
           rewrite H1;
           unfold clean_ciphers, filter;
@@ -556,113 +545,86 @@ Section SingleAdversarySimulates.
         unfold honest_cipher_filter_fn; cases cipherMsg; simpl in *; rewrite H; eauto.
     Qed.
 
+    Hint Extern 1 (honest_cipher_filter_fn _ _ _ ?c = _) => unfold honest_cipher_filter_fn; cases c.
+
+    Lemma clean_ciphers_added_honest_cipher_not_cleaned :
+      forall allks honestk cs c_id c k,
+          honest_signing_key allks honestk k = true
+        -> k = cipher_signing_key c
+        -> clean_ciphers allks honestk (cs $+ (c_id,c)) = clean_ciphers allks honestk cs $+ (c_id,c).
+    Proof.
+      intros.
+      apply map_eq_Equal; unfold Equal; intros.
+      (* unfold honest_signing_key,honest_key in H. *)
+
+      case (y ==n c_id); intros; subst; clean_map_lookups.
+      - erewrite clean_ciphers_keeps_honest_cipher; auto.
+      - case_eq (clean_ciphers allks honestk cs $? y); intros; subst.
+        + case_eq (cs $? c_id); intros; subst; auto.
+          * case_eq (cs $? y); intros; subst; auto.
+            ** assert (cs $? y = Some c2) as HH by assumption;
+                 eapply clean_ciphers_reduces_or_keeps_same_ciphers in HH; invert HH;
+                   split_ands; subst; contra_map_lookup.
+
+               apply clean_ciphers_keeps_honest_cipher; auto.
+
+            ** exfalso. eapply clean_ciphers_no_new_ciphers in H2; contra_map_lookup.
+
+          * unfold clean_ciphers, filter.
+            rewrite fold_add; auto.
+            unfold honest_cipher_filter_fn.
+            cases c; simpl in *; rewrite H; auto.
+        + case_eq (cs $? y); intros; subst; eauto.
+          eapply clean_ciphers_eliminates_dishonest_cipher; eauto.
+          case_eq (honest_signing_key allks honestk (cipher_signing_key c0)); intros; subst; auto.
+          exfalso; eapply clean_ciphers_keeps_honest_cipher in H1; contra_map_lookup; auto.
+    Qed.
+
     Lemma honest_enc_cipher_not_cleaned :
-      forall {t} cs k__sign k__enc honestk advk c_id (msg : message t) cipherMsg,
-          encryptMessage k__sign k__enc msg c_id = Some cipherMsg
-        -> honestk $? (keyId k__sign) = Some k__sign
-        -> adv_no_honest_keys advk honestk
-        -> key_heaps_compatible honestk advk
-        -> clean_ciphers honestk advk (cs $+ (c_id, cipherMsg)) = clean_ciphers honestk advk cs $+ (c_id, cipherMsg).
+      forall {t} cs k__sign k__enc allks honestk advk c_id (msg : message t) cipherMsg,
+          encryptMessage allks k__sign k__enc msg c_id = Some cipherMsg
+        -> honestk $? (key_ref k__sign) = Some k__sign
+        -> has_private_key allks k__sign = true
+        -> adv_no_honest_keys allks honestk advk
+        -> clean_ciphers allks honestk (cs $+ (c_id, cipherMsg)) = clean_ciphers allks honestk cs $+ (c_id, cipherMsg).
     Proof.
       intros.
       pose proof (enc_message_has_honest_signing_key _ _ _ H H0 H1 H2) as HONEST; split_ands.
-
-      apply map_eq_Equal; unfold Equal; intros.
-
-      case (y ==n c_id); intros; subst.
-      - m_equal.
-        erewrite clean_ciphers_keeps_honest_cipher; eauto.
-      - rewrite add_neq_o by auto.
-        case_eq (clean_ciphers honestk advk cs $? y); intros; subst.
-        + case_eq (cs $? c_id); intros; subst; eauto.
-          * case_eq (cs $? y); intros; subst; eauto.
-            ** assert (cs $? y = Some c1) as HH by assumption;
-                 eapply clean_ciphers_reduces_or_keeps_same_ciphers in HH; invert HH; invert H4; subst;
-                   split_ands; contra_map_lookup.
-
-               rewrite H4. 
-               apply clean_ciphers_keeps_honest_cipher; eauto.
-               unfold honest_cipher_filter_fn; cases c; eauto.
-
-            ** exfalso. eapply clean_ciphers_no_new_ciphers in H7; contra_map_lookup.
-
-          * unfold clean_ciphers, filter.
-            rewrite fold_add; auto.
-            unfold honest_cipher_filter_fn.
-            rewrite H3; simpl.
-            rewrite add_neq_o; eauto.
-            rewrite not_find_in_iff; assumption.
-        + case_eq (cs $? y); intros; subst; eauto.
-          eapply clean_ciphers_eliminates_dishonest_cipher; eauto.
-          case_eq (honest_signing_key honestk advk (cipher_signing_key c)); intros; subst; eauto.
-          exfalso.
-          eapply clean_ciphers_keeps_honest_cipher in H6; contra_map_lookup.
-          unfold honest_cipher_filter_fn; cases c; eauto.
+      eapply clean_ciphers_added_honest_cipher_not_cleaned; subst; eauto.
     Qed.
 
     Lemma honest_sign_cipher_not_cleaned :
-      forall {t} cs k honestk advk c_id (msg : message t) cipherMsg,
-          signMessage k msg c_id = Some cipherMsg
-        -> honestk $? (keyId k) = Some k
-        -> adv_no_honest_keys advk honestk
-        -> key_heaps_compatible honestk advk
-        (* -> honest_signing_key honestk advk (keyId k) = true *)
-        -> clean_ciphers honestk advk (cs $+ (c_id, cipherMsg)) = clean_ciphers honestk advk cs $+ (c_id, cipherMsg).
+      forall {t} cs k allks honestk advk c_id (msg : message t) cipherMsg,
+          signMessage allks k msg c_id = Some cipherMsg
+        -> honestk $? (key_ref k) = Some k
+        -> has_private_key allks k = true
+        -> adv_no_honest_keys allks honestk advk
+        -> clean_ciphers allks honestk (cs $+ (c_id, cipherMsg)) = clean_ciphers allks honestk cs $+ (c_id, cipherMsg).
     Proof.
       intros.
       pose proof (sign_message_has_honest_signing_key _ _ H H0 H1 H2) as HONEST; split_ands.
-
-      apply map_eq_Equal; unfold Equal; intros.
-
-      case (y ==n c_id); intros; subst.
-      - m_equal.
-        erewrite clean_ciphers_keeps_honest_cipher; eauto.
-      - rewrite add_neq_o by auto.
-        case_eq (clean_ciphers honestk advk cs $? y); intros; subst.
-        + case_eq (cs $? c_id); intros; subst; eauto.
-          * case_eq (cs $? y); intros; subst; eauto.
-            ** assert (cs $? y = Some c1) as HH by assumption;
-                 eapply clean_ciphers_reduces_or_keeps_same_ciphers in HH; invert HH; invert H4; subst;
-                   split_ands; contra_map_lookup.
-
-               rewrite H4.
-               apply clean_ciphers_keeps_honest_cipher; eauto.
-               unfold honest_cipher_filter_fn; cases c; eauto.
-
-            ** exfalso. eapply clean_ciphers_no_new_ciphers in H7; contra_map_lookup.
-
-          * unfold clean_ciphers, filter.
-            rewrite fold_add; auto.
-            unfold honest_cipher_filter_fn.
-            rewrite H3; simpl.
-            rewrite add_neq_o; eauto.
-            rewrite not_find_in_iff; assumption.
-        + case_eq (cs $? y); intros; subst; eauto.
-          eapply clean_ciphers_eliminates_dishonest_cipher; eauto.
-          case_eq (honest_signing_key honestk advk (cipher_signing_key c)); intros; subst; eauto.
-          exfalso.
-          eapply clean_ciphers_keeps_honest_cipher in H6; contra_map_lookup.
-          unfold honest_cipher_filter_fn; cases c; eauto.
+      eapply clean_ciphers_added_honest_cipher_not_cleaned; subst; eauto.
     Qed.
 
     Hint Resolve honest_enc_cipher_not_cleaned honest_sign_cipher_not_cleaned.
 
     Lemma honest_silent_step_advuniv_implies_honest_step_origuniv :
-      forall {A B C} cs cs' lbl (usrs usrs' : honest_users A) (adv adv' : user_data B) ks ks' qmsgs qmsgs' bd bd' b,
+      forall {A B C} cs cs' lbl (usrs usrs' : honest_users A) (adv adv' : user_data B) gks gks' ks ks' qmsgs qmsgs' bd bd' b,
         step_user lbl bd bd'
         -> forall (cmd : user_cmd C) cs__s honestk,
           honestk = findUserKeys usrs
-          -> adv_no_honest_keys adv.(key_heap) honestk
-          -> key_heaps_compatible honestk adv.(key_heap)
-          -> cs__s = clean_ciphers honestk adv.(key_heap) cs
-          -> bd = (usrs, adv, cs, ks, qmsgs, cmd)
+          -> adv_no_honest_keys gks honestk adv.(key_heap)
+          -> ciphers_honestly_signed gks honestk cs = true
+          (* -> key_heaps_compatible honestk adv.(key_heap) *)
+          -> cs__s = clean_ciphers gks honestk cs
+          -> bd = (usrs, adv, cs, gks, ks, qmsgs, cmd)
           -> forall cmd' cs__s',
-              cs__s' = clean_ciphers honestk adv.(key_heap) cs'
-              -> bd' = (usrs', adv', cs', ks', qmsgs', cmd')
+              cs__s' = clean_ciphers gks' honestk cs'
+              -> bd' = (usrs', adv', cs', gks', ks', qmsgs', cmd')
               -> lbl = Silent
-              -> step_user (B:=B) lbl (usrs, powerless_adv b, cs__s, ks, qmsgs, cmd) (usrs', powerless_adv b, cs__s', ks', qmsgs', cmd').
+              -> step_user (B:=B) lbl (usrs, powerless_adv b, cs__s, gks, ks, qmsgs, cmd) (usrs', powerless_adv b, cs__s', gks', ks', qmsgs', cmd').
     Proof.
-      induction 1; inversion 5; inversion 2; intro; subst;
+      induction 1; inversion 5; inversion 2; intros; subst;
         repeat match goal with
                | [ H : Action _ = Silent |- _ ] => invert H
                end;
@@ -671,106 +633,96 @@ Section SingleAdversarySimulates.
 
       - eapply honest_enc_cipher_not_cleaned; eauto.
         admit. (* need link that the ks is in findUserKeys usrs *)
-      - eapply clean_ciphers_keeps_honest_cipher; eauto.
-        unfold honest_cipher_filter_fn, honest_signing_key.
-        unfold adv_no_honest_keys in H5. specialize (H5 (keyId k__sign)).
+        
+      - assert (key_ref k__sign = k__signid) by admit.
         assert (findUserKeys usrs' $? k__signid = Some k__sign) by admit.
-        unfold key_heaps_compatible in *; split_ands.
-        unfold keys_good in *.
-        assert (keyId k__sign = k__signid) by auto.
-        destruct k__sign; subst; simpl in *.
+        subst.
 
-        cases (key_heap adv' $? keyId).
-        + rewrite H2. assert (RealWorld.keyId k = keyId) by auto; destruct k; subst; simpl in *.
-          cases keyUsage.
-          * exfalso. admit.
-          * cases keyType; cases keyType0; eauto; contra_map_lookup.
-            ** exfalso. cases has_private_access; eauto; split_ors; contra_map_lookup.
-            ** cases has_private_access0; eauto; split_ors; contra_map_lookup.
+        Ltac foo1 :=
+          match goal with
+          |  [ H : ?x = ?x |- _ ] => clear H
+          | [ |- clean_ciphers _ _ _ $? _ = Some _ ] => eapply clean_ciphers_keeps_honest_cipher
+          | [ |- honest_cipher_filter_fn _ _ _ _ = _ ] => unfold honest_cipher_filter_fn, honest_signing_key,honest_key
+          | [ H : ?m $? ?k = _ |- context[?m $? ?k] ] => rewrite H 
+          | [ |- context [match ?matchee with _ => _ end] ] => cases matchee; subst
+          | [ |- ?hasp && _ = _ ] => cases hasp; simpl
+          | [ |- false = true ] => exfalso; simpl in *
+          | [ H : _ && _ = true |- _ ] => apply andb_prop in H; split_ands
+          | [ H : match ?matchee with _ => _ end = _
+           ,  H1 : ?matchee = _ |- _] => rewrite H1 in H
+          | [ H  : ciphers_honestly_signed ?gks ?ks ?cs = true
+            , H1 : ?cs $? _ = Some ?c
+              |- cipher_honestly_signed ?gks ?ks ?c = true] =>
+            unfold ciphers_honestly_signed in H; rewrite for_all_iff in H by auto; eapply H
+          | [ |- MapsTo _ _ _ ] => apply find_mapsto_iff
+          | [ H : cipher_honestly_signed _ _ _ = true |- _ ] => unfold cipher_honestly_signed,honest_signing_key, honest_key in H
+          end.
 
-          (* TODO tbraje: this is where I left off before other refactorings *)
-               admit. admit.
+        Ltac doit :=
+          repeat foo1; auto;
+          match goal with
+          | [ H  : ciphers_honestly_signed ?gks ?ks ?cs = true
+            , H1 : ?cs $? _ = Some ?c
+              |- False ] => assert (cipher_honestly_signed gks ks c = true)
+          end;
+          repeat foo1; eauto.
 
-        + admit.
+        doit; discriminate.
 
-      - admit.
-      - admit.
-                                     
-      (* - apply clean_ciphers_keeps_honest_cipher; unfold honest_cipher; eauto. *)
-      (*   unfold adv_no_honest_keys in H5. specialize (H5 k__signid). *)
-      (*   cases (findUserKeys adv' $? k__signid); auto. *)
-      (*   destruct k; cases keyType; auto. *)
-      (*   rewrite H1 in H5; invert H5. *)
-      (*   cases has_private_access; auto. *)
-      (*   rewrite H1 in H5; invert H5. *)
+      - eapply honest_sign_cipher_not_cleaned; eauto.
+        admit.
 
-      (* - eapply honest_sign_cipher_not_cleaned; eauto. *)
-      (*   unfold adv_no_honest_keys in H5. specialize (H5 (keyId k)). *)
-      (*   cases (findUserKeys adv' $? keyId k); auto. *)
-      (*     right; exists k0. destruct k0. cases keyType; simpl; eauto. *)
-      (*     rewrite H5 in H0; invert H0. *)
-      (*     cases has_private_access; eauto. *)
-      (*     rewrite H5 in H0; invert H0. *)
-
-      (* - apply clean_ciphers_keeps_honest_cipher; unfold honest_cipher; eauto. *)
-      (*   unfold adv_no_honest_keys in H3. specialize (H3 (keyId k)). *)
-      (*   cases (findUserKeys adv' $? keyId k); auto. *)
-      (*   destruct k0; cases keyType; auto. *)
-      (*   rewrite H3 in H0; invert H0. *)
-      (*   cases has_private_access; auto. *)
-      (*   rewrite H3 in H0; invert H0. *)
+      - assert (findUserKeys usrs' $? key_ref k = Some k) by admit.
+        doit; discriminate.
 
     Admitted.
 
     Lemma honest_loud_step_advuniv_implies_honest_step_origuniv :
-      forall {A B C} cs cs' lbl (usrs usrs' : honest_users A) (adv adv' : user_data B) ks ks' qmsgs qmsgs' bd bd' a b,
+      forall {A B C} cs cs' lbl (usrs usrs' : honest_users A) (adv adv' : user_data B) gks gks' ks ks' qmsgs qmsgs' bd bd' a b,
         step_user lbl bd bd'
         -> forall (cmd : user_cmd C) cs__s honestk,
           honestk = findUserKeys usrs
-          -> adv_no_honest_keys adv.(key_heap) ks
-          -> cs__s = clean_ciphers honestk adv.(key_heap) cs
-          -> bd = (usrs, adv, cs, ks, qmsgs, cmd)
+          -> adv_no_honest_keys gks honestk adv.(key_heap)
+          -> cs__s = clean_ciphers gks honestk cs
+          -> bd = (usrs, adv, cs, gks, ks, qmsgs, cmd)
           -> forall cmd' cs__s',
-              cs__s' = clean_ciphers honestk adv.(key_heap) cs'
-              -> bd' = (usrs', adv', cs', ks', qmsgs', cmd')
+              cs__s' = clean_ciphers gks honestk cs'
+              -> bd' = (usrs', adv', cs', gks', ks', qmsgs', cmd')
               -> lbl = Action a
-              -> action_adversary_safe honestk adv.(key_heap) a = true
-              -> step_user (B:=B) lbl (usrs, powerless_adv b, cs__s, ks, qmsgs, cmd) (usrs', powerless_adv b, cs__s', ks', qmsgs', cmd').
+              -> action_adversary_safe gks honestk adv.(key_heap) a = true
+              -> step_user (B:=B) lbl (usrs, powerless_adv b, cs__s, gks, ks, qmsgs, cmd) (usrs', powerless_adv b, cs__s', gks', ks', qmsgs', cmd').
     Proof.
       induction 1; inversion 4; inversion 2; intro; subst; econstructor; eauto; try discriminate.
 
-      - invert H16. unfold action_adversary_safe in H.
+      - invert H17. unfold action_adversary_safe in H.
         eapply clean_ciphers_accepts_non_spoofable; eauto.
-        admit.
-        (* unfold negb in H; cases (msg_pattern_spoofable (findUserKeys adv') pat); eauto. *)
+        rewrite <- negb_true_iff; assumption.
 
-      - unfold addUserKeys; m_equal; simpl. admit.
+      - unfold addUserKeys, powerless_adv; f_equal; simpl. admit. (* add constraint to operational semantics *)
         
     Admitted.
 
     Lemma honest_silent_step_nochange_adversaries :
-      forall {A B C} cs cs' lbl (usrs usrs' : honest_users A) (adv adv' : user_data B) ks ks' qmsgs qmsgs' bd bd',
+      forall {A B C} cs cs' lbl (usrs usrs' : honest_users A) (adv adv' : user_data B) gks gks' ks ks' qmsgs qmsgs' bd bd',
         step_user lbl bd bd'
         -> forall (cmd : user_cmd C),
-          bd = (usrs, adv, cs, ks, qmsgs, cmd)
+          bd = (usrs, adv, cs, gks, ks, qmsgs, cmd)
           -> lbl = Silent
           -> forall cmd',
-              bd' = (usrs', adv', cs', ks', qmsgs', cmd')
+              bd' = (usrs', adv', cs', gks', ks', qmsgs', cmd')
             -> adv = adv'.
     Proof.
       induction 1; inversion 1; inversion 2; subst; eauto.
       invert H4.
     Qed.
 
-
-
     Lemma user_step_adds_no_users :
-      forall {A B C} cs cs' lbl (usrs usrs' : honest_users A) (adv adv' : user_data B) ks ks' qmsgs qmsgs' bd bd',
+      forall {A B C} cs cs' lbl (usrs usrs' : honest_users A) (adv adv' : user_data B) gks gks' ks ks' qmsgs qmsgs' bd bd',
         step_user lbl bd bd'
         -> forall (cmd : user_cmd C),
-          bd = (usrs, adv, cs, ks, qmsgs, cmd)
+          bd = (usrs, adv, cs, gks, ks, qmsgs, cmd)
           -> forall cmd',
-            bd' = (usrs', adv', cs', ks', qmsgs', cmd')
+            bd' = (usrs', adv', cs', gks', ks', qmsgs', cmd')
             -> forall u_id' u_d,
               usrs' $? u_id' = Some u_d
               -> usrs $? u_id' <> None.
@@ -780,10 +732,7 @@ Section SingleAdversarySimulates.
                | [ H : ?us $? ?uid = Some _ |- ?us $? ?uid <> None ] => solve [ rewrite H; intro C; invert C ]
                end.
 
-      case (u_id' ==n rec_u_id); intro.
-      - subst. rewrite H1; intro C; invert C.
-      - rewrite add_neq_o in H11 by auto.
-        rewrite H11; intro C; invert C.
+      case (u_id' ==n rec_u_id); intro; subst; unfold not; intros; clean_map_lookups.
     Qed.
 
     (* Lemma user_step_adds_removes_no_adversaries : *)
@@ -874,104 +823,90 @@ Section SingleAdversarySimulates.
 
 
     Lemma adv_step_implies_no_new_ciphers_after_cleaning :
-      forall {A B C} cs cs' lbl (usrs usrs' : honest_users A) (adv adv' : user_data B) ks' qmsgs' bd bd',
+      forall {A B C} cs cs' lbl (usrs usrs' : honest_users A) (adv adv' : user_data B) gks gks' ks' qmsgs' bd bd',
         step_user lbl bd bd'
         -> forall (cmd : user_cmd C) honestk cs__s,
-            bd = (usrs, adv, cs, adv.(key_heap), adv.(msg_heap), cmd)
+            bd = (usrs, adv, cs, gks, adv.(key_heap), adv.(msg_heap), cmd)
           -> honestk = findUserKeys usrs
-          (* -> key_heaps_compatible (findUserKeys usrs) adv.(key_heap) *)
-          -> adv_no_honest_keys adv.(key_heap) (findUserKeys usrs)
-          -> message_queue_safe honestk adv.(msg_heap) = true
-          -> cs__s = clean_ciphers honestk adv.(key_heap) cs
+          -> all_user_key_perms_good usrs
+          -> keys_good gks
+          -> adv_no_honest_keys gks (findUserKeys usrs) adv.(key_heap)
+          -> message_queue_safe gks honestk adv.(msg_heap) = true
+          -> cs__s = clean_ciphers gks honestk cs
           -> forall cmd' honestk' cs__s',
-                bd' = (usrs', adv', cs', ks', qmsgs', cmd')
-              -> honestk' = findUserKeys usrs
-              -> cs__s' = clean_ciphers honestk' (adv'.(key_heap) $k++ ks') cs'
+                bd' = (usrs', adv', cs', gks', ks', qmsgs', cmd')
+              -> honestk' = findUserKeys usrs'
+              -> cs__s' = clean_ciphers gks' honestk' cs'
               -> cs__s = cs__s'.
     Proof.
-      induction 1; inversion 1; inversion 5; intros; subst;
+      induction 1; inversion 1; inversion 7; intros; subst;
         try rewrite merge_keys_refl; eauto.
 
-      (* Recv *)
-      - rewrite <- merge_keys_assoc, merge_keys_refl.
-        admit. (* need small lemmas about safe message queues and finding keys in messages *)
-
       (* Send *)
-      - simpl; rewrite merge_keys_symmetric, <- merge_keys_assoc, merge_keys_refl.
-        admit. (* how can we prove that the adversary couldn't have created a message with any honest keys here? *)
+      - erewrite findUserKeys_readd_user_same_keys_idempotent; eauto using findUserKeys_result_perms_good.
 
       (* Encrypt *)
-      - assert (honest_signing_key (findUserKeys usrs') (key_heap adv') (cipher_signing_key cipherMsg) = false).
+      - assert (honest_signing_key gks' (findUserKeys usrs') (cipher_signing_key cipherMsg) = false).
         unfold encryptMessage, adv_no_honest_keys in *.
         unfold honest_signing_key.
         destruct k__sign; destruct k__enc; simpl in *.
-        specialize (H14 keyId).
-        cases keyUsage; cases keyUsage0; try discriminate.
-        cases keyType; try discriminate.
-        invert H4; simpl; rewrite H1 in H14; rewrite H14; trivial.
-        cases has_private_access; invert H4; simpl; rewrite H1 in H14; split_ors; rewrite H; trivial.
+        specialize (H18 key_ref).
+        cases (gks' $? key_ref); try discriminate.
+        destruct k; simpl in *. cases keyType; rewrite H1 in *; try contradiction.
+          cases keyUsage; try discriminate.
+          cases (gks' $? key_ref0); try discriminate. destruct k; simpl in *. cases keyUsage; try discriminate.
+          unfold sign_if_ok in *; cases has_private_access; invert H5. simpl. rewrite Heq, H18; auto.
 
-        eapply clean_ciphers_eliminates_added_dishonest_cipher; eauto.
-        rewrite <- not_find_in_iff; assumption.
+        eapply clean_ciphers_eliminates_added_dishonest_cipher; clean_map_lookups; eauto.
 
-      (* Decrypt *)
-      - rewrite <- merge_keys_assoc, merge_keys_refl.
-        admit.
-
-      (* Sign *)
-      - assert (honest_signing_key (findUserKeys usrs') (key_heap adv') (cipher_signing_key cipherMsg) = false).
+      - assert (honest_signing_key gks' (findUserKeys usrs') (cipher_signing_key cipherMsg) = false).
         unfold signMessage, adv_no_honest_keys in *.
         unfold honest_signing_key.
         destruct k; simpl in *.
-        specialize (H12 keyId).
-        cases keyUsage; cases keyType; try discriminate.
-        invert H2; simpl; rewrite H0 in H12; rewrite H12; trivial.
-        cases has_private_access; invert H2; simpl; rewrite H0 in H12; split_ors; rewrite H; trivial.
+        specialize (H16 key_ref).
+        cases (gks' $? key_ref); try discriminate.
+        destruct k; simpl in *. cases keyType; rewrite H0 in *; try contradiction.
+          cases keyUsage; try discriminate.
+          cases (gks' $? key_ref); try discriminate. invert Heq.
+          unfold sign_if_ok in *; cases has_private_access; invert H3. simpl. rewrite Heq0, H16; auto.
 
-        eapply clean_ciphers_eliminates_added_dishonest_cipher; eauto.
-        rewrite <- not_find_in_iff; assumption.
+        eapply clean_ciphers_eliminates_added_dishonest_cipher; clean_map_lookups; eauto.
 
-    Admitted.
+    Qed.
 
     Lemma adv_step_implies_no_user_impact_after_cleaning :
-      forall {A B C} cs cs' lbl (usrs usrs' : honest_users A) (adv adv' : user_data B) ks' qmsgs' bd bd',
+      forall {A B C} cs cs' lbl (usrs usrs' : honest_users A) (adv adv' : user_data B) gks gks' ks' qmsgs' bd bd',
         step_user lbl bd bd'
         -> forall (cmd : user_cmd C) honestk usrs__s,
-            bd = (usrs, adv, cs, adv.(key_heap), adv.(msg_heap), cmd)
+            bd = (usrs, adv, cs, gks, adv.(key_heap), adv.(msg_heap), cmd)
           -> honestk = findUserKeys usrs
-          -> usrs__s = clean_users honestk adv.(key_heap) usrs
+          -> usrs__s = clean_users gks honestk cs usrs
           -> forall cmd' honestk' usrs__s',
-                bd' = (usrs', adv', cs', ks', qmsgs', cmd')
+                bd' = (usrs', adv', cs', gks', ks', qmsgs', cmd')
               -> honestk' = findUserKeys usrs'
-              -> usrs__s' = clean_users honestk' (adv'.(key_heap) $k++ ks') usrs'
+              -> usrs__s' = clean_users gks' honestk' cs' usrs'
               -> usrs__s = usrs__s'.
     Proof.
       induction 1; inversion 1; inversion 3; intros; subst;
         try rewrite merge_keys_refl; eauto.
 
-      (* Recv *)
-      - rewrite <- merge_keys_assoc, merge_keys_refl. 
-        admit.
-
-      (* Send *)
-      - simpl. rewrite merge_keys_symmetric, <- merge_keys_assoc, merge_keys_refl.
-         admit.
-
-      (* Decrypt *)
-      - rewrite <- merge_keys_assoc, merge_keys_refl.
-        admit.
+      (* Sent *)
+      (* Encrypt *)
+      (* Sign *)
 
     Admitted.
 
 
     Lemma adv_step_stays_in_R :
       forall {A B} (U__i : IdealWorld.universe A) (U__r : universe A B) (R : universe A B -> IdealWorld.universe A -> Prop) (b : B)
-        (cmd : user_cmd B) lbl (usrs : honest_users A) (adv : user_data B) cs ks qmsgs,
+        (cmd : user_cmd B) lbl (usrs : honest_users A) (adv : user_data B) cs gks ks qmsgs,
         step_user lbl
                   (build_data_step U__r U__r.(adversary))
-                  (usrs, adv, cs, ks, qmsgs, cmd)
+                  (usrs, adv, cs, gks, ks, qmsgs, cmd)
         -> R (strip_adversary U__r b) U__i
-        -> R (strip_adversary (buildUniverseAdv usrs cs {| key_heap := adv.(key_heap) $k++ ks; protocol := cmd; msg_heap := qmsgs |}) b) U__i.
+        -> adv_no_honest_keys (all_keys U__r) (findUserKeys (users U__r)) (key_heap (adversary U__r))
+        -> message_queue_safe (all_keys U__r) (findUserKeys (users U__r)) (msg_heap (adversary U__r)) = true
+        -> R (strip_adversary (buildUniverseAdv usrs cs gks {| key_heap := adv.(key_heap) $k++ ks; protocol := cmd; msg_heap := qmsgs |}) b) U__i.
     Proof.
       intros.
       unfold buildUniverseAdv, strip_adversary, build_data_step in *; subst; simpl.
@@ -982,12 +917,18 @@ Section SingleAdversarySimulates.
         idtac cs; idtac cs'
       end.
 
-      assert ( (clean_users (findUserKeys (users U__r)) (key_heap (adversary U__r)) (users U__r)) = (clean_users (findUserKeys usrs) (key_heap adv $k++ ks) usrs) ).
-      eapply adv_step_implies_no_user_impact_after_cleaning; eauto.
+      assert ( clean_users U__r.(all_keys) (findUserKeys U__r.(users)) U__r.(all_ciphers) (users U__r)
+             = clean_users gks (findUserKeys usrs) cs usrs ) by eauto using adv_step_implies_no_user_impact_after_cleaning.
 
-      assert ( (clean_ciphers (findUserKeys (users U__r)) (key_heap (adversary U__r)) (all_ciphers U__r)) = (clean_ciphers (findUserKeys usrs) (key_heap adv $k++ ks) cs) ).
+      assert ( (clean_ciphers (all_keys U__r) (findUserKeys (users U__r)) (all_ciphers U__r)) =
+               (clean_ciphers gks (findUserKeys usrs) cs) ).
       eapply adv_step_implies_no_new_ciphers_after_cleaning; eauto.
 
+      (* assert ( (clean_users (findUserKeys (users U__r)) (key_heap (adversary U__r)) (users U__r)) = (clean_users (findUserKeys usrs) (key_heap adv $k++ ks) usrs) ). *)
+      (* eapply adv_step_implies_no_user_impact_after_cleaning; eauto. *)
+
+      (* assert ( (clean_ciphers (findUserKeys (users U__r)) (key_heap (adversary U__r)) (all_ciphers U__r)) = (clean_ciphers (findUserKeys usrs) (key_heap adv $k++ ks) cs) ). *)
+      (* eapply adv_step_implies_no_new_ciphers_after_cleaning; eauto. *)
 
 
 
@@ -1044,7 +985,6 @@ Section SingleAdversarySimulates.
 
 
 
-
   Hint Constructors RealWorld.step_user.
 
   Hint Extern 1 (rstepSilent _ (strip_adversary _)) => 
@@ -1070,18 +1010,29 @@ Section SingleAdversarySimulates.
     end.
   Hint Extern 1 (_ = RealWorld.adversary _) => solve [ symmetry ; assumption ].
 
+
+      (* -> RealWorld.keys_good U__r.(RealWorld.all_keys) *)
+      (* -> RealWorld.all_user_key_perms_good U__r.(RealWorld.users) *)
+      (* -> RealWorld.adv_no_honest_keys U__r.(RealWorld.all_keys) U__r.(RealWorld.adversary).(RealWorld.key_heap) (RealWorld.findUserKeys U__r.(RealWorld.users)) *)
+      (* -> forall U__r', *)
+      (*     rstepSilent U__r U__r' *)
+      (*     -> exists U__i', *)
+      (*       istepSilent ^* U__i U__i' *)
+      (*       /\ R U__r' U__i') *)
+
+
   Lemma simulates_with_adversary_silent :
     forall {A B} (U__ra : RealWorld.universe A B) (U__i : IdealWorld.universe A) (R : RealWorld.universe A B -> IdealWorld.universe A -> Prop) (b : B),
       (forall (U__r : RealWorld.universe A B) (U__i : IdealWorld.universe A),
           R U__r U__i
-          -> RealWorld.key_heaps_compatible (RealWorld.findUserKeys (RealWorld.users U__r)) (RealWorld.key_heap (RealWorld.adversary U__r))
-          -> RealWorld.adv_no_honest_keys (RealWorld.key_heap (RealWorld.adversary U__r)) (RealWorld.findUserKeys (RealWorld.users U__r))
+          -> RealWorld.all_user_key_perms_good U__r.(RealWorld.users)
+          -> RealWorld.adv_no_honest_keys U__r.(RealWorld.all_keys) (RealWorld.findUserKeys (RealWorld.users U__r)) (RealWorld.key_heap (RealWorld.adversary U__r))
           -> forall U__r' : RealWorld.universe A B,
               rstepSilent U__r U__r'
               -> exists U__i' : IdealWorld.universe A, (istepSilent) ^* U__i U__i' /\ R U__r' U__i')
 
-      -> RealWorld.key_heaps_compatible (RealWorld.findUserKeys (RealWorld.users U__ra)) (RealWorld.key_heap (RealWorld.adversary U__ra))
-      -> RealWorld.adv_no_honest_keys U__ra.(RealWorld.adversary).(RealWorld.key_heap) (RealWorld.findUserKeys U__ra.(RealWorld.users))
+      -> RealWorld.all_user_key_perms_good U__ra.(RealWorld.users)
+      -> RealWorld.adv_no_honest_keys U__ra.(RealWorld.all_keys) (RealWorld.findUserKeys U__ra.(RealWorld.users)) U__ra.(RealWorld.adversary).(RealWorld.key_heap)
       -> R (strip_adversary U__ra b) U__i
       -> forall U__ra',
           rstepSilent U__ra U__ra'
